<?xml version="1.0"?>
<rdf:RDF xmlns="http://semanticbible.org/ns/2006/NTNames#"
     xml:base="http://semanticbible.org/ns/2006/NTNames"
     xmlns:dc="http://purl.org/dc/elements/1.1/"
     xmlns:rdfs="http://www.w3.org/2000/01/rdf-schema#"
     xmlns:owl="http://www.w3.org/2002/07/owl#"
     xmlns:xsd="http://www.w3.org/2001/XMLSchema#"
     xmlns:rdf="http://www.w3.org/1999/02/22-rdf-syntax-ns#"
     xmlns:rss="http://purl.org/rss/1.0/">
    <owl:Ontology rdf:about="http://semanticbible.org/ns/2006/NTNames">
        <owl:versionInfo rdf:datatype="http://www.w3.org/2001/XMLSchema#string">1.0</owl:versionInfo>
        <rdfs:comment xml:lang="en">The names here are as
transliterated in the English Standard Version (ESV), copyright Â©
2001 by Crossway Bibles, a division of Good News Publishers.

Reuse note: where feasible, class names coincide with SUMO (Suggested
Upper Merged Ontology), as developed within the IEEE Standard Upper
Ontology Working Group, described at http://www.ontologyportal.org/,
and available as OWL at http://reliant.teknowledge.com/DAML/SUMO.owl
(but not without some problems). I&#39;ve copied, rather than re-used, but
this provides a future migration path toward coordinating the two
ontologies.

</rdfs:comment>
    </owl:Ontology>
    


    <!-- 
    ///////////////////////////////////////////////////////////////////////////////////////
    //
    // Annotation properties
    //
    ///////////////////////////////////////////////////////////////////////////////////////
     -->

    


    <!-- 
    ///////////////////////////////////////////////////////////////////////////////////////
    //
    // Datatypes
    //
    ///////////////////////////////////////////////////////////////////////////////////////
     -->

    


    <!-- 
    ///////////////////////////////////////////////////////////////////////////////////////
    //
    // Object Properties
    //
    ///////////////////////////////////////////////////////////////////////////////////////
     -->

    


    <!-- http://semanticbible.org/ns/2006/NTNames#antagonistOf -->

    <owl:ObjectProperty rdf:about="http://semanticbible.org/ns/2006/NTNames#antagonistOf">
        <rdfs:label xml:lang="en">antagonist of</rdfs:label>
        <rdfs:comment xml:lang="en">&quot;A person who opposes and contends against this person&quot;, similar to http://purl.org/vocab/relationship vocabulary, but with different domain and range. For clarity, &lt;X antagonistOf Y&gt; means X opposes, etc. Y, and also (by inference) &lt;Y hasAntagonist X&gt;. However, it does _not_ necessarily mean &lt;Y antagonistOf X&gt;, i.e. it is not necessarily reciprocal.</rdfs:comment>
        <rdfs:subPropertyOf rdf:resource="http://semanticbible.org/ns/2006/NTNames#knows"/>
    </owl:ObjectProperty>
    


    <!-- http://semanticbible.org/ns/2006/NTNames#childOf -->

    <owl:ObjectProperty rdf:about="http://semanticbible.org/ns/2006/NTNames#childOf">
        <rdfs:label xml:lang="en">child of</rdfs:label>
        <rdfs:comment xml:lang="en">Similar to http://purl.org/vocab/relationship vocabulary, but with different domain and range. In-laws are considered relatives. </rdfs:comment>
        <rdfs:subPropertyOf rdf:resource="http://semanticbible.org/ns/2006/NTNames#relativeOf"/>
    </owl:ObjectProperty>
    


    <!-- http://semanticbible.org/ns/2006/NTNames#collaboratesWith -->

    <owl:ObjectProperty rdf:about="http://semanticbible.org/ns/2006/NTNames#collaboratesWith">
        <rdfs:label xml:lang="en">collaborates with</rdfs:label>
        <rdfs:comment xml:lang="en">&quot;A person who works toward a common goal with this person&quot;, similar to http://purl.org/vocab/relationship vocabulary, but with different domain and range. Those to whom the author of a New Testament Epistle send greetings are assumed to be collaborators, though this is perhaps broader than the general sense of the word. However, simple Christian fellowship or conversion do not constitute collaboration in this sense. </rdfs:comment>
        <rdfs:subPropertyOf rdf:resource="http://semanticbible.org/ns/2006/NTNames#knows"/>
    </owl:ObjectProperty>
    


    <!-- http://semanticbible.org/ns/2006/NTNames#enemyOf -->

    <owl:ObjectProperty rdf:about="http://semanticbible.org/ns/2006/NTNames#enemyOf">
        <rdfs:label xml:lang="en">enemy of</rdfs:label>
        <rdfs:comment xml:lang="en">&quot;A person towards whom this person feels hatred, intends injury to, or opposes the interests of&quot;, similar to http://purl.org/vocab/relationship vocabulary, but with different domain and range. For clarity, &lt;X, enemyOf, Y&gt; means X feels hatred, etc. towards Y, and also (by inference) &lt;Y, hasEnemy, X&gt;. However, it does _not_ necessarily mean &lt;Y, enemyOf, X&gt;, i.e. it is not necessarily reciprocal.</rdfs:comment>
        <rdfs:subPropertyOf rdf:resource="http://semanticbible.org/ns/2006/NTNames#knows"/>
    </owl:ObjectProperty>
    


    <!-- http://semanticbible.org/ns/2006/NTNames#ethnicity -->

    <owl:ObjectProperty rdf:about="http://semanticbible.org/ns/2006/NTNames#ethnicity">
        <rdfs:label xml:lang="en">ethnicity</rdfs:label>
        <rdfs:comment xml:lang="en">The ethnicity or, more generally, cultural heritage of a person. This can overlap with both religiousBelief (which may, however, change over time) and nativePlace (which, like ethnicity, does not change, though residency might). Whether a given property represents ethnicity or citizenship (nativePlace) can be a difficult decision, but in general, ethnic identities like &quot;Jewish&quot; or &quot;Greek&quot; take precedence. For example, we consider the Apostle Paul to have Jewish ethnicity, though he was a citizen of Tarsus, because he was raised as a Jew. Ethnicity is not specified without specific evidence, either textual or reliable tradition: for example, having a Greek name is not sufficient. </rdfs:comment>
    </owl:ObjectProperty>
    


    <!-- http://semanticbible.org/ns/2006/NTNames#ethnicityOf -->

    <owl:ObjectProperty rdf:about="http://semanticbible.org/ns/2006/NTNames#ethnicityOf">
        <rdfs:label xml:lang="en">ethnicity of</rdfs:label>
    </owl:ObjectProperty>
    


    <!-- http://semanticbible.org/ns/2006/NTNames#hasAntagonist -->

    <owl:ObjectProperty rdf:about="http://semanticbible.org/ns/2006/NTNames#hasAntagonist">
        <rdfs:label xml:lang="en">has antagonist</rdfs:label>
        <rdfs:comment xml:lang="en">inverse of antagonistOf, which is not necessarily reciprocal</rdfs:comment>
        <rdfs:subPropertyOf rdf:resource="http://semanticbible.org/ns/2006/NTNames#knows"/>
    </owl:ObjectProperty>
    


    <!-- http://semanticbible.org/ns/2006/NTNames#hasEnemy -->

    <owl:ObjectProperty rdf:about="http://semanticbible.org/ns/2006/NTNames#hasEnemy">
        <rdfs:label xml:lang="en">has enemy</rdfs:label>
        <rdfs:comment xml:lang="en">inverse of enemyOf, which is not necessarily reciprocal</rdfs:comment>
        <rdfs:subPropertyOf rdf:resource="http://semanticbible.org/ns/2006/NTNames#knows"/>
    </owl:ObjectProperty>
    


    <!-- http://semanticbible.org/ns/2006/NTNames#knows -->

    <owl:ObjectProperty rdf:about="http://semanticbible.org/ns/2006/NTNames#knows">
        <rdfs:label xml:lang="en">knows</rdfs:label>
        <rdfs:comment xml:lang="en">&quot;A person known by this person (indicating some level of reciprocated interaction between the parties)&quot;, similar to http://purl.org/vocab/relationship vocabulary, but with different domain and range. Therefore this is a symmetric relationship: if I know you, you also know me (or else we don&#39;t &quot;know&quot; each other in this sense). </rdfs:comment>
    </owl:ObjectProperty>
    


    <!-- http://semanticbible.org/ns/2006/NTNames#location -->

    <owl:ObjectProperty rdf:about="http://semanticbible.org/ns/2006/NTNames#location">
        <rdfs:label xml:lang="en">location</rdfs:label>
        <rdfs:comment xml:lang="en">The location property relates a GeographicArea to a GeographicLocation. Each GeographicArea is assumed to have only one location, and no GeographicAreas share a location. </rdfs:comment>
    </owl:ObjectProperty>
    


    <!-- http://semanticbible.org/ns/2006/NTNames#locationOf -->

    <owl:ObjectProperty rdf:about="http://semanticbible.org/ns/2006/NTNames#locationOf"/>
    


    <!-- http://semanticbible.org/ns/2006/NTNames#member -->

    <owl:ObjectProperty rdf:about="http://semanticbible.org/ns/2006/NTNames#member">
        <rdfs:label xml:lang="en">member</rdfs:label>
        <rdfs:comment xml:lang="en">Group has member Human. Inverse of memberOf. No provision for membership changes over time.</rdfs:comment>
    </owl:ObjectProperty>
    


    <!-- http://semanticbible.org/ns/2006/NTNames#memberOf -->

    <owl:ObjectProperty rdf:about="http://semanticbible.org/ns/2006/NTNames#memberOf">
        <rdfs:label xml:lang="en">member of</rdfs:label>
        <rdfs:comment xml:lang="en">Human is a memberOf a Group. Inverse of member. There are subtleties about Collections in SUMO that i&#39;m omiting here.</rdfs:comment>
    </owl:ObjectProperty>
    


    <!-- http://semanticbible.org/ns/2006/NTNames#nativePlace -->

    <owl:ObjectProperty rdf:about="http://semanticbible.org/ns/2006/NTNames#nativePlace">
        <rdfs:label xml:lang="en">native place</rdfs:label>
        <rdfs:comment xml:lang="en">Birthplace, or place in which a person grows up. Unlike residentOf, only one possible value. residentPlace is to be preferred unless the birthplace relationship is clearly identified.</rdfs:comment>
        <rdfs:subPropertyOf rdf:resource="http://semanticbible.org/ns/2006/NTNames#visitedPlace"/>
    </owl:ObjectProperty>
    


    <!-- http://semanticbible.org/ns/2006/NTNames#nativePlaceOf -->

    <owl:ObjectProperty rdf:about="http://semanticbible.org/ns/2006/NTNames#nativePlaceOf">
        <rdfs:subPropertyOf rdf:resource="http://semanticbible.org/ns/2006/NTNames#visitedPlaceOf"/>
    </owl:ObjectProperty>
    


    <!-- http://semanticbible.org/ns/2006/NTNames#parentOf -->

    <owl:ObjectProperty rdf:about="http://semanticbible.org/ns/2006/NTNames#parentOf">
        <rdfs:label xml:lang="en">parent of</rdfs:label>
        <rdfs:comment xml:lang="en">Similar to http://purl.org/vocab/relationship vocabulary, but with different domain and range.</rdfs:comment>
        <rdfs:subPropertyOf rdf:resource="http://semanticbible.org/ns/2006/NTNames#relativeOf"/>
    </owl:ObjectProperty>
    


    <!-- http://semanticbible.org/ns/2006/NTNames#politicalBelief -->

    <owl:ObjectProperty rdf:about="http://semanticbible.org/ns/2006/NTNames#politicalBelief">
        <rdfs:label xml:lang="en">political belief</rdfs:label>
        <rdfs:comment xml:lang="en">Holding to a PoliticalBelief</rdfs:comment>
    </owl:ObjectProperty>
    


    <!-- http://semanticbible.org/ns/2006/NTNames#possiblySamePersonAs -->

    <owl:ObjectProperty rdf:about="http://semanticbible.org/ns/2006/NTNames#possiblySamePersonAs">
        <rdfs:label xml:lang="en">possibly same person as</rdfs:label>
        <rdfs:comment xml:lang="en">This person may be the same as the other person, though there isn&#39;t enough evidence to definitively say so. Typically the individuals will have the same name, and some overlap of circumstances that makes it possible. </rdfs:comment>
    </owl:ObjectProperty>
    


    <!-- http://semanticbible.org/ns/2006/NTNames#relativeOf -->

    <owl:ObjectProperty rdf:about="http://semanticbible.org/ns/2006/NTNames#relativeOf">
        <rdfs:label xml:lang="en">relative of</rdfs:label>
        <rdfs:comment xml:lang="en">A person who is related by kinship to this person. No attempt is made to delineate precisely which kinship relations qualify: this is used when a description indicates two people are &quot;related&quot;. parent/child/siblingOf are subproperties of this, properly speaking. </rdfs:comment>
    </owl:ObjectProperty>
    


    <!-- http://semanticbible.org/ns/2006/NTNames#religiousBelief -->

    <owl:ObjectProperty rdf:about="http://semanticbible.org/ns/2006/NTNames#religiousBelief">
        <rdfs:label xml:lang="en">religious belief</rdfs:label>
        <rdfs:comment xml:lang="en">Having a ReligiousBelief as an attribute</rdfs:comment>
    </owl:ObjectProperty>
    


    <!-- http://semanticbible.org/ns/2006/NTNames#religiousBeliefOf -->

    <owl:ObjectProperty rdf:about="http://semanticbible.org/ns/2006/NTNames#religiousBeliefOf">
        <rdfs:label xml:lang="en">religious belief of</rdfs:label>
    </owl:ObjectProperty>
    


    <!-- http://semanticbible.org/ns/2006/NTNames#residentPlace -->

    <owl:ObjectProperty rdf:about="http://semanticbible.org/ns/2006/NTNames#residentPlace">
        <rdfs:label xml:lang="en">resident place</rdfs:label>
        <rdfs:comment xml:lang="en">The location a person or group of people resides in. Range values may change over time: no attempt is made to capture this. Transient residence of very short duration is assumed to be visited, not resident. People addressed in a letter bound for a specific destination (e.g. the epistle of Paul to the Romans) are assumed to be resident there unless there is indication to the contrary (since the timing of a letter&#39;s arrival could not be determined with high precision). </rdfs:comment>
        <rdfs:subPropertyOf rdf:resource="http://semanticbible.org/ns/2006/NTNames#visitedPlace"/>
    </owl:ObjectProperty>
    


    <!-- http://semanticbible.org/ns/2006/NTNames#residentPlaceOf -->

    <owl:ObjectProperty rdf:about="http://semanticbible.org/ns/2006/NTNames#residentPlaceOf">
        <rdfs:subPropertyOf rdf:resource="http://semanticbible.org/ns/2006/NTNames#visitedPlaceOf"/>
    </owl:ObjectProperty>
    


    <!-- http://semanticbible.org/ns/2006/NTNames#siblingOf -->

    <owl:ObjectProperty rdf:about="http://semanticbible.org/ns/2006/NTNames#siblingOf">
        <rdfs:label xml:lang="en">sibling of</rdfs:label>
        <rdfs:comment xml:lang="en">Similar to http://purl.org/vocab/relationship vocabulary, but with different domain and range.</rdfs:comment>
        <rdfs:subPropertyOf rdf:resource="http://semanticbible.org/ns/2006/NTNames#relativeOf"/>
    </owl:ObjectProperty>
    


    <!-- http://semanticbible.org/ns/2006/NTNames#spouseOf -->

    <owl:ObjectProperty rdf:about="http://semanticbible.org/ns/2006/NTNames#spouseOf">
        <rdfs:label xml:lang="en">spouse of</rdfs:label>
        <rdfs:comment xml:lang="en">Similar to http://purl.org/vocab/relationship vocabulary, but with different domain and range. Multiple spouses are all included, whether sequential (Herodias) or simultaneous (the woman at the well). </rdfs:comment>
    </owl:ObjectProperty>
    


    <!-- http://semanticbible.org/ns/2006/NTNames#subregion -->

    <owl:ObjectProperty rdf:about="http://semanticbible.org/ns/2006/NTNames#subregion">
        <rdfs:label xml:lang="en">subregion</rdfs:label>
        <rdfs:comment xml:lang="en">Inverse of subregionOf</rdfs:comment>
    </owl:ObjectProperty>
    


    <!-- http://semanticbible.org/ns/2006/NTNames#subregionOf -->

    <owl:ObjectProperty rdf:about="http://semanticbible.org/ns/2006/NTNames#subregionOf">
        <rdfs:label xml:lang="en">subregion of</rdfs:label>
        <rdfs:comment xml:lang="en">A smaller GeographicArea is a subregionOf a larger one (e.g. Jerusalem is a subregionOf Israel).</rdfs:comment>
    </owl:ObjectProperty>
    


    <!-- http://semanticbible.org/ns/2006/NTNames#visitedPlace -->

    <owl:ObjectProperty rdf:about="http://semanticbible.org/ns/2006/NTNames#visitedPlace">
        <rdfs:label xml:lang="en">visited place</rdfs:label>
        <rdfs:comment xml:lang="en">Places that a human visited. For current purposes, only instances which are explicitly mentioned in Scripture are included, not those that might be inferred (e.g. if going from from A to B implies visiting C, C would not be listed). </rdfs:comment>
    </owl:ObjectProperty>
    


    <!-- http://semanticbible.org/ns/2006/NTNames#visitedPlaceOf -->

    <owl:ObjectProperty rdf:about="http://semanticbible.org/ns/2006/NTNames#visitedPlaceOf"/>
    


    <!-- 
    ///////////////////////////////////////////////////////////////////////////////////////
    //
    // Data properties
    //
    ///////////////////////////////////////////////////////////////////////////////////////
     -->

    


    <!-- http://semanticbible.org/ns/2006/NTNames#LNID -->

    <owl:DatatypeProperty rdf:about="http://semanticbible.org/ns/2006/NTNames#LNID">
        <rdfs:label xml:lang="en">Louw-Nida identifier</rdfs:label>
        <rdfs:comment xml:lang="en">Louw-Nida identifier, keying specific Greek terms (and their English translations) to their taxonomy of semantic domains. A string like &quot;33.X&#39;.439&quot; identifies the term sumballo, which can be translated as &quot;to express differences of opinion in a forceful way&quot;. In their scheme, this has domain index 33 (Communication), with sub-domain index X&#39; (Dispute, Debate). The final integer index uniquely defines this term (but the same term may have multiple senses). The sub-domain index can be determined from the term index, but it seems helpful to include both. Note the possible values of the sub-domain index are A-Z, then A&#39;-Z&#39;, etc.</rdfs:comment>
    </owl:DatatypeProperty>
    


    <!-- http://semanticbible.org/ns/2006/NTNames#altitude -->

    <owl:DatatypeProperty rdf:about="http://semanticbible.org/ns/2006/NTNames#altitude">
        <rdfs:label xml:lang="en">altitude</rdfs:label>
        <rdfs:comment xml:lang="en">The altitude component of a GeographicLocation</rdfs:comment>
    </owl:DatatypeProperty>
    


    <!-- http://semanticbible.org/ns/2006/NTNames#description -->

    <owl:DatatypeProperty rdf:about="http://semanticbible.org/ns/2006/NTNames#description">
        <rdfs:label xml:lang="en">description</rdfs:label>
        <rdfs:comment xml:lang="en">A brief description of the salient aspects of a Human, based on their being mentioned in Scripture. This is not the way to enter dictionary-style definitions.</rdfs:comment>
    </owl:DatatypeProperty>
    


    <!-- http://semanticbible.org/ns/2006/NTNames#hasOnlyGenealogyMention -->

    <owl:DatatypeProperty rdf:about="http://semanticbible.org/ns/2006/NTNames#hasOnlyGenealogyMention">
        <rdfs:label xml:lang="en">has only genealogy mention</rdfs:label>
        <rdfs:comment xml:lang="en">The only mention of this person in the New Testament text is the genealogies of Jesus recorded in Matthew 1 and/or Luke 3. Since only limited information (their ancestry) is available about this special subset of names, this property exists to support filtering them out (or in). </rdfs:comment>
    </owl:DatatypeProperty>
    


    <!-- http://semanticbible.org/ns/2006/NTNames#latitude -->

    <owl:DatatypeProperty rdf:about="http://semanticbible.org/ns/2006/NTNames#latitude">
        <rdfs:label xml:lang="en">latitude</rdfs:label>
        <rdfs:comment xml:lang="en">The latitude component of a GeographicLocation</rdfs:comment>
    </owl:DatatypeProperty>
    


    <!-- http://semanticbible.org/ns/2006/NTNames#longitude -->

    <owl:DatatypeProperty rdf:about="http://semanticbible.org/ns/2006/NTNames#longitude">
        <rdfs:label xml:lang="en">longitude</rdfs:label>
        <rdfs:comment xml:lang="en">The longiitude component of a GeographicLocation</rdfs:comment>
    </owl:DatatypeProperty>
    


    <!-- http://semanticbible.org/ns/2006/NTNames#name_en -->

    <owl:DatatypeProperty rdf:about="http://semanticbible.org/ns/2006/NTNames#name_en">
        <rdfs:label xml:lang="en">English name</rdfs:label>
        <rdfs:comment xml:lang="en">The human language name of an Object in English. 
Since Protege (3.0 build 141) doesn&#39;t seem to support loading and saving xml:lang attributes on properties, different subproperties are used for representing names in different languages.</rdfs:comment>
    </owl:DatatypeProperty>
    


    <!-- http://semanticbible.org/ns/2006/NTNames#name_grc -->

    <owl:DatatypeProperty rdf:about="http://semanticbible.org/ns/2006/NTNames#name_grc">
        <rdfs:label xml:lang="en">Greek name</rdfs:label>
        <rdfs:comment xml:lang="en">The human language name of an Object in Koine (not Modern) Greek, in the standard dictionary form (nominative case). 
 Since Protege (3.0 build 141) doesn&#39;t seem to support loading and saving xml:lang attributes on properties, different subproperties are used for representing names in different languages. &quot;grc&quot; is the three-letter ISO-639-2 standard designator for Koine Greek.</rdfs:comment>
    </owl:DatatypeProperty>
    


    <!-- http://semanticbible.org/ns/2006/NTNames#occupation -->

    <owl:DatatypeProperty rdf:about="http://semanticbible.org/ns/2006/NTNames#occupation">
        <rdfs:label xml:lang="en">occupation</rdfs:label>
    </owl:DatatypeProperty>
    


    <!-- 
    ///////////////////////////////////////////////////////////////////////////////////////
    //
    // Classes
    //
    ///////////////////////////////////////////////////////////////////////////////////////
     -->

    


    <!-- http://semanticbible.org/ns/2006/NTNames#Agent -->

    <owl:Class rdf:about="http://semanticbible.org/ns/2006/NTNames#Agent">
        <rdfs:label xml:lang="en">Agent</rdfs:label>
        <rdfs:comment xml:lang="en">Comparable to http://reliant.teknowledge.com/DAML/SUMO.owl#Agent
SUO 1.55: July 14, 2003
Something or someone that can act on its own and 
produce changes in the world.</rdfs:comment>
    </owl:Class>
    


    <!-- http://semanticbible.org/ns/2006/NTNames#Angel -->

    <owl:Class rdf:about="http://semanticbible.org/ns/2006/NTNames#Angel">
        <rdfs:label xml:lang="en">Angel</rdfs:label>
        <owl:disjointWith rdf:resource="http://semanticbible.org/ns/2006/NTNames#Human"/>
        <owl:disjointWith rdf:resource="http://semanticbible.org/ns/2006/NTNames#SupernaturalBeing"/>
        <rdfs:comment xml:lang="en">Supernatural beings that work to support God&#39;s purposes as his agents.</rdfs:comment>
    </owl:Class>
    


    <!-- http://semanticbible.org/ns/2006/NTNames#BeliefGroup -->

    <owl:Class rdf:about="http://semanticbible.org/ns/2006/NTNames#BeliefGroup">
        <rdfs:label xml:lang="en">Belief Group</rdfs:label>
        <rdfs:comment xml:lang="en">Comparable to http://reliant.teknowledge.com/DAML/SUMO.owl#BeliefGroup
SUO 1.55: July 14, 2003
A &amp;%Group whose &amp;%members share a belief or
set of beliefs.
For NTN, this covers groups defined by a particular set of beliefs (orthodox or heretical) which are informal, rather than formal, in membership and activity.</rdfs:comment>
    </owl:Class>
    


    <!-- http://semanticbible.org/ns/2006/NTNames#BeliefSystem -->

    <owl:Class rdf:about="http://semanticbible.org/ns/2006/NTNames#BeliefSystem">
        <rdfs:label xml:lang="en">Belief system</rdfs:label>
        <rdfs:comment xml:lang="en">An organization of propositions into an identifiable belief system. A person who holds to a belief system can be considered a member of the corresponding BeliefGroup.

The notion of Proposition here is derived from http://reliant.teknowledge.com/DAML/SUMO.owl#Proposition.</rdfs:comment>
    </owl:Class>
    


    <!-- http://semanticbible.org/ns/2006/NTNames#Character -->

    <owl:Class rdf:about="http://semanticbible.org/ns/2006/NTNames#Character">
        <rdfs:label xml:lang="en">Character</rdfs:label>
        <rdfs:comment xml:lang="en">Broadly the same as http://reliant.teknowledge.com/DAML/SUMO.owl#Character
SUO 1.55: July 14, 2003
An element of an alphabet, a set of numerals, etc.
Note that a &amp;%Character may or may not be part of a &amp;%Language.  &amp;%Character
is a subclass of &amp;%SymbolicString, because every instance of &amp;%Character is
an alphanumeric sequence consisting of a single element.</rdfs:comment>
    </owl:Class>
    


    <!-- http://semanticbible.org/ns/2006/NTNames#CitizenshipAttribute -->

    <owl:Class rdf:about="http://semanticbible.org/ns/2006/NTNames#CitizenshipAttribute">
        <rdfs:label rdf:datatype="http://www.w3.org/2001/XMLSchema#string">Citizenship attribute</rdfs:label>
        <rdfs:comment xml:lang="en">Belonging to the citizenry of a country (e.g. Roman). There may be parallel ethnicity attributes (Roman being the primary example) which are not easily distinguished. In the case of Roman, while all ethnic Romans (in the general sense, though not necessarily legal sense [e.g. slaves]) are Roman citizens, there are other Roman citizens (e.g. Paul) who have different ethnicity. </rdfs:comment>
    </owl:Class>
    


    <!-- http://semanticbible.org/ns/2006/NTNames#City -->

    <owl:Class rdf:about="http://semanticbible.org/ns/2006/NTNames#City">
        <rdfs:label xml:lang="en">City</rdfs:label>
        <owl:disjointWith rdf:resource="http://semanticbible.org/ns/2006/NTNames#Nation"/>
        <owl:disjointWith rdf:resource="http://semanticbible.org/ns/2006/NTNames#StateOrProvince"/>
        <rdfs:comment xml:lang="en">Based on SUMO, http://reliant.teknowledge.com/DAML/SUMO.owl#City
SUO 1.55: July 14, 2003
A &amp;%LandArea of relatively small size, inhabited
by a community of people, and having some sort of political structure.
Note that this class includes both large cities and small settlements
like towns, villages, hamlets, etc.</rdfs:comment>
    </owl:Class>
    


    <!-- http://semanticbible.org/ns/2006/NTNames#CognitiveAgent -->

    <owl:Class rdf:about="http://semanticbible.org/ns/2006/NTNames#CognitiveAgent">
        <rdfs:label xml:lang="en">Cognitive Agent</rdfs:label>
        <owl:disjointWith>
            <owl:Restriction>
                <owl:onProperty rdf:resource="http://semanticbible.org/ns/2006/NTNames#religiousBelief"/>
                <owl:someValuesFrom rdf:resource="http://www.w3.org/2002/07/owl#Thing"/>
            </owl:Restriction>
        </owl:disjointWith>
        <rdfs:comment xml:lang="en">Comparable to http://reliant.teknowledge.com/DAML/SUMO.owl#CognitiveAgent
SUO 1.55: July 14, 2003
A &amp;%SentientAgent with responsibilities 
and the ability to reason, deliberate, make plans, etc.  This is 
essentially the legal/ethical notion of a person.  Note that, although 
&amp;%Human is a subclass of &amp;%CognitiveAgent, there may be instances of 
&amp;%CognitiveAgent which are not also instances of &amp;%Human.  For example, 
chimpanzees, gorillas, dolphins, whales, and some extraterrestrials 
(if they exist) may be &amp;%CognitiveAgents.</rdfs:comment>
    </owl:Class>
    


    <!-- http://semanticbible.org/ns/2006/NTNames#ContentBearingObject -->

    <owl:Class rdf:about="http://semanticbible.org/ns/2006/NTNames#ContentBearingObject">
        <rdfs:label xml:lang="en">Content Bearing Object</rdfs:label>
        <rdfs:comment xml:lang="en">Broadly the same as http://reliant.teknowledge.com/DAML/SUMO.owl#ContentBearingObject
SUO 1.55: July 14, 2003
Any &amp;%SelfConnectedObject that expresses 
information.</rdfs:comment>
    </owl:Class>
    


    <!-- http://semanticbible.org/ns/2006/NTNames#EthnicGroup -->

    <owl:Class rdf:about="http://semanticbible.org/ns/2006/NTNames#EthnicGroup">
        <rdfs:label xml:lang="en">Ethnic Group</rdfs:label>
        <owl:disjointWith rdf:resource="http://semanticbible.org/ns/2006/NTNames#Organization"/>
        <owl:disjointWith rdf:resource="http://semanticbible.org/ns/2006/NTNames#PoliticalOrganization"/>
        <owl:disjointWith rdf:resource="http://semanticbible.org/ns/2006/NTNames#ResidenceGroup"/>
        <owl:disjointWith rdf:resource="http://semanticbible.org/ns/2006/NTNames#Tribe"/>
        <rdfs:comment xml:lang="en">Comparable to http://reliant.teknowledge.com/DAML/SUMO.owl#EthnicGroup
SUO 1.55: July 14, 2003
A &amp;%Group whose &amp;%members originate from
the same &amp;%GeographicArea or share the same &amp;%Language and/or cultural
practices.</rdfs:comment>
    </owl:Class>
    


    <!-- http://semanticbible.org/ns/2006/NTNames#EthnicityAttribute -->

    <owl:Class rdf:about="http://semanticbible.org/ns/2006/NTNames#EthnicityAttribute">
        <rdfs:label xml:lang="en">Ethnicity attribute</rdfs:label>
        <owl:disjointWith>
            <owl:Restriction>
                <owl:onProperty rdf:resource="http://semanticbible.org/ns/2006/NTNames#ethnicityOf"/>
                <owl:someValuesFrom rdf:resource="http://www.w3.org/2002/07/owl#Thing"/>
            </owl:Restriction>
        </owl:disjointWith>
        <rdfs:comment xml:lang="en">The attribute of belonging to a particular ethnic group, or originating from a GeographicArea. Unlike Residency, which can change, Ethnicity is considered permanent.</rdfs:comment>
    </owl:Class>
    


    <!-- http://semanticbible.org/ns/2006/NTNames#EvilSupernaturalBeing -->

    <owl:Class rdf:about="http://semanticbible.org/ns/2006/NTNames#EvilSupernaturalBeing">
        <rdfs:label xml:lang="en">Evil Supernatural Being</rdfs:label>
        <rdfs:comment xml:lang="en">Class of malevolent supernatural beings, whose instances include Satan and demons. </rdfs:comment>
    </owl:Class>
    


    <!-- http://semanticbible.org/ns/2006/NTNames#FixedHoliday -->

    <owl:Class rdf:about="http://semanticbible.org/ns/2006/NTNames#FixedHoliday">
        <rdfs:label xml:lang="en">Fixed holiday</rdfs:label>
        <rdfs:comment xml:lang="en">Would be a subclass of http://reliant.teknowledge.com/DAML/SUMO.owl#TimeInterval, but is specified within MILO.
MILO: &amp;%FixedHoliday is the class of &amp;%Holidays 
whose observance is fixed to recurrences of the calendar day that the 
holiday commemorates.</rdfs:comment>
    </owl:Class>
    


    <!-- http://semanticbible.org/ns/2006/NTNames#FreshWaterArea -->

    <owl:Class rdf:about="http://semanticbible.org/ns/2006/NTNames#FreshWaterArea">
        <rdfs:label xml:lang="en">Fresh Water Area</rdfs:label>
        <rdfs:comment xml:lang="en">Based on SUMO, http://reliant.teknowledge.com/DAML/SUMO.owl#FreshWaterArea

SUO 1.55: July 14, 2003
A &amp;%WaterArea whose &amp;%Water is not saline,
e.g. most rivers and lakes.</rdfs:comment>
    </owl:Class>
    


    <!-- http://semanticbible.org/ns/2006/NTNames#GeographicArea -->

    <owl:Class rdf:about="http://semanticbible.org/ns/2006/NTNames#GeographicArea">
        <rdfs:label xml:lang="en">Geographic Area</rdfs:label>
        <rdfs:comment xml:lang="en">Based on SUMO, http://reliant.teknowledge.com/DAML/SUMO.owl#GeographicArea
SUO 1.55: July 14, 2003
A geographic location, generally having 
definite boundaries.  Note that this differs from its immediate superclass 
&amp;%Region in that a &amp;%GeographicArea is a three-dimensional &amp;%Region of the 
earth.  Accordingly, all astronomical objects other than earth and all 
one-dimensional and two-dimensional &amp;%Regions are not classed under 
&amp;%GeographicArea.</rdfs:comment>
    </owl:Class>
    


    <!-- http://semanticbible.org/ns/2006/NTNames#GeographicLocation -->

    <owl:Class rdf:about="http://semanticbible.org/ns/2006/NTNames#GeographicLocation">
        <rdfs:label xml:lang="en">Geographic Location</rdfs:label>
        <rdfs:comment rdf:datatype="http://www.w3.org/2001/XMLSchema#string">A collection of properties describing geographic location. </rdfs:comment>
    </owl:Class>
    


    <!-- http://semanticbible.org/ns/2006/NTNames#GeopoliticalArea -->

    <owl:Class rdf:about="http://semanticbible.org/ns/2006/NTNames#GeopoliticalArea">
        <rdfs:label xml:lang="en">Geopolitical Area</rdfs:label>
        <owl:disjointWith rdf:resource="http://semanticbible.org/ns/2006/NTNames#Island"/>
        <rdfs:comment xml:lang="en">Based on SUMO, http://reliant.teknowledge.com/DAML/SUMO.owl#GeopoliticalArea
SUO 1.55: July 14, 2003
Any &amp;%GeographicArea which is associated 
with some sort of political structure.  This class includes &amp;%Lands, 
&amp;%Cities, districts of cities, counties, etc.  Note that the identity 
of a &amp;%GeopoliticalArea may remain constant after a change in borders.</rdfs:comment>
    </owl:Class>
    


    <!-- http://semanticbible.org/ns/2006/NTNames#God -->

    <owl:Class rdf:about="http://semanticbible.org/ns/2006/NTNames#God">
        <rdfs:label xml:lang="en">God</rdfs:label>
        <rdfs:comment xml:lang="en">Self-documenting</rdfs:comment>
    </owl:Class>
    


    <!-- http://semanticbible.org/ns/2006/NTNames#Group -->

    <owl:Class rdf:about="http://semanticbible.org/ns/2006/NTNames#Group">
        <rdfs:label xml:lang="en">Group</rdfs:label>
        <owl:disjointWith>
            <owl:Restriction>
                <owl:onProperty rdf:resource="http://semanticbible.org/ns/2006/NTNames#religiousBelief"/>
                <owl:someValuesFrom rdf:resource="http://www.w3.org/2002/07/owl#Thing"/>
            </owl:Restriction>
        </owl:disjointWith>
        <rdfs:comment xml:lang="en">Comparable to http://reliant.teknowledge.com/DAML/SUMO.owl#Group
SUO 1.55: July 14, 2003
A &amp;%Collection of &amp;%Agents, e.g. a flock
of sheep, a herd of goats, or the local Boy Scout troop.</rdfs:comment>
    </owl:Class>
    


    <!-- http://semanticbible.org/ns/2006/NTNames#GroupOfPeople -->

    <owl:Class rdf:about="http://semanticbible.org/ns/2006/NTNames#GroupOfPeople">
        <rdfs:label xml:lang="en">Group of People</rdfs:label>
        <owl:disjointWith>
            <owl:Restriction>
                <owl:onProperty rdf:resource="http://semanticbible.org/ns/2006/NTNames#religiousBelief"/>
                <owl:someValuesFrom rdf:resource="http://www.w3.org/2002/07/owl#Thing"/>
            </owl:Restriction>
        </owl:disjointWith>
        <rdfs:comment xml:lang="en">Comparable to http://reliant.teknowledge.com/DAML/SUMO.owl#GroupOfPeople
SUO 1.55: July 14, 2003
Any &amp;%Group whose &amp;%members are
exclusively &amp;%Humans.</rdfs:comment>
    </owl:Class>
    


    <!-- http://semanticbible.org/ns/2006/NTNames#Human -->

    <owl:Class rdf:about="http://semanticbible.org/ns/2006/NTNames#Human">
        <rdfs:label xml:lang="en">Human</rdfs:label>
        <owl:disjointWith rdf:resource="http://semanticbible.org/ns/2006/NTNames#SupernaturalBeing"/>
        <rdfs:comment xml:lang="en">Comparable to http://reliant.teknowledge.com/DAML/SUMO.owl#Human
SUO 1.55: July 14, 2003
Modern man, the only remaining species of the Homo genus.</rdfs:comment>
    </owl:Class>
    


    <!-- http://semanticbible.org/ns/2006/NTNames#HumanAttribute -->

    <owl:Class rdf:about="http://semanticbible.org/ns/2006/NTNames#HumanAttribute">
        <rdfs:label xml:lang="en">Human attribute</rdfs:label>
        <rdfs:comment xml:lang="en">Attributes of people, overlapping with the class hierarchy under suo:Group: this is unsatisfactory.</rdfs:comment>
    </owl:Class>
    


    <!-- http://semanticbible.org/ns/2006/NTNames#Island -->

    <owl:Class rdf:about="http://semanticbible.org/ns/2006/NTNames#Island">
        <rdfs:label xml:lang="en">Island</rdfs:label>
        <rdfs:comment xml:lang="en">Based on SUMO, http://reliant.teknowledge.com/DAML/SUMO.owl#Island
SUO 1.55: July 14, 2003
A &amp;%LandArea that is completely surrounded by a &amp;%WaterArea.</rdfs:comment>
    </owl:Class>
    


    <!-- http://semanticbible.org/ns/2006/NTNames#LandArea -->

    <owl:Class rdf:about="http://semanticbible.org/ns/2006/NTNames#LandArea">
        <rdfs:label xml:lang="en">Land Area</rdfs:label>
        <owl:disjointWith>
            <owl:Restriction>
                <owl:onProperty rdf:resource="http://semanticbible.org/ns/2006/NTNames#location"/>
                <owl:someValuesFrom rdf:resource="http://www.w3.org/2002/07/owl#Thing"/>
            </owl:Restriction>
        </owl:disjointWith>
        <owl:disjointWith>
            <owl:Restriction>
                <owl:onProperty rdf:resource="http://semanticbible.org/ns/2006/NTNames#subregionOf"/>
                <owl:someValuesFrom rdf:resource="http://www.w3.org/2002/07/owl#Thing"/>
            </owl:Restriction>
        </owl:disjointWith>
        <owl:disjointWith>
            <owl:Restriction>
                <owl:onProperty rdf:resource="http://semanticbible.org/ns/2006/NTNames#subregion"/>
                <owl:someValuesFrom rdf:resource="http://www.w3.org/2002/07/owl#Thing"/>
            </owl:Restriction>
        </owl:disjointWith>
        <rdfs:comment xml:lang="en">Based on SUMO, http://reliant.teknowledge.com/DAML/SUMO.owl#LandArea
SUO 1.55: July 14, 2003
An area which is predominantly solid ground,
e.g. a &amp;%Nation, a mountain, a desert, etc.  Note that a &amp;%LandArea may
contain some relatively small &amp;%WaterAreas.  For example, Australia is
a &amp;%LandArea even though it contains various rivers and lakes.</rdfs:comment>
    </owl:Class>
    


    <!-- http://semanticbible.org/ns/2006/NTNames#Man -->

    <owl:Class rdf:about="http://semanticbible.org/ns/2006/NTNames#Man">
        <rdfs:label xml:lang="en">Man</rdfs:label>
        <owl:disjointWith rdf:resource="http://semanticbible.org/ns/2006/NTNames#Woman"/>
        <owl:disjointWith>
            <owl:Restriction>
                <owl:onProperty rdf:resource="http://semanticbible.org/ns/2006/NTNames#ethnicity"/>
                <owl:someValuesFrom rdf:resource="http://www.w3.org/2002/07/owl#Thing"/>
            </owl:Restriction>
        </owl:disjointWith>
        <rdfs:comment xml:lang="en">SUO 1.55: July 14, 2003
The class of &amp;%Male &amp;%Humans.</rdfs:comment>
    </owl:Class>
    


    <!-- http://semanticbible.org/ns/2006/NTNames#Mountain -->

    <owl:Class rdf:about="http://semanticbible.org/ns/2006/NTNames#Mountain">
        <rdfs:label xml:lang="en">Mountain</rdfs:label>
        <rdfs:comment xml:lang="en">Wordnet: &quot;a land mass that projects well above its surroundings; higher than a hill. &quot;
Used here for things referred to as &quot;mount&quot;, even though some of these might seem
like hills to well-traveled observers. </rdfs:comment>
    </owl:Class>
    


    <!-- http://semanticbible.org/ns/2006/NTNames#Nation -->

    <owl:Class rdf:about="http://semanticbible.org/ns/2006/NTNames#Nation">
        <rdfs:label xml:lang="en">Nation</rdfs:label>
        <owl:disjointWith rdf:resource="http://semanticbible.org/ns/2006/NTNames#StateOrProvince"/>
        <rdfs:comment xml:lang="en">Based on SUMO, http://reliant.teknowledge.com/DAML/SUMO.owl#Nation
SUO 1.55: July 14, 2003
The broadest &amp;%GeopoliticalArea, i.e. &amp;%Nations are
&amp;%GeopoliticalAreas that are not part of any other overarching and
comprehensive governance structure (excepting commonwealths and other sorts
of loose international organizations).
Note that modern nations referred to in the New Testament (Spain,
Italy, Libya) are typically not instances of Nation, but rather
of Region (if the borders are indefinite) or of LandArea.</rdfs:comment>
    </owl:Class>
    


    <!-- http://semanticbible.org/ns/2006/NTNames#NaturalLanguage -->

    <owl:Class rdf:about="http://semanticbible.org/ns/2006/NTNames#NaturalLanguage">
        <rdfs:label xml:lang="en">Natural Language</rdfs:label>
        <rdfs:comment xml:lang="en">Broadly the same as http://reliant.teknowledge.com/DAML/SUMO.owl#NaturalLanguage
SUO 1.55: July 14, 2003
The &amp;%subclass of &amp;%HumanLanguages which
are not designed and which evolve from generation to generation.  This
&amp;%Class includes all of the national languages, e.g. English, Spanish,
Japanese, etc.  Note that this class includes dialects of natural
languages.</rdfs:comment>
    </owl:Class>
    


    <!-- http://semanticbible.org/ns/2006/NTNames#Object -->

    <owl:Class rdf:about="http://semanticbible.org/ns/2006/NTNames#Object">
        <rdfs:label xml:lang="en">Object</rdfs:label>
        <rdfs:comment xml:lang="en">Following http://reliant.teknowledge.com/DAML/SUMO.owl#Object, this &quot;Corresponds roughly to the class of ordinary 
objects.  Examples include normal physical objects, geographical regions, 
and locations of &amp;%Processes, the complement of &amp;%Objects in the &amp;%Physical class. &quot;</rdfs:comment>
    </owl:Class>
    


    <!-- http://semanticbible.org/ns/2006/NTNames#Organization -->

    <owl:Class rdf:about="http://semanticbible.org/ns/2006/NTNames#Organization">
        <rdfs:label xml:lang="en">Organization</rdfs:label>
        <owl:disjointWith rdf:resource="http://semanticbible.org/ns/2006/NTNames#PoliticalOrganization"/>
        <owl:disjointWith rdf:resource="http://semanticbible.org/ns/2006/NTNames#ResidenceGroup"/>
        <owl:disjointWith rdf:resource="http://semanticbible.org/ns/2006/NTNames#Tribe"/>
        <rdfs:comment xml:lang="en">Comparable to http://reliant.teknowledge.com/DAML/SUMO.owl#Organization
SUO 1.55: July 14, 2003
An &amp;%Organization is a corporate or similar institution. The &amp;%members of an &amp;%Organization typically have a common purpose or function. Note that this class also covers divisions, departments, etc. of organizations.  For example, both the Shell Corporation and the accounting department at Shell would both be instances of &amp;%Organization.  Note too that the existence of an &amp;%Organization is dependent on the existence of at least one &amp;%member (since &amp;%Organization is a subclass of &amp;%Collection).  Accordingly, in cases of purely legal organizations, a fictitious &amp;%member 
should be assumed.</rdfs:comment>
    </owl:Class>
    


    <!-- http://semanticbible.org/ns/2006/NTNames#PoliticalAttribute -->

    <owl:Class rdf:about="http://semanticbible.org/ns/2006/NTNames#PoliticalAttribute">
        <rdfs:label xml:lang="en">Political attribute</rdfs:label>
        <rdfs:comment xml:lang="en">The attribute of ascribing to a PoliticalBeliefSystem, or belonging to a political party or system.</rdfs:comment>
    </owl:Class>
    


    <!-- http://semanticbible.org/ns/2006/NTNames#PoliticalBeliefSystem -->

    <owl:Class rdf:about="http://semanticbible.org/ns/2006/NTNames#PoliticalBeliefSystem">
        <rdfs:label xml:lang="en">Political belief system</rdfs:label>
        <owl:disjointWith rdf:resource="http://semanticbible.org/ns/2006/NTNames#ReligiousBeliefSystem"/>
    </owl:Class>
    


    <!-- http://semanticbible.org/ns/2006/NTNames#PoliticalOrganization -->

    <owl:Class rdf:about="http://semanticbible.org/ns/2006/NTNames#PoliticalOrganization">
        <rdfs:label xml:lang="en">Political Organization</rdfs:label>
        <owl:disjointWith rdf:resource="http://semanticbible.org/ns/2006/NTNames#ResidenceGroup"/>
        <owl:disjointWith rdf:resource="http://semanticbible.org/ns/2006/NTNames#Tribe"/>
        <rdfs:comment xml:lang="en">Comparable to http://reliant.teknowledge.com/DAML/SUMO.owl#PoliticalOrganization
SUO 1.55: July 14, 2003
An &amp;%Organization that is a &amp;%Government,
a &amp;%subOrganization of a &amp;%Government, or an &amp;%Organization that is attempting
to bring about some sort of political change.</rdfs:comment>
    </owl:Class>
    


    <!-- http://semanticbible.org/ns/2006/NTNames#Region -->

    <owl:Class rdf:about="http://semanticbible.org/ns/2006/NTNames#Region">
        <rdfs:label xml:lang="en">Region</rdfs:label>
        <rdfs:comment xml:lang="en">Comparable to http://reliant.teknowledge.com/DAML/SUMO.owl#Region: &quot;A topographic location.  Regions encompass surfaces of Objects, imaginary places, and GeographicAreas. &quot;</rdfs:comment>
    </owl:Class>
    


    <!-- http://semanticbible.org/ns/2006/NTNames#ReligiousBelief -->

    <owl:Class rdf:about="http://semanticbible.org/ns/2006/NTNames#ReligiousBelief">
        <rdfs:label xml:lang="en">Religious belief</rdfs:label>
        <rdfs:comment xml:lang="en">The attribute of ascribing to a ReligiousBeliefSystem (which includes philosophies).</rdfs:comment>
    </owl:Class>
    


    <!-- http://semanticbible.org/ns/2006/NTNames#ReligiousBeliefSystem -->

    <owl:Class rdf:about="http://semanticbible.org/ns/2006/NTNames#ReligiousBeliefSystem">
        <rdfs:label xml:lang="en">Religious belief system</rdfs:label>
        <rdfs:comment xml:lang="en">A system of religious beliefs, or a philosophy.</rdfs:comment>
    </owl:Class>
    


    <!-- http://semanticbible.org/ns/2006/NTNames#ReligiousOrganization -->

    <owl:Class rdf:about="http://semanticbible.org/ns/2006/NTNames#ReligiousOrganization">
        <rdfs:label xml:lang="en">Religious Organization</rdfs:label>
        <rdfs:comment xml:lang="en">Comparable to http://reliant.teknowledge.com/DAML/SUMO.owl#ReligiousOrganization
SUO 1.55: July 14, 2003
An &amp;%Organization whose members
share a set of religious beliefs.</rdfs:comment>
    </owl:Class>
    


    <!-- http://semanticbible.org/ns/2006/NTNames#ResidenceGroup -->

    <owl:Class rdf:about="http://semanticbible.org/ns/2006/NTNames#ResidenceGroup">
        <rdfs:label xml:lang="en">Residence Group</rdfs:label>
        <owl:disjointWith rdf:resource="http://semanticbible.org/ns/2006/NTNames#Tribe"/>
        <rdfs:comment xml:lang="en">A group identified by common residence in a City or StateOrProvince. At the level of Nation, this should generally be EthnicGroup. Unlike EthnicGroup, they need not have cultural or ethnic features in common.</rdfs:comment>
    </owl:Class>
    


    <!-- http://semanticbible.org/ns/2006/NTNames#ResidencyAttribute -->

    <owl:Class rdf:about="http://semanticbible.org/ns/2006/NTNames#ResidencyAttribute">
        <rdfs:label xml:lang="en">Residency attribute</rdfs:label>
        <rdfs:comment xml:lang="en">The attribute of living in a particular City or Province. Unlike Ethnicity, which is permanent, Residency can change.</rdfs:comment>
    </owl:Class>
    


    <!-- http://semanticbible.org/ns/2006/NTNames#SaltWaterArea -->

    <owl:Class rdf:about="http://semanticbible.org/ns/2006/NTNames#SaltWaterArea">
        <rdfs:label xml:lang="en">Salt Water Area</rdfs:label>
        <rdfs:comment xml:lang="en">Based on SUMO, http://reliant.teknowledge.com/DAML/SUMO.owl#SaltWaterArea
SUO 1.55: July 14, 2003
A &amp;%WaterArea whose &amp;%Water is saline, e.g.
oceans and seas.</rdfs:comment>
    </owl:Class>
    


    <!-- http://semanticbible.org/ns/2006/NTNames#Series -->

    <owl:Class rdf:about="http://semanticbible.org/ns/2006/NTNames#Series">
        <rdfs:label xml:lang="en">Series</rdfs:label>
        <rdfs:comment xml:lang="en">Broadly the same as http://reliant.teknowledge.com/DAML/SUMO.owl#Series
SUO 1.55: July 14, 2003
A &amp;%Text consisting of multiple self-contained units.  
Some examples are an encyclopedia containing a couple dozen volumes, a television 
series made up of many episodes, a film serial, etc.</rdfs:comment>
    </owl:Class>
    


    <!-- http://semanticbible.org/ns/2006/NTNames#SonOfGod -->

    <owl:Class rdf:about="http://semanticbible.org/ns/2006/NTNames#SonOfGod">
        <rdfs:label xml:lang="en">Son of God</rdfs:label>
        <rdfs:comment xml:lang="en">Both Human and God</rdfs:comment>
    </owl:Class>
    


    <!-- http://semanticbible.org/ns/2006/NTNames#StateOrProvince -->

    <owl:Class rdf:about="http://semanticbible.org/ns/2006/NTNames#StateOrProvince">
        <rdfs:label xml:lang="en">State or Province</rdfs:label>
        <rdfs:comment xml:lang="en">Based on SUMO, http://reliant.teknowledge.com/DAML/SUMO.owl#StateOrProvince
SUO 1.55: July 14, 2003
Administrative subdivisions of a
&amp;%Nation that are broader than any other political subdivisions that
may exist.  This &amp;%Class includes the states of the United States, as
well as the provinces of Canada and European countries.
Here it covers both provinces and districts.</rdfs:comment>
    </owl:Class>
    


    <!-- http://semanticbible.org/ns/2006/NTNames#SupernaturalBeing -->

    <owl:Class rdf:about="http://semanticbible.org/ns/2006/NTNames#SupernaturalBeing">
        <rdfs:label xml:lang="en">Supernatural Being</rdfs:label>
        <rdfs:comment xml:lang="en">A CognitiveAgent whose effects are not limited to the physical world. This includes the Lord Almighty, as well as supposed or imaginary deities.</rdfs:comment>
    </owl:Class>
    


    <!-- http://semanticbible.org/ns/2006/NTNames#SupernaturalRegion -->

    <owl:Class rdf:about="http://semanticbible.org/ns/2006/NTNames#SupernaturalRegion">
        <rdfs:comment rdf:datatype="http://www.w3.org/2001/XMLSchema#string">Those regions that are outside normal human existence. </rdfs:comment>
    </owl:Class>
    


    <!-- http://semanticbible.org/ns/2006/NTNames#Tribe -->

    <owl:Class rdf:about="http://semanticbible.org/ns/2006/NTNames#Tribe">
        <rdfs:label xml:lang="en">Tribe</rdfs:label>
        <rdfs:comment xml:lang="en">Subclass for the Twelve Tribes of Israel</rdfs:comment>
    </owl:Class>
    


    <!-- http://semanticbible.org/ns/2006/NTNames#WaterArea -->

    <owl:Class rdf:about="http://semanticbible.org/ns/2006/NTNames#WaterArea">
        <rdfs:label xml:lang="en">Water Area</rdfs:label>
        <rdfs:comment xml:lang="en">Based on SUMO, http://reliant.teknowledge.com/DAML/SUMO.owl#WaterArea
SUO 1.55: July 14, 2003
A body which is made up predominantly of water,
e.g. rivers, lakes, oceans, etc.</rdfs:comment>
    </owl:Class>
    


    <!-- http://semanticbible.org/ns/2006/NTNames#Woman -->

    <owl:Class rdf:about="http://semanticbible.org/ns/2006/NTNames#Woman">
        <rdfs:label xml:lang="en">Woman</rdfs:label>
        <owl:disjointWith>
            <owl:Restriction>
                <owl:onProperty rdf:resource="http://semanticbible.org/ns/2006/NTNames#ethnicity"/>
                <owl:someValuesFrom rdf:resource="http://www.w3.org/2002/07/owl#Thing"/>
            </owl:Restriction>
        </owl:disjointWith>
        <rdfs:comment xml:lang="en">SUO 1.55: July 14, 2003
The class of &amp;%Female &amp;%Humans.</rdfs:comment>
    </owl:Class>
    


    <!-- 
    ///////////////////////////////////////////////////////////////////////////////////////
    //
    // Individuals
    //
    ///////////////////////////////////////////////////////////////////////////////////////
     -->

    


    <!-- http://semanticbible.org/ns/2006/NTNames#Aaron -->

    <owl:NamedIndividual rdf:about="http://semanticbible.org/ns/2006/NTNames#Aaron">
        <rdfs:label xml:lang="en">Aaron</rdfs:label>
        <ethnicity rdf:resource="http://semanticbible.org/ns/2006/NTNames#Jewish"/>
    </owl:NamedIndividual>
    


    <!-- http://semanticbible.org/ns/2006/NTNames#Abel -->

    <owl:NamedIndividual rdf:about="http://semanticbible.org/ns/2006/NTNames#Abel">
        <rdfs:label xml:lang="en">Abel</rdfs:label>
        <childOf rdf:resource="http://semanticbible.org/ns/2006/NTNames#Eve"/>
    </owl:NamedIndividual>
    


    <!-- http://semanticbible.org/ns/2006/NTNames#Abiathar -->

    <owl:NamedIndividual rdf:about="http://semanticbible.org/ns/2006/NTNames#Abiathar">
        <rdfs:label xml:lang="en">Abiathar</rdfs:label>
        <occupation rdf:datatype="http://www.w3.org/2001/XMLSchema#string">high priest</occupation>
    </owl:NamedIndividual>
    


    <!-- http://semanticbible.org/ns/2006/NTNames#AbijahSonOfRehoboam -->

    <owl:NamedIndividual rdf:about="http://semanticbible.org/ns/2006/NTNames#AbijahSonOfRehoboam">
        <rdfs:label xml:lang="en">Abijah</rdfs:label>
        <hasOnlyGenealogyMention rdf:datatype="http://www.w3.org/2001/XMLSchema#boolean">true</hasOnlyGenealogyMention>
        <rdfs:comment xml:lang="en">His occupation as king comes from Old Testament sources, 2Chr.12-13.</rdfs:comment>
    </owl:NamedIndividual>
    


    <!-- http://semanticbible.org/ns/2006/NTNames#AbijahthePriest -->

    <owl:NamedIndividual rdf:about="http://semanticbible.org/ns/2006/NTNames#AbijahthePriest">
        <rdfs:label xml:lang="en">Abijah</rdfs:label>
        <rdfs:comment xml:lang="en">Zacharias, father of John the Baptist, was a descendant of Abijah.</rdfs:comment>
    </owl:NamedIndividual>
    


    <!-- http://semanticbible.org/ns/2006/NTNames#Abilene -->

    <owl:NamedIndividual rdf:about="http://semanticbible.org/ns/2006/NTNames#Abilene">
        <rdfs:label xml:lang="en">Abilene</rdfs:label>
    </owl:NamedIndividual>
    


    <!-- http://semanticbible.org/ns/2006/NTNames#Abiud -->

    <owl:NamedIndividual rdf:about="http://semanticbible.org/ns/2006/NTNames#Abiud">
        <rdfs:label xml:lang="en">Abiud</rdfs:label>
    </owl:NamedIndividual>
    


    <!-- http://semanticbible.org/ns/2006/NTNames#Abraham -->

    <owl:NamedIndividual rdf:about="http://semanticbible.org/ns/2006/NTNames#Abraham">
        <rdfs:label xml:lang="en">Abraham</rdfs:label>
        <rdfs:label xml:lang="en">Abram</rdfs:label>
    </owl:NamedIndividual>
    


    <!-- http://semanticbible.org/ns/2006/NTNames#Achaia -->

    <owl:NamedIndividual rdf:about="http://semanticbible.org/ns/2006/NTNames#Achaia">
        <rdfs:label xml:lang="en">Achaia</rdfs:label>
    </owl:NamedIndividual>
    


    <!-- http://semanticbible.org/ns/2006/NTNames#Achaicus -->

    <owl:NamedIndividual rdf:about="http://semanticbible.org/ns/2006/NTNames#Achaicus">
        <rdfs:label xml:lang="en">Achaicus</rdfs:label>
        <rdfs:comment rdf:datatype="http://www.w3.org/2001/XMLSchema#string">His residence in Corinth and visit to Ephesus follow from Paul&#39;s statement in 1Cor.16.17, and the assumption that Paul was in Ephesus when he wrote 1 Corinthians. </rdfs:comment>
    </owl:NamedIndividual>
    


    <!-- http://semanticbible.org/ns/2006/NTNames#Achim -->

    <owl:NamedIndividual rdf:about="http://semanticbible.org/ns/2006/NTNames#Achim">
        <rdfs:label xml:lang="en">Achim</rdfs:label>
    </owl:NamedIndividual>
    


    <!-- http://semanticbible.org/ns/2006/NTNames#Adam -->

    <owl:NamedIndividual rdf:about="http://semanticbible.org/ns/2006/NTNames#Adam">
        <rdfs:label xml:lang="en">Adam</rdfs:label>
        <rdfs:comment xml:lang="en">Though Luke&#39;s geneaology lists Adam as &quot;the son of God&quot;, this is not in the biological sense of childOf</rdfs:comment>
    </owl:NamedIndividual>
    


    <!-- http://semanticbible.org/ns/2006/NTNames#Addi -->

    <owl:NamedIndividual rdf:about="http://semanticbible.org/ns/2006/NTNames#Addi">
        <rdfs:label xml:lang="en">Addi</rdfs:label>
    </owl:NamedIndividual>
    


    <!-- http://semanticbible.org/ns/2006/NTNames#Admin -->

    <owl:NamedIndividual rdf:about="http://semanticbible.org/ns/2006/NTNames#Admin">
        <rdfs:label xml:lang="en">Admin</rdfs:label>
        <rdfs:label xml:lang="en">Aram</rdfs:label>
    </owl:NamedIndividual>
    


    <!-- http://semanticbible.org/ns/2006/NTNames#Adramyttium -->

    <owl:NamedIndividual rdf:about="http://semanticbible.org/ns/2006/NTNames#Adramyttium">
        <rdfs:label xml:lang="en">Adramyttium</rdfs:label>
    </owl:NamedIndividual>
    


    <!-- http://semanticbible.org/ns/2006/NTNames#Adriatic -->

    <owl:NamedIndividual rdf:about="http://semanticbible.org/ns/2006/NTNames#Adriatic">
        <rdfs:label xml:lang="en">Adriatic</rdfs:label>
    </owl:NamedIndividual>
    


    <!-- http://semanticbible.org/ns/2006/NTNames#Aeneas -->

    <owl:NamedIndividual rdf:about="http://semanticbible.org/ns/2006/NTNames#Aeneas">
        <rdfs:label xml:lang="en">Aeneas</rdfs:label>
    </owl:NamedIndividual>
    


    <!-- http://semanticbible.org/ns/2006/NTNames#Aenon -->

    <owl:NamedIndividual rdf:about="http://semanticbible.org/ns/2006/NTNames#Aenon">
        <rdf:type rdf:resource="http://semanticbible.org/ns/2006/NTNames#LandArea"/>
        <rdfs:label xml:lang="en">Aenon</rdfs:label>
    </owl:NamedIndividual>
    


    <!-- http://semanticbible.org/ns/2006/NTNames#Agabus -->

    <owl:NamedIndividual rdf:about="http://semanticbible.org/ns/2006/NTNames#Agabus">
        <rdfs:label xml:lang="en">Agabus</rdfs:label>
        <occupation rdf:datatype="http://www.w3.org/2001/XMLSchema#string">prophet</occupation>
        <collaboratesWith rdf:resource="http://semanticbible.org/ns/2006/NTNames#Paul"/>
    </owl:NamedIndividual>
    


    <!-- http://semanticbible.org/ns/2006/NTNames#Ahaz -->

    <owl:NamedIndividual rdf:about="http://semanticbible.org/ns/2006/NTNames#Ahaz">
        <rdf:type rdf:resource="http://semanticbible.org/ns/2006/NTNames#Man"/>
        <rdfs:label xml:lang="en">Ahaz</rdfs:label>
        <rdfs:comment xml:lang="en">See OT descriptions in 2 Kings 16; Isa. 7-9; 2 Chr. 28.</rdfs:comment>
        <parentOf rdf:resource="http://semanticbible.org/ns/2006/NTNames#Hezekiah"/>
    </owl:NamedIndividual>
    


    <!-- http://semanticbible.org/ns/2006/NTNames#Akeldama -->

    <owl:NamedIndividual rdf:about="http://semanticbible.org/ns/2006/NTNames#Akeldama">
        <rdfs:label xml:lang="en">Akeldama</rdfs:label>
    </owl:NamedIndividual>
    


    <!-- http://semanticbible.org/ns/2006/NTNames#Alexander -->

    <owl:NamedIndividual rdf:about="http://semanticbible.org/ns/2006/NTNames#Alexander">
        <rdfs:label xml:lang="en">Alexander</rdfs:label>
        <hasOnlyGenealogyMention rdf:datatype="http://www.w3.org/2001/XMLSchema#boolean">false</hasOnlyGenealogyMention>
    </owl:NamedIndividual>
    


    <!-- http://semanticbible.org/ns/2006/NTNames#AlexanderOfEphesus -->

    <owl:NamedIndividual rdf:about="http://semanticbible.org/ns/2006/NTNames#AlexanderOfEphesus">
        <rdfs:label xml:lang="en">Alexander</rdfs:label>
    </owl:NamedIndividual>
    


    <!-- http://semanticbible.org/ns/2006/NTNames#AlexanderOfTheSanhedrin -->

    <owl:NamedIndividual rdf:about="http://semanticbible.org/ns/2006/NTNames#AlexanderOfTheSanhedrin">
        <rdf:type rdf:resource="http://semanticbible.org/ns/2006/NTNames#Man"/>
        <rdfs:label xml:lang="en">Alexander</rdfs:label>
        <collaboratesWith rdf:resource="http://semanticbible.org/ns/2006/NTNames#JohnOfTheSanhedrin"/>
        <relativeOf rdf:resource="http://semanticbible.org/ns/2006/NTNames#JohnOfTheSanhedrin"/>
    </owl:NamedIndividual>
    


    <!-- http://semanticbible.org/ns/2006/NTNames#AlexanderTheCoppersmith -->

    <owl:NamedIndividual rdf:about="http://semanticbible.org/ns/2006/NTNames#AlexanderTheCoppersmith">
        <rdfs:label xml:lang="en">Alexander</rdfs:label>
        <rdfs:comment xml:lang="en">This may be the same as AlexanderTheHeretic, since they are both identified as opponents of Paul and the Gospel, and they both resided in Ephesus.</rdfs:comment>
    </owl:NamedIndividual>
    


    <!-- http://semanticbible.org/ns/2006/NTNames#AlexanderTheHeretic -->

    <owl:NamedIndividual rdf:about="http://semanticbible.org/ns/2006/NTNames#AlexanderTheHeretic">
        <rdfs:label xml:lang="en">Alexander</rdfs:label>
    </owl:NamedIndividual>
    


    <!-- http://semanticbible.org/ns/2006/NTNames#Alexandria -->

    <owl:NamedIndividual rdf:about="http://semanticbible.org/ns/2006/NTNames#Alexandria">
        <rdfs:label xml:lang="en">Alexandria</rdfs:label>
    </owl:NamedIndividual>
    


    <!-- http://semanticbible.org/ns/2006/NTNames#AlexandriaGeodata -->

    <owl:NamedIndividual rdf:about="http://semanticbible.org/ns/2006/NTNames#AlexandriaGeodata">
        <rdfs:label xml:lang="en">geodata for Alexandria</rdfs:label>
    </owl:NamedIndividual>
    


    <!-- http://semanticbible.org/ns/2006/NTNames#Alexandrians -->

    <owl:NamedIndividual rdf:about="http://semanticbible.org/ns/2006/NTNames#Alexandrians">
        <rdfs:label xml:lang="en">Alexandrians</rdfs:label>
    </owl:NamedIndividual>
    


    <!-- http://semanticbible.org/ns/2006/NTNames#Almighty -->

    <owl:NamedIndividual rdf:about="http://semanticbible.org/ns/2006/NTNames#Almighty">
        <rdfs:label xml:lang="en">Almighty</rdfs:label>
        <rdfs:comment rdf:datatype="http://www.w3.org/2001/XMLSchema#string">&quot;Eli&quot; is Aramaic for &quot;My God&quot;. </rdfs:comment>
    </owl:NamedIndividual>
    


    <!-- http://semanticbible.org/ns/2006/NTNames#Alpha -->

    <owl:NamedIndividual rdf:about="http://semanticbible.org/ns/2006/NTNames#Alpha">
        <rdfs:label xml:lang="en">Alpha</rdfs:label>
    </owl:NamedIndividual>
    


    <!-- http://semanticbible.org/ns/2006/NTNames#Alphaeus -->

    <owl:NamedIndividual rdf:about="http://semanticbible.org/ns/2006/NTNames#Alphaeus">
        <rdfs:label xml:lang="en">Alphaeus</rdfs:label>
        <rdfs:comment rdf:datatype="http://www.w3.org/2001/XMLSchema#string">The identification of Alphaeus with Clopas is not completely certain: see ISBE for Alphaeus.</rdfs:comment>
    </owl:NamedIndividual>
    


    <!-- http://semanticbible.org/ns/2006/NTNames#AlphaeusFatherOfLevi -->

    <owl:NamedIndividual rdf:about="http://semanticbible.org/ns/2006/NTNames#AlphaeusFatherOfLevi">
        <rdfs:label xml:lang="en">Alphaeus</rdfs:label>
        <rdfs:comment xml:lang="en">That both James the Less and Levi had fathers named Alphaeus has led some to speculate they were brothers, but this seems unlikely.</rdfs:comment>
    </owl:NamedIndividual>
    


    <!-- http://semanticbible.org/ns/2006/NTNames#Amminadab -->

    <owl:NamedIndividual rdf:about="http://semanticbible.org/ns/2006/NTNames#Amminadab">
        <rdfs:label xml:lang="en">Amminadab</rdfs:label>
    </owl:NamedIndividual>
    


    <!-- http://semanticbible.org/ns/2006/NTNames#Amos -->

    <owl:NamedIndividual rdf:about="http://semanticbible.org/ns/2006/NTNames#Amos">
        <rdfs:label xml:lang="en">Amos</rdfs:label>
        <ethnicity rdf:resource="http://semanticbible.org/ns/2006/NTNames#Jewish"/>
    </owl:NamedIndividual>
    


    <!-- http://semanticbible.org/ns/2006/NTNames#AmosSonOfNahum -->

    <owl:NamedIndividual rdf:about="http://semanticbible.org/ns/2006/NTNames#AmosSonOfNahum">
        <rdfs:label xml:lang="en">Amos</rdfs:label>
        <rdfs:comment xml:lang="en">There&#39;s no evidence other than the similar (and not uncommon) name to suggest this man is the same Amos as the Old Testament prophet. </rdfs:comment>
    </owl:NamedIndividual>
    


    <!-- http://semanticbible.org/ns/2006/NTNames#Amphipolis -->

    <owl:NamedIndividual rdf:about="http://semanticbible.org/ns/2006/NTNames#Amphipolis">
        <rdf:type rdf:resource="http://semanticbible.org/ns/2006/NTNames#City"/>
        <rdfs:label xml:lang="en">Amphipolis</rdfs:label>
    </owl:NamedIndividual>
    


    <!-- http://semanticbible.org/ns/2006/NTNames#AmphipolisGeodata -->

    <owl:NamedIndividual rdf:about="http://semanticbible.org/ns/2006/NTNames#AmphipolisGeodata">
        <rdfs:label xml:lang="en">geodata for Amphipolis</rdfs:label>
        <longitude rdf:datatype="http://www.w3.org/2001/XMLSchema#double">23.83947945942736</longitude>
    </owl:NamedIndividual>
    


    <!-- http://semanticbible.org/ns/2006/NTNames#Ampliatus -->

    <owl:NamedIndividual rdf:about="http://semanticbible.org/ns/2006/NTNames#Ampliatus">
        <rdfs:label xml:lang="en">Ampliatus</rdfs:label>
        <residentPlace rdf:resource="http://semanticbible.org/ns/2006/NTNames#Rome"/>
    </owl:NamedIndividual>
    


    <!-- http://semanticbible.org/ns/2006/NTNames#Ananias -->

    <owl:NamedIndividual rdf:about="http://semanticbible.org/ns/2006/NTNames#Ananias">
        <rdfs:label xml:lang="en">Ananias</rdfs:label>
        <description rdf:datatype="http://www.w3.org/2001/XMLSchema#string">A member of the early church in Jerusalem who conspired with his wife to deceive the church about a gift of property, and who was consequently struck dead.</description>
        <rdfs:comment rdf:datatype="http://www.w3.org/2001/XMLSchema#string">Residence in Jerusalem is assumed by the account in Acts 5, where the church is still primarily Jersualem-based. </rdfs:comment>
    </owl:NamedIndividual>
    


    <!-- http://semanticbible.org/ns/2006/NTNames#AnaniasOfDamascus -->

    <owl:NamedIndividual rdf:about="http://semanticbible.org/ns/2006/NTNames#AnaniasOfDamascus">
        <rdfs:label xml:lang="en">Ananias</rdfs:label>
        <description rdf:datatype="http://www.w3.org/2001/XMLSchema#string">Ananias was sent to Paul to restore his sight, after his encounter with Christ on the road to Damascus</description>
    </owl:NamedIndividual>
    


    <!-- http://semanticbible.org/ns/2006/NTNames#AnaniasTheHighPriest -->

    <owl:NamedIndividual rdf:about="http://semanticbible.org/ns/2006/NTNames#AnaniasTheHighPriest">
        <rdfs:label xml:lang="en">Ananias</rdfs:label>
        <rdfs:comment rdf:datatype="http://www.w3.org/2001/XMLSchema#string">ISBE describes him as a Sadducee, though it&#39;s not clear why.</rdfs:comment>
    </owl:NamedIndividual>
    


    <!-- http://semanticbible.org/ns/2006/NTNames#Andrew -->

    <owl:NamedIndividual rdf:about="http://semanticbible.org/ns/2006/NTNames#Andrew">
        <rdfs:label xml:lang="en">Andrew</rdfs:label>
        <description rdf:datatype="http://www.w3.org/2001/XMLSchema#string">One of Jesus&#39; twelve apostles, and the first one called.</description>
        <rdfs:comment xml:lang="en">One could infer that Andrew followed Jesus back from Bethany to Galilee in his early ministry, and therefore visited Cana and Capernaum. But this is not explicitly described.</rdfs:comment>
        <collaboratesWith rdf:resource="http://semanticbible.org/ns/2006/NTNames#JohnSonOfZebedee"/>
        <siblingOf rdf:resource="http://semanticbible.org/ns/2006/NTNames#SimonPeter"/>
    </owl:NamedIndividual>
    


    <!-- http://semanticbible.org/ns/2006/NTNames#Andronicus -->

    <owl:NamedIndividual rdf:about="http://semanticbible.org/ns/2006/NTNames#Andronicus">
        <rdfs:label xml:lang="en">Andronicus</rdfs:label>
        <rdfs:comment xml:lang="en">Paul&#39;s description of Andronicus as &quot;my kinsman&quot; is taken in the general snese (e.g. coming from the same region), rather than literally. As a &quot;fellow-prisoner&quot;, he and Junia are assumed to be collaborators with Paul. </rdfs:comment>
        <religiousBelief rdf:resource="http://semanticbible.org/ns/2006/NTNames#Christianity"/>
    </owl:NamedIndividual>
    


    <!-- http://semanticbible.org/ns/2006/NTNames#Anna -->

    <owl:NamedIndividual rdf:about="http://semanticbible.org/ns/2006/NTNames#Anna">
        <rdfs:label xml:lang="en">Anna</rdfs:label>
        <hasOnlyGenealogyMention rdf:datatype="http://www.w3.org/2001/XMLSchema#boolean">false</hasOnlyGenealogyMention>
        <ethnicity rdf:resource="http://semanticbible.org/ns/2006/NTNames#Jewish"/>
        <childOf rdf:resource="http://semanticbible.org/ns/2006/NTNames#Phanuel"/>
    </owl:NamedIndividual>
    


    <!-- http://semanticbible.org/ns/2006/NTNames#Annas -->

    <owl:NamedIndividual rdf:about="http://semanticbible.org/ns/2006/NTNames#Annas">
        <rdfs:label xml:lang="en">Annas</rdfs:label>
        <rdfs:comment xml:lang="en">Annas&#39; highpriesthood ended in 15 AD, but he continued to be described as high-priest after his son-in-law, Caiaphas, had taken the position.</rdfs:comment>
        <collaboratesWith rdf:resource="http://semanticbible.org/ns/2006/NTNames#Caiaphas"/>
    </owl:NamedIndividual>
    


    <!-- http://semanticbible.org/ns/2006/NTNames#Antioch -->

    <owl:NamedIndividual rdf:about="http://semanticbible.org/ns/2006/NTNames#Antioch">
        <rdfs:label xml:lang="en">Antioch</rdfs:label>
    </owl:NamedIndividual>
    


    <!-- http://semanticbible.org/ns/2006/NTNames#AntiochGeodata -->

    <owl:NamedIndividual rdf:about="http://semanticbible.org/ns/2006/NTNames#AntiochGeodata">
        <rdfs:label xml:lang="en">geodata for Antioch</rdfs:label>
    </owl:NamedIndividual>
    


    <!-- http://semanticbible.org/ns/2006/NTNames#AntiochInPisidia -->

    <owl:NamedIndividual rdf:about="http://semanticbible.org/ns/2006/NTNames#AntiochInPisidia">
        <rdfs:label xml:lang="en">Antioch</rdfs:label>
        <rdfs:label xml:lang="en">Antioch in Pisidia</rdfs:label>
        <rdfs:comment xml:lang="en">This Antioch is located in the Pisidian region of Asia Minor, a different place from the town of the same name in Syria</rdfs:comment>
    </owl:NamedIndividual>
    


    <!-- http://semanticbible.org/ns/2006/NTNames#AntiochInPisidiaGeodata -->

    <owl:NamedIndividual rdf:about="http://semanticbible.org/ns/2006/NTNames#AntiochInPisidiaGeodata">
        <rdfs:label xml:lang="en">geodata for Antioch</rdfs:label>
        <altitude rdf:datatype="http://www.w3.org/2001/XMLSchema#int">0</altitude>
    </owl:NamedIndividual>
    


    <!-- http://semanticbible.org/ns/2006/NTNames#Antipas -->

    <owl:NamedIndividual rdf:about="http://semanticbible.org/ns/2006/NTNames#Antipas">
        <rdfs:label xml:lang="en">Antipas</rdfs:label>
    </owl:NamedIndividual>
    


    <!-- http://semanticbible.org/ns/2006/NTNames#Antipatris -->

    <owl:NamedIndividual rdf:about="http://semanticbible.org/ns/2006/NTNames#Antipatris">
        <rdfs:label xml:lang="en">Antipatris</rdfs:label>
        <location rdf:resource="http://semanticbible.org/ns/2006/NTNames#AntipatrisGeodata"/>
    </owl:NamedIndividual>
    


    <!-- http://semanticbible.org/ns/2006/NTNames#AntipatrisGeodata -->

    <owl:NamedIndividual rdf:about="http://semanticbible.org/ns/2006/NTNames#AntipatrisGeodata">
        <rdfs:label xml:lang="en">geodata for Antipatris</rdfs:label>
    </owl:NamedIndividual>
    


    <!-- http://semanticbible.org/ns/2006/NTNames#Apelles -->

    <owl:NamedIndividual rdf:about="http://semanticbible.org/ns/2006/NTNames#Apelles">
        <rdfs:label xml:lang="en">Apelles</rdfs:label>
        <religiousBelief rdf:resource="http://semanticbible.org/ns/2006/NTNames#Christianity"/>
        <knows rdf:resource="http://semanticbible.org/ns/2006/NTNames#Priscilla"/>
    </owl:NamedIndividual>
    


    <!-- http://semanticbible.org/ns/2006/NTNames#Apollonia -->

    <owl:NamedIndividual rdf:about="http://semanticbible.org/ns/2006/NTNames#Apollonia">
        <rdfs:label xml:lang="en">Apollonia</rdfs:label>
    </owl:NamedIndividual>
    


    <!-- http://semanticbible.org/ns/2006/NTNames#ApolloniaGeodata -->

    <owl:NamedIndividual rdf:about="http://semanticbible.org/ns/2006/NTNames#ApolloniaGeodata">
        <rdfs:label xml:lang="en">geodata for Apollonia</rdfs:label>
    </owl:NamedIndividual>
    


    <!-- http://semanticbible.org/ns/2006/NTNames#Apollos -->

    <owl:NamedIndividual rdf:about="http://semanticbible.org/ns/2006/NTNames#Apollos">
        <rdfs:label xml:lang="en">Apollos</rdfs:label>
        <collaboratesWith rdf:resource="http://semanticbible.org/ns/2006/NTNames#Aquila"/>
    </owl:NamedIndividual>
    


    <!-- http://semanticbible.org/ns/2006/NTNames#Apphia -->

    <owl:NamedIndividual rdf:about="http://semanticbible.org/ns/2006/NTNames#Apphia">
        <rdf:type rdf:resource="http://semanticbible.org/ns/2006/NTNames#Woman"/>
        <rdfs:label xml:lang="en">Apphia</rdfs:label>
        <rdfs:comment xml:lang="en">Being the spouseOf Philemon is implied by their mention together in the salutation of the Letter to Philemon, though it is not definite. 
Paul describes her as &quot;our sister&quot;, presumably in Christ rather than literally. See Philemon about ResidentPlace.</rdfs:comment>
        <religiousBelief rdf:resource="http://semanticbible.org/ns/2006/NTNames#Christianity"/>
    </owl:NamedIndividual>
    


    <!-- http://semanticbible.org/ns/2006/NTNames#Appius -->

    <owl:NamedIndividual rdf:about="http://semanticbible.org/ns/2006/NTNames#Appius">
        <rdf:type rdf:resource="http://semanticbible.org/ns/2006/NTNames#City"/>
        <rdfs:label xml:lang="en">Appius</rdfs:label>
    </owl:NamedIndividual>
    


    <!-- http://semanticbible.org/ns/2006/NTNames#Aquila -->

    <owl:NamedIndividual rdf:about="http://semanticbible.org/ns/2006/NTNames#Aquila">
        <rdfs:label xml:lang="en">Aquila</rdfs:label>
        <description rdf:datatype="http://www.w3.org/2001/XMLSchema#string">a tentmaked converted by Paul who, together with his wife, became evangelists</description>
        <collaboratesWith rdf:resource="http://semanticbible.org/ns/2006/NTNames#Apollos"/>
    </owl:NamedIndividual>
    


    <!-- http://semanticbible.org/ns/2006/NTNames#Arabia -->

    <owl:NamedIndividual rdf:about="http://semanticbible.org/ns/2006/NTNames#Arabia">
        <rdfs:label xml:lang="en">Arabia</rdfs:label>
    </owl:NamedIndividual>
    


    <!-- http://semanticbible.org/ns/2006/NTNames#Arabians -->

    <owl:NamedIndividual rdf:about="http://semanticbible.org/ns/2006/NTNames#Arabians">
        <rdfs:label xml:lang="en">Arabians</rdfs:label>
    </owl:NamedIndividual>
    


    <!-- http://semanticbible.org/ns/2006/NTNames#Aramaic -->

    <owl:NamedIndividual rdf:about="http://semanticbible.org/ns/2006/NTNames#Aramaic">
        <rdfs:label xml:lang="en">Aramaic</rdfs:label>
    </owl:NamedIndividual>
    


    <!-- http://semanticbible.org/ns/2006/NTNames#Archelaus -->

    <owl:NamedIndividual rdf:about="http://semanticbible.org/ns/2006/NTNames#Archelaus">
        <rdfs:label xml:lang="en">Archelaus</rdfs:label>
    </owl:NamedIndividual>
    


    <!-- http://semanticbible.org/ns/2006/NTNames#Archippus -->

    <owl:NamedIndividual rdf:about="http://semanticbible.org/ns/2006/NTNames#Archippus">
        <rdfs:label xml:lang="en">Archippus</rdfs:label>
        <rdfs:comment xml:lang="en">Paul describes Archippus as &quot;our fellow soldier&quot; in Philemon 1:2, perhaps based on service together in Ephesus (RWP).</rdfs:comment>
    </owl:NamedIndividual>
    


    <!-- http://semanticbible.org/ns/2006/NTNames#Areopagite -->

    <owl:NamedIndividual rdf:about="http://semanticbible.org/ns/2006/NTNames#Areopagite">
        <rdfs:label xml:lang="en">Areopagite</rdfs:label>
    </owl:NamedIndividual>
    


    <!-- http://semanticbible.org/ns/2006/NTNames#Areopagus -->

    <owl:NamedIndividual rdf:about="http://semanticbible.org/ns/2006/NTNames#Areopagus">
        <rdfs:label xml:lang="en">Areopagus</rdfs:label>
    </owl:NamedIndividual>
    


    <!-- http://semanticbible.org/ns/2006/NTNames#Aretas -->

    <owl:NamedIndividual rdf:about="http://semanticbible.org/ns/2006/NTNames#Aretas">
        <rdfs:label xml:lang="en">Aretas</rdfs:label>
    </owl:NamedIndividual>
    


    <!-- http://semanticbible.org/ns/2006/NTNames#Arimathea -->

    <owl:NamedIndividual rdf:about="http://semanticbible.org/ns/2006/NTNames#Arimathea">
        <rdfs:label xml:lang="en">Arimathea</rdfs:label>
        <rdfs:comment xml:lang="en">Arimathea is known as the native place of Joseph, a member of the Sanhedrin and a disciple who put Jesus&#39; body in his own tomb after the crucifixion.</rdfs:comment>
    </owl:NamedIndividual>
    


    <!-- http://semanticbible.org/ns/2006/NTNames#ArimatheaGeodata -->

    <owl:NamedIndividual rdf:about="http://semanticbible.org/ns/2006/NTNames#ArimatheaGeodata">
        <rdfs:label xml:lang="en">geodata for Arimathea</rdfs:label>
    </owl:NamedIndividual>
    


    <!-- http://semanticbible.org/ns/2006/NTNames#Aristarchus -->

    <owl:NamedIndividual rdf:about="http://semanticbible.org/ns/2006/NTNames#Aristarchus">
        <rdfs:label xml:lang="en">Aristarchus</rdfs:label>
    </owl:NamedIndividual>
    


    <!-- http://semanticbible.org/ns/2006/NTNames#Aristobulus -->

    <owl:NamedIndividual rdf:about="http://semanticbible.org/ns/2006/NTNames#Aristobulus">
        <rdfs:label xml:lang="en">Aristobulus</rdfs:label>
        <rdfs:comment xml:lang="en">Paul addresses &quot;the family/household of Aristobulus&quot;, which may refer to slaves: so we have no evidence about the beliefs or other attributes of Aristobulus himself, other than his residence in Rome. One of the grandsons of Herod the Great had this name, though the name was common enough that this need not be the same man. </rdfs:comment>
    </owl:NamedIndividual>
    


    <!-- http://semanticbible.org/ns/2006/NTNames#Armageddon -->

    <owl:NamedIndividual rdf:about="http://semanticbible.org/ns/2006/NTNames#Armageddon">
        <rdfs:label xml:lang="en">Armageddon</rdfs:label>
    </owl:NamedIndividual>
    


    <!-- http://semanticbible.org/ns/2006/NTNames#Arni -->

    <owl:NamedIndividual rdf:about="http://semanticbible.org/ns/2006/NTNames#Arni">
        <rdfs:label xml:lang="en">Arni</rdfs:label>
        <rdfs:comment xml:lang="en">Likely a variant form of Ram, as Hezron&#39;s son is called in Matthew&#39;s genealogy. </rdfs:comment>
    </owl:NamedIndividual>
    


    <!-- http://semanticbible.org/ns/2006/NTNames#Arphaxad -->

    <owl:NamedIndividual rdf:about="http://semanticbible.org/ns/2006/NTNames#Arphaxad">
        <rdfs:label xml:lang="en">Arphaxad</rdfs:label>
    </owl:NamedIndividual>
    


    <!-- http://semanticbible.org/ns/2006/NTNames#Artemas -->

    <owl:NamedIndividual rdf:about="http://semanticbible.org/ns/2006/NTNames#Artemas">
        <rdfs:label xml:lang="en">Artemas</rdfs:label>
    </owl:NamedIndividual>
    


    <!-- http://semanticbible.org/ns/2006/NTNames#Artemis -->

    <owl:NamedIndividual rdf:about="http://semanticbible.org/ns/2006/NTNames#Artemis">
        <rdfs:label xml:lang="en">Artemis</rdfs:label>
    </owl:NamedIndividual>
    


    <!-- http://semanticbible.org/ns/2006/NTNames#Asaph -->

    <owl:NamedIndividual rdf:about="http://semanticbible.org/ns/2006/NTNames#Asaph">
        <rdfs:label xml:lang="en">Asaph</rdfs:label>
        <rdfs:comment xml:lang="en">Not the same as the psalmist and leader of King David&#39;s choir in 1Chr.6.39.</rdfs:comment>
    </owl:NamedIndividual>
    


    <!-- http://semanticbible.org/ns/2006/NTNames#Asher -->

    <owl:NamedIndividual rdf:about="http://semanticbible.org/ns/2006/NTNames#Asher">
        <rdfs:label xml:lang="en">Asher</rdfs:label>
        <rdfs:comment xml:lang="en">One of the sons of Judah</rdfs:comment>
        <childOf rdf:resource="http://semanticbible.org/ns/2006/NTNames#Jacob"/>
    </owl:NamedIndividual>
    


    <!-- http://semanticbible.org/ns/2006/NTNames#Asia -->

    <owl:NamedIndividual rdf:about="http://semanticbible.org/ns/2006/NTNames#Asia">
        <rdfs:label xml:lang="en">Asia</rdfs:label>
    </owl:NamedIndividual>
    


    <!-- http://semanticbible.org/ns/2006/NTNames#Asians -->

    <owl:NamedIndividual rdf:about="http://semanticbible.org/ns/2006/NTNames#Asians">
        <rdfs:label xml:lang="en">Asians</rdfs:label>
    </owl:NamedIndividual>
    


    <!-- http://semanticbible.org/ns/2006/NTNames#Asiarchs -->

    <owl:NamedIndividual rdf:about="http://semanticbible.org/ns/2006/NTNames#Asiarchs">
        <rdf:type rdf:resource="http://semanticbible.org/ns/2006/NTNames#GroupOfPeople"/>
        <rdfs:label xml:lang="en">Asiarchs</rdfs:label>
    </owl:NamedIndividual>
    


    <!-- http://semanticbible.org/ns/2006/NTNames#Assassins -->

    <owl:NamedIndividual rdf:about="http://semanticbible.org/ns/2006/NTNames#Assassins">
        <rdf:type rdf:resource="http://semanticbible.org/ns/2006/NTNames#PoliticalOrganization"/>
        <rdfs:label xml:lang="en">Assassins</rdfs:label>
    </owl:NamedIndividual>
    


    <!-- http://semanticbible.org/ns/2006/NTNames#Assos -->

    <owl:NamedIndividual rdf:about="http://semanticbible.org/ns/2006/NTNames#Assos">
        <rdfs:label xml:lang="en">Assos</rdfs:label>
    </owl:NamedIndividual>
    


    <!-- http://semanticbible.org/ns/2006/NTNames#AssosGeodata -->

    <owl:NamedIndividual rdf:about="http://semanticbible.org/ns/2006/NTNames#AssosGeodata">
        <rdfs:label xml:lang="en">geodata for Assos</rdfs:label>
    </owl:NamedIndividual>
    


    <!-- http://semanticbible.org/ns/2006/NTNames#Asyncritus -->

    <owl:NamedIndividual rdf:about="http://semanticbible.org/ns/2006/NTNames#Asyncritus">
        <rdfs:label xml:lang="en">Asyncritus</rdfs:label>
        <residentPlace rdf:resource="http://semanticbible.org/ns/2006/NTNames#Rome"/>
    </owl:NamedIndividual>
    


    <!-- http://semanticbible.org/ns/2006/NTNames#Athenians -->

    <owl:NamedIndividual rdf:about="http://semanticbible.org/ns/2006/NTNames#Athenians">
        <rdfs:label xml:lang="en">Athenians</rdfs:label>
    </owl:NamedIndividual>
    


    <!-- http://semanticbible.org/ns/2006/NTNames#Athens -->

    <owl:NamedIndividual rdf:about="http://semanticbible.org/ns/2006/NTNames#Athens">
        <rdfs:label xml:lang="en">Athens</rdfs:label>
    </owl:NamedIndividual>
    


    <!-- http://semanticbible.org/ns/2006/NTNames#Attalia -->

    <owl:NamedIndividual rdf:about="http://semanticbible.org/ns/2006/NTNames#Attalia">
        <rdfs:label xml:lang="en">Attalia</rdfs:label>
        <location rdf:resource="http://semanticbible.org/ns/2006/NTNames#AttaliaGeodata"/>
    </owl:NamedIndividual>
    


    <!-- http://semanticbible.org/ns/2006/NTNames#AttaliaGeodata -->

    <owl:NamedIndividual rdf:about="http://semanticbible.org/ns/2006/NTNames#AttaliaGeodata">
        <rdfs:label xml:lang="en">geodata for Attalia</rdfs:label>
    </owl:NamedIndividual>
    


    <!-- http://semanticbible.org/ns/2006/NTNames#AugustanCohort -->

    <owl:NamedIndividual rdf:about="http://semanticbible.org/ns/2006/NTNames#AugustanCohort">
        <rdf:type rdf:resource="http://semanticbible.org/ns/2006/NTNames#PoliticalOrganization"/>
        <rdfs:label xml:lang="en">Augustan Cohort</rdfs:label>
        <rdfs:comment xml:lang="en">A Roman legion.</rdfs:comment>
    </owl:NamedIndividual>
    


    <!-- http://semanticbible.org/ns/2006/NTNames#Augustus -->

    <owl:NamedIndividual rdf:about="http://semanticbible.org/ns/2006/NTNames#Augustus">
        <rdfs:label xml:lang="en">Augustus</rdfs:label>
    </owl:NamedIndividual>
    


    <!-- http://semanticbible.org/ns/2006/NTNames#Azor -->

    <owl:NamedIndividual rdf:about="http://semanticbible.org/ns/2006/NTNames#Azor">
        <rdf:type rdf:resource="http://semanticbible.org/ns/2006/NTNames#Man"/>
        <rdfs:label xml:lang="en">Azor</rdfs:label>
        <childOf rdf:resource="http://semanticbible.org/ns/2006/NTNames#EliakimSonOfAbiud"/>
    </owl:NamedIndividual>
    


    <!-- http://semanticbible.org/ns/2006/NTNames#Azotus -->

    <owl:NamedIndividual rdf:about="http://semanticbible.org/ns/2006/NTNames#Azotus">
        <rdfs:label xml:lang="en">Azotus</rdfs:label>
        <subregionOf rdf:resource="http://semanticbible.org/ns/2006/NTNames#Judea"/>
    </owl:NamedIndividual>
    


    <!-- http://semanticbible.org/ns/2006/NTNames#Babylon -->

    <owl:NamedIndividual rdf:about="http://semanticbible.org/ns/2006/NTNames#Babylon">
        <rdf:type rdf:resource="http://semanticbible.org/ns/2006/NTNames#City"/>
        <rdfs:label xml:lang="en">Babylon</rdfs:label>
        <rdfs:comment xml:lang="en">Babylon also has a metaphorical usage as a symbol of the world system opposed to God</rdfs:comment>
    </owl:NamedIndividual>
    


    <!-- http://semanticbible.org/ns/2006/NTNames#BabylonGeodata -->

    <owl:NamedIndividual rdf:about="http://semanticbible.org/ns/2006/NTNames#BabylonGeodata">
        <rdfs:label xml:lang="en">geodata for Babylon</rdfs:label>
        <latitude rdf:datatype="http://www.w3.org/2001/XMLSchema#double">32.53660983263659</latitude>
        <longitude rdf:datatype="http://www.w3.org/2001/XMLSchema#double">44.42007455918414</longitude>
    </owl:NamedIndividual>
    


    <!-- http://semanticbible.org/ns/2006/NTNames#Balaam -->

    <owl:NamedIndividual rdf:about="http://semanticbible.org/ns/2006/NTNames#Balaam">
        <rdfs:label xml:lang="en">Balaam</rdfs:label>
    </owl:NamedIndividual>
    


    <!-- http://semanticbible.org/ns/2006/NTNames#Balak -->

    <owl:NamedIndividual rdf:about="http://semanticbible.org/ns/2006/NTNames#Balak">
        <rdfs:label xml:lang="en">Balak</rdfs:label>
    </owl:NamedIndividual>
    


    <!-- http://semanticbible.org/ns/2006/NTNames#Bar-Jesus -->

    <owl:NamedIndividual rdf:about="http://semanticbible.org/ns/2006/NTNames#Bar-Jesus">
        <rdfs:label xml:lang="en">Bar-Jesus</rdfs:label>
        <rdfs:comment xml:lang="en">Elymas is a transliteration of an Aramaic or Arabic word equivalent to &#39;magician&#39;.</rdfs:comment>
    </owl:NamedIndividual>
    


    <!-- http://semanticbible.org/ns/2006/NTNames#Barabbas -->

    <owl:NamedIndividual rdf:about="http://semanticbible.org/ns/2006/NTNames#Barabbas">
        <rdfs:label xml:lang="en">Barabbas</rdfs:label>
    </owl:NamedIndividual>
    


    <!-- http://semanticbible.org/ns/2006/NTNames#Barachiah -->

    <owl:NamedIndividual rdf:about="http://semanticbible.org/ns/2006/NTNames#Barachiah">
        <rdfs:label xml:lang="en">Barachiah</rdfs:label>
    </owl:NamedIndividual>
    


    <!-- http://semanticbible.org/ns/2006/NTNames#Barak -->

    <owl:NamedIndividual rdf:about="http://semanticbible.org/ns/2006/NTNames#Barak">
        <rdfs:label xml:lang="en">Barak</rdfs:label>
    </owl:NamedIndividual>
    


    <!-- http://semanticbible.org/ns/2006/NTNames#Barnabas -->

    <owl:NamedIndividual rdf:about="http://semanticbible.org/ns/2006/NTNames#Barnabas">
        <rdfs:label xml:lang="en">Barnabas</rdfs:label>
        <collaboratesWith rdf:resource="http://semanticbible.org/ns/2006/NTNames#JohnMark"/>
        <collaboratesWith rdf:resource="http://semanticbible.org/ns/2006/NTNames#SimonPeter"/>
    </owl:NamedIndividual>
    


    <!-- http://semanticbible.org/ns/2006/NTNames#Bartholomew -->

    <owl:NamedIndividual rdf:about="http://semanticbible.org/ns/2006/NTNames#Bartholomew">
        <rdfs:label xml:lang="en">Bartholomew</rdfs:label>
        <rdfs:comment xml:lang="en">Many believe Bartholemew is another name for Nathanael, though their identity is deduced rather than stated.</rdfs:comment>
    </owl:NamedIndividual>
    


    <!-- http://semanticbible.org/ns/2006/NTNames#Bartimaeus -->

    <owl:NamedIndividual rdf:about="http://semanticbible.org/ns/2006/NTNames#Bartimaeus">
        <rdfs:label xml:lang="en">Bartimaeus</rdfs:label>
    </owl:NamedIndividual>
    


    <!-- http://semanticbible.org/ns/2006/NTNames#Bathsheba -->

    <owl:NamedIndividual rdf:about="http://semanticbible.org/ns/2006/NTNames#Bathsheba">
        <rdfs:label xml:lang="en">Bathsheba</rdfs:label>
        <rdfs:comment xml:lang="en">Not named in the New Testament, but referred to in Matt.1.6 as &quot;the wife of Uriah&quot;. Since Uriah was a Hittite, it&#39;s not clear what her religiousBelief might have been. </rdfs:comment>
    </owl:NamedIndividual>
    


    <!-- http://semanticbible.org/ns/2006/NTNames#Benjamin -->

    <owl:NamedIndividual rdf:about="http://semanticbible.org/ns/2006/NTNames#Benjamin">
        <rdfs:label xml:lang="en">Benjamin</rdfs:label>
        <siblingOf rdf:resource="http://semanticbible.org/ns/2006/NTNames#Gad"/>
    </owl:NamedIndividual>
    


    <!-- http://semanticbible.org/ns/2006/NTNames#Beor -->

    <owl:NamedIndividual rdf:about="http://semanticbible.org/ns/2006/NTNames#Beor">
        <rdfs:label xml:lang="en">Beor</rdfs:label>
    </owl:NamedIndividual>
    


    <!-- http://semanticbible.org/ns/2006/NTNames#Berea -->

    <owl:NamedIndividual rdf:about="http://semanticbible.org/ns/2006/NTNames#Berea">
        <rdfs:label xml:lang="en">Berea</rdfs:label>
    </owl:NamedIndividual>
    


    <!-- http://semanticbible.org/ns/2006/NTNames#BereaGeodata -->

    <owl:NamedIndividual rdf:about="http://semanticbible.org/ns/2006/NTNames#BereaGeodata">
        <rdfs:label xml:lang="en">geodata for Berea</rdfs:label>
    </owl:NamedIndividual>
    


    <!-- http://semanticbible.org/ns/2006/NTNames#Bernice -->

    <owl:NamedIndividual rdf:about="http://semanticbible.org/ns/2006/NTNames#Bernice">
        <rdfs:label xml:lang="en">Bernice</rdfs:label>
        <rdfs:comment xml:lang="en">Smith notes that Bernice &quot;lived  under circumstances of great suspicion&quot; with her brother Herod Agrippa II, i.e. they may have had an incestuous relationship. </rdfs:comment>
        <siblingOf rdf:resource="http://semanticbible.org/ns/2006/NTNames#HerodAgrippaII"/>
    </owl:NamedIndividual>
    


    <!-- http://semanticbible.org/ns/2006/NTNames#Bethany -->

    <owl:NamedIndividual rdf:about="http://semanticbible.org/ns/2006/NTNames#Bethany">
        <rdfs:label xml:lang="en">Bethany</rdfs:label>
    </owl:NamedIndividual>
    


    <!-- http://semanticbible.org/ns/2006/NTNames#BethanyBeyondtheJordan -->

    <owl:NamedIndividual rdf:about="http://semanticbible.org/ns/2006/NTNames#BethanyBeyondtheJordan">
        <rdfs:label xml:lang="en">Bethany beyond the Jordan</rdfs:label>
        <rdfs:comment xml:lang="en">Distinguished from the Bethany near Jerusalem: since the time of Origen, the location has been unknown.</rdfs:comment>
    </owl:NamedIndividual>
    


    <!-- http://semanticbible.org/ns/2006/NTNames#BethanyBeyondtheJordanGeodata -->

    <owl:NamedIndividual rdf:about="http://semanticbible.org/ns/2006/NTNames#BethanyBeyondtheJordanGeodata">
        <rdfs:label xml:lang="en">geodata for Bethany Beyond the Jordan</rdfs:label>
    </owl:NamedIndividual>
    


    <!-- http://semanticbible.org/ns/2006/NTNames#Bethesda -->

    <owl:NamedIndividual rdf:about="http://semanticbible.org/ns/2006/NTNames#Bethesda">
        <rdfs:label xml:lang="en">Bethesda</rdfs:label>
    </owl:NamedIndividual>
    


    <!-- http://semanticbible.org/ns/2006/NTNames#Bethlehem -->

    <owl:NamedIndividual rdf:about="http://semanticbible.org/ns/2006/NTNames#Bethlehem">
        <rdfs:label xml:lang="en">Bethlehem</rdfs:label>
    </owl:NamedIndividual>
    


    <!-- http://semanticbible.org/ns/2006/NTNames#BethlehemGeodata -->

    <owl:NamedIndividual rdf:about="http://semanticbible.org/ns/2006/NTNames#BethlehemGeodata">
        <rdfs:label xml:lang="en">geodata for Bethlehem</rdfs:label>
    </owl:NamedIndividual>
    


    <!-- http://semanticbible.org/ns/2006/NTNames#Bethphage -->

    <owl:NamedIndividual rdf:about="http://semanticbible.org/ns/2006/NTNames#Bethphage">
        <rdf:type rdf:resource="http://semanticbible.org/ns/2006/NTNames#City"/>
        <rdfs:label xml:lang="en">Bethphage</rdfs:label>
    </owl:NamedIndividual>
    


    <!-- http://semanticbible.org/ns/2006/NTNames#Bethsaida -->

    <owl:NamedIndividual rdf:about="http://semanticbible.org/ns/2006/NTNames#Bethsaida">
        <rdfs:label xml:lang="en">Bethsaida</rdfs:label>
        <rdfs:comment xml:lang="en">NNE of Sea of Galilee, &quot;Bethsaida Julia&quot;. ISBE has a thorough account
of whether, given Mark 6.45 and John&#39;s &quot;Bethsaida of Galilee&quot;, 
there were two such towns (with a second, smaller one on the west side),
or only one</rdfs:comment>
    </owl:NamedIndividual>
    


    <!-- http://semanticbible.org/ns/2006/NTNames#BethsaidaGeodata -->

    <owl:NamedIndividual rdf:about="http://semanticbible.org/ns/2006/NTNames#BethsaidaGeodata">
        <rdfs:label xml:lang="en">geodata for Bethsaida</rdfs:label>
    </owl:NamedIndividual>
    


    <!-- http://semanticbible.org/ns/2006/NTNames#Bithynia -->

    <owl:NamedIndividual rdf:about="http://semanticbible.org/ns/2006/NTNames#Bithynia">
        <rdfs:label xml:lang="en">Bithynia</rdfs:label>
    </owl:NamedIndividual>
    


    <!-- http://semanticbible.org/ns/2006/NTNames#Blastus -->

    <owl:NamedIndividual rdf:about="http://semanticbible.org/ns/2006/NTNames#Blastus">
        <rdfs:label xml:lang="en">Blastus</rdfs:label>
    </owl:NamedIndividual>
    


    <!-- http://semanticbible.org/ns/2006/NTNames#Boanerges -->

    <owl:NamedIndividual rdf:about="http://semanticbible.org/ns/2006/NTNames#Boanerges">
        <rdf:type rdf:resource="http://semanticbible.org/ns/2006/NTNames#GroupOfPeople"/>
        <rdfs:label xml:lang="en">Boanerges</rdfs:label>
        <rdfs:label xml:lang="en">Sons of Thunder</rdfs:label>
        <rdfs:comment xml:lang="en">Jesus&#39; nickname for two of his disciples: James, the son of Zebedee, and John, his brother.</rdfs:comment>
    </owl:NamedIndividual>
    


    <!-- http://semanticbible.org/ns/2006/NTNames#Boaz -->

    <owl:NamedIndividual rdf:about="http://semanticbible.org/ns/2006/NTNames#Boaz">
        <rdfs:label xml:lang="en">Boaz</rdfs:label>
    </owl:NamedIndividual>
    


    <!-- http://semanticbible.org/ns/2006/NTNames#CaesarAugustus -->

    <owl:NamedIndividual rdf:about="http://semanticbible.org/ns/2006/NTNames#CaesarAugustus">
        <rdfs:label xml:lang="en">Caesar</rdfs:label>
        <rdfs:comment rdf:datatype="http://www.w3.org/2001/XMLSchema#string">Caesar is used as a name for several different individuals in the New Testament</rdfs:comment>
        <occupation rdf:datatype="http://www.w3.org/2001/XMLSchema#string">emperor</occupation>
    </owl:NamedIndividual>
    


    <!-- http://semanticbible.org/ns/2006/NTNames#CaesarNero -->

    <owl:NamedIndividual rdf:about="http://semanticbible.org/ns/2006/NTNames#CaesarNero">
        <rdfs:label xml:lang="en">Caesar</rdfs:label>
        <rdfs:comment rdf:datatype="http://www.w3.org/2001/XMLSchema#string">Caesar is used as a name for several different individuals in the New Testament</rdfs:comment>
        <ethnicity rdf:resource="http://semanticbible.org/ns/2006/NTNames#Roman"/>
    </owl:NamedIndividual>
    


    <!-- http://semanticbible.org/ns/2006/NTNames#Caesarea -->

    <owl:NamedIndividual rdf:about="http://semanticbible.org/ns/2006/NTNames#Caesarea">
        <rdfs:label xml:lang="en">Caesarea</rdfs:label>
    </owl:NamedIndividual>
    


    <!-- http://semanticbible.org/ns/2006/NTNames#CaesareaGeodata -->

    <owl:NamedIndividual rdf:about="http://semanticbible.org/ns/2006/NTNames#CaesareaGeodata">
        <rdfs:label xml:lang="en">geodata for Caesarea</rdfs:label>
    </owl:NamedIndividual>
    


    <!-- http://semanticbible.org/ns/2006/NTNames#CaesareaPhilippi -->

    <owl:NamedIndividual rdf:about="http://semanticbible.org/ns/2006/NTNames#CaesareaPhilippi">
        <rdfs:label xml:lang="en">Caesarea Philippi</rdfs:label>
    </owl:NamedIndividual>
    


    <!-- http://semanticbible.org/ns/2006/NTNames#CaesareaPhilippiGeodata -->

    <owl:NamedIndividual rdf:about="http://semanticbible.org/ns/2006/NTNames#CaesareaPhilippiGeodata">
        <rdfs:label xml:lang="en">geodata for Caesarea Philippi</rdfs:label>
    </owl:NamedIndividual>
    


    <!-- http://semanticbible.org/ns/2006/NTNames#Caiaphas -->

    <owl:NamedIndividual rdf:about="http://semanticbible.org/ns/2006/NTNames#Caiaphas">
        <rdfs:label xml:lang="en">Caiaphas</rdfs:label>
    </owl:NamedIndividual>
    


    <!-- http://semanticbible.org/ns/2006/NTNames#Cain -->

    <owl:NamedIndividual rdf:about="http://semanticbible.org/ns/2006/NTNames#Cain">
        <rdfs:label xml:lang="en">Cain</rdfs:label>
        <siblingOf rdf:resource="http://semanticbible.org/ns/2006/NTNames#Abel"/>
        <childOf rdf:resource="http://semanticbible.org/ns/2006/NTNames#Eve"/>
    </owl:NamedIndividual>
    


    <!-- http://semanticbible.org/ns/2006/NTNames#CainanSonOfArphaxad -->

    <owl:NamedIndividual rdf:about="http://semanticbible.org/ns/2006/NTNames#CainanSonOfArphaxad">
        <rdfs:label xml:lang="en">Cainan</rdfs:label>
    </owl:NamedIndividual>
    


    <!-- http://semanticbible.org/ns/2006/NTNames#CainanSonOfEnosh -->

    <owl:NamedIndividual rdf:about="http://semanticbible.org/ns/2006/NTNames#CainanSonOfEnosh">
        <rdfs:label xml:lang="en">Cainan</rdfs:label>
        <rdfs:comment xml:lang="en">Kenan in the NIV</rdfs:comment>
    </owl:NamedIndividual>
    


    <!-- http://semanticbible.org/ns/2006/NTNames#Caiphas -->

    <owl:NamedIndividual rdf:about="http://semanticbible.org/ns/2006/NTNames#Caiphas">
        <rdf:type rdf:resource="http://semanticbible.org/ns/2006/NTNames#Man"/>
        <rdfs:label xml:lang="en">Caiphas</rdfs:label>
        <rdfs:comment xml:lang="en">see Caiaphas</rdfs:comment>
    </owl:NamedIndividual>
    


    <!-- http://semanticbible.org/ns/2006/NTNames#Cana -->

    <owl:NamedIndividual rdf:about="http://semanticbible.org/ns/2006/NTNames#Cana">
        <rdfs:label xml:lang="en">Cana</rdfs:label>
        <location rdf:resource="http://semanticbible.org/ns/2006/NTNames#CanaGeodata"/>
    </owl:NamedIndividual>
    


    <!-- http://semanticbible.org/ns/2006/NTNames#CanaGeodata -->

    <owl:NamedIndividual rdf:about="http://semanticbible.org/ns/2006/NTNames#CanaGeodata">
        <rdfs:label xml:lang="en">geodata for Cana</rdfs:label>
        <latitude rdf:datatype="http://www.w3.org/2001/XMLSchema#double">32.75209569199829</latitude>
    </owl:NamedIndividual>
    


    <!-- http://semanticbible.org/ns/2006/NTNames#Canaan -->

    <owl:NamedIndividual rdf:about="http://semanticbible.org/ns/2006/NTNames#Canaan">
        <rdfs:label xml:lang="en">Canaan</rdfs:label>
        <residentPlaceOf rdf:resource="http://semanticbible.org/ns/2006/NTNames#Abraham"/>
    </owl:NamedIndividual>
    


    <!-- http://semanticbible.org/ns/2006/NTNames#Canaanite -->

    <owl:NamedIndividual rdf:about="http://semanticbible.org/ns/2006/NTNames#Canaanite">
        <rdfs:label xml:lang="en">Canaanite</rdfs:label>
        <rdfs:comment xml:lang="en">In the Old Testament, a people living west of the Jordan river who were partially displaced by the Israelites. In New Testament times, Canaanites lived primarily in the area of Phoenicia. Cananean, in contrast, is almost certainly political, rather than ethnic. </rdfs:comment>
    </owl:NamedIndividual>
    


    <!-- http://semanticbible.org/ns/2006/NTNames#Cananaean -->

    <owl:NamedIndividual rdf:about="http://semanticbible.org/ns/2006/NTNames#Cananaean">
        <rdfs:label xml:lang="en">Cananaean</rdfs:label>
        <rdfs:comment xml:lang="en">This attribute is only used by Matthew and Mark to describe Simon, one of Jesus&#39; disciples. Given what else we know of Simon, it almost certainly designates a political attribute, rather than ethnicity.</rdfs:comment>
    </owl:NamedIndividual>
    


    <!-- http://semanticbible.org/ns/2006/NTNames#Candace -->

    <owl:NamedIndividual rdf:about="http://semanticbible.org/ns/2006/NTNames#Candace">
        <rdfs:label xml:lang="en">Candace</rdfs:label>
        <rdfs:comment xml:lang="en">Candace is actually a title like &quot;Pharaoh&quot; rather than a personal name, hence her occupation as queen.</rdfs:comment>
    </owl:NamedIndividual>
    


    <!-- http://semanticbible.org/ns/2006/NTNames#Capernaum -->

    <owl:NamedIndividual rdf:about="http://semanticbible.org/ns/2006/NTNames#Capernaum">
        <rdfs:label xml:lang="en">Capernaum</rdfs:label>
    </owl:NamedIndividual>
    


    <!-- http://semanticbible.org/ns/2006/NTNames#CapernaumGeodata -->

    <owl:NamedIndividual rdf:about="http://semanticbible.org/ns/2006/NTNames#CapernaumGeodata">
        <rdf:type rdf:resource="http://semanticbible.org/ns/2006/NTNames#GeographicLocation"/>
        <rdfs:label xml:lang="en">geodata for Capernaum</rdfs:label>
        <longitude rdf:datatype="http://www.w3.org/2001/XMLSchema#double">35.57534055705805</longitude>
    </owl:NamedIndividual>
    


    <!-- http://semanticbible.org/ns/2006/NTNames#Cappadocia -->

    <owl:NamedIndividual rdf:about="http://semanticbible.org/ns/2006/NTNames#Cappadocia">
        <rdfs:label xml:lang="en">Cappadocia</rdfs:label>
    </owl:NamedIndividual>
    


    <!-- http://semanticbible.org/ns/2006/NTNames#Carpus -->

    <owl:NamedIndividual rdf:about="http://semanticbible.org/ns/2006/NTNames#Carpus">
        <rdf:type rdf:resource="http://semanticbible.org/ns/2006/NTNames#Man"/>
        <rdfs:label xml:lang="en">Carpus</rdfs:label>
    </owl:NamedIndividual>
    


    <!-- http://semanticbible.org/ns/2006/NTNames#Cauda -->

    <owl:NamedIndividual rdf:about="http://semanticbible.org/ns/2006/NTNames#Cauda">
        <rdfs:label xml:lang="en">Cauda</rdfs:label>
    </owl:NamedIndividual>
    


    <!-- http://semanticbible.org/ns/2006/NTNames#Cenchreae -->

    <owl:NamedIndividual rdf:about="http://semanticbible.org/ns/2006/NTNames#Cenchreae">
        <rdfs:label xml:lang="en">Cenchreae</rdfs:label>
    </owl:NamedIndividual>
    


    <!-- http://semanticbible.org/ns/2006/NTNames#CenchreaeGeodata -->

    <owl:NamedIndividual rdf:about="http://semanticbible.org/ns/2006/NTNames#CenchreaeGeodata">
        <rdfs:label xml:lang="en">geodata for Cenchreae</rdfs:label>
        <longitude rdf:datatype="http://www.w3.org/2001/XMLSchema#double">22.96102305563464</longitude>
    </owl:NamedIndividual>
    


    <!-- http://semanticbible.org/ns/2006/NTNames#Chaldeans -->

    <owl:NamedIndividual rdf:about="http://semanticbible.org/ns/2006/NTNames#Chaldeans">
        <rdfs:label xml:lang="en">Chaldeans</rdfs:label>
    </owl:NamedIndividual>
    


    <!-- http://semanticbible.org/ns/2006/NTNames#Chios -->

    <owl:NamedIndividual rdf:about="http://semanticbible.org/ns/2006/NTNames#Chios">
        <rdfs:label xml:lang="en">Chios</rdfs:label>
    </owl:NamedIndividual>
    


    <!-- http://semanticbible.org/ns/2006/NTNames#Chloe -->

    <owl:NamedIndividual rdf:about="http://semanticbible.org/ns/2006/NTNames#Chloe">
        <rdfs:label xml:lang="en">Chloe</rdfs:label>
        <rdfs:comment rdf:datatype="http://www.w3.org/2001/XMLSchema#string">&quot;Chloe&#39;s people&quot; are mentioned in 1Cor.1.11: so while they were clearly Christians who knew the church in Corinth, nothing more specific is known about her. She may have resided in Ephesus instead of Corinth. </rdfs:comment>
    </owl:NamedIndividual>
    


    <!-- http://semanticbible.org/ns/2006/NTNames#Chorazin -->

    <owl:NamedIndividual rdf:about="http://semanticbible.org/ns/2006/NTNames#Chorazin">
        <rdfs:label xml:lang="en">Chorazin</rdfs:label>
    </owl:NamedIndividual>
    


    <!-- http://semanticbible.org/ns/2006/NTNames#Christian -->

    <owl:NamedIndividual rdf:about="http://semanticbible.org/ns/2006/NTNames#Christian">
        <rdfs:label xml:lang="en">Christian</rdfs:label>
    </owl:NamedIndividual>
    


    <!-- http://semanticbible.org/ns/2006/NTNames#Christianity -->

    <owl:NamedIndividual rdf:about="http://semanticbible.org/ns/2006/NTNames#Christianity">
        <rdfs:label xml:lang="en">Christianity</rdfs:label>
        <rdfs:comment xml:lang="en">Not referenced as a belief system in the New Testament.</rdfs:comment>
    </owl:NamedIndividual>
    


    <!-- http://semanticbible.org/ns/2006/NTNames#Christians -->

    <owl:NamedIndividual rdf:about="http://semanticbible.org/ns/2006/NTNames#Christians">
        <rdfs:label xml:lang="en">Christians</rdfs:label>
    </owl:NamedIndividual>
    


    <!-- http://semanticbible.org/ns/2006/NTNames#Chuza -->

    <owl:NamedIndividual rdf:about="http://semanticbible.org/ns/2006/NTNames#Chuza">
        <rdf:type rdf:resource="http://semanticbible.org/ns/2006/NTNames#Man"/>
        <rdfs:label xml:lang="en">Chuza</rdfs:label>
        <rdfs:comment xml:lang="en">Though Chuza&#39;s wife was a devoted follower of Jesus, there&#39;s no evidence as to Chuza&#39;s belief.</rdfs:comment>
    </owl:NamedIndividual>
    


    <!-- http://semanticbible.org/ns/2006/NTNames#Cilicia -->

    <owl:NamedIndividual rdf:about="http://semanticbible.org/ns/2006/NTNames#Cilicia">
        <rdf:type rdf:resource="http://semanticbible.org/ns/2006/NTNames#StateOrProvince"/>
        <rdfs:label xml:lang="en">Cilicia</rdfs:label>
    </owl:NamedIndividual>
    


    <!-- http://semanticbible.org/ns/2006/NTNames#Claudia -->

    <owl:NamedIndividual rdf:about="http://semanticbible.org/ns/2006/NTNames#Claudia">
        <rdfs:label xml:lang="en">Claudia</rdfs:label>
        <rdfs:comment rdf:datatype="http://www.w3.org/2001/XMLSchema#string">Rome as ResidentPlace because Paul was imprisoned there when writing to Timothy.</rdfs:comment>
        <knows rdf:resource="http://semanticbible.org/ns/2006/NTNames#Paul"/>
        <knows rdf:resource="http://semanticbible.org/ns/2006/NTNames#Timothy"/>
    </owl:NamedIndividual>
    


    <!-- http://semanticbible.org/ns/2006/NTNames#Claudius -->

    <owl:NamedIndividual rdf:about="http://semanticbible.org/ns/2006/NTNames#Claudius">
        <rdfs:label xml:lang="en">Claudius</rdfs:label>
        <description rdf:datatype="http://www.w3.org/2001/XMLSchema#string">One of the emperors of Rome</description>
        <occupation rdf:datatype="http://www.w3.org/2001/XMLSchema#string">emperor</occupation>
    </owl:NamedIndividual>
    


    <!-- http://semanticbible.org/ns/2006/NTNames#ClaudiusLysias -->

    <owl:NamedIndividual rdf:about="http://semanticbible.org/ns/2006/NTNames#ClaudiusLysias">
        <rdfs:label xml:lang="en">Claudius Lysias</rdfs:label>
        <description rdf:datatype="http://www.w3.org/2001/XMLSchema#string">the military tribune commanding the Roman forces in Jerusalem</description>
        <rdfs:comment xml:lang="en">Greek ethnicity is suggested by his surname. </rdfs:comment>
        <knows rdf:resource="http://semanticbible.org/ns/2006/NTNames#Felix"/>
    </owl:NamedIndividual>
    


    <!-- http://semanticbible.org/ns/2006/NTNames#Clement -->

    <owl:NamedIndividual rdf:about="http://semanticbible.org/ns/2006/NTNames#Clement">
        <rdfs:label xml:lang="en">Clement</rdfs:label>
        <description rdf:datatype="http://www.w3.org/2001/XMLSchema#string">a companion of the Apostle Paul</description>
    </owl:NamedIndividual>
    


    <!-- http://semanticbible.org/ns/2006/NTNames#Cleopas -->

    <owl:NamedIndividual rdf:about="http://semanticbible.org/ns/2006/NTNames#Cleopas">
        <rdfs:label xml:lang="en">Cleopas</rdfs:label>
        <owl:versionInfo rdf:datatype="http://www.w3.org/2001/XMLSchema#string">TODO: Cleopas knew the 11, and the women who went to the tomb</owl:versionInfo>
        <rdfs:comment xml:lang="en">&quot;The name is a contraction of Cleopatros, not identical with Clopas of Joh 19:25.&quot; (ISBE) Jerusalem could have been his place of residence. </rdfs:comment>
        <religiousBelief rdf:resource="http://semanticbible.org/ns/2006/NTNames#Christianity"/>
    </owl:NamedIndividual>
    


    <!-- http://semanticbible.org/ns/2006/NTNames#Cnidus -->

    <owl:NamedIndividual rdf:about="http://semanticbible.org/ns/2006/NTNames#Cnidus">
        <rdfs:label xml:lang="en">Cnidus</rdfs:label>
    </owl:NamedIndividual>
    


    <!-- http://semanticbible.org/ns/2006/NTNames#CnidusGeodata -->

    <owl:NamedIndividual rdf:about="http://semanticbible.org/ns/2006/NTNames#CnidusGeodata">
        <rdfs:label xml:lang="en">geodata for Cnidus</rdfs:label>
    </owl:NamedIndividual>
    


    <!-- http://semanticbible.org/ns/2006/NTNames#Colossae -->

    <owl:NamedIndividual rdf:about="http://semanticbible.org/ns/2006/NTNames#Colossae">
        <rdfs:label xml:lang="en">Colossae</rdfs:label>
    </owl:NamedIndividual>
    


    <!-- http://semanticbible.org/ns/2006/NTNames#ColossaeGeodata -->

    <owl:NamedIndividual rdf:about="http://semanticbible.org/ns/2006/NTNames#ColossaeGeodata">
        <rdfs:label xml:lang="en">geodata for Colossae</rdfs:label>
        <longitude rdf:datatype="http://www.w3.org/2001/XMLSchema#double">29.19879351988703</longitude>
        <latitude rdf:datatype="http://www.w3.org/2001/XMLSchema#double">37.82980850278283</latitude>
    </owl:NamedIndividual>
    


    <!-- http://semanticbible.org/ns/2006/NTNames#Corinth -->

    <owl:NamedIndividual rdf:about="http://semanticbible.org/ns/2006/NTNames#Corinth">
        <rdfs:label xml:lang="en">Corinth</rdfs:label>
    </owl:NamedIndividual>
    


    <!-- http://semanticbible.org/ns/2006/NTNames#CorinthGeodata -->

    <owl:NamedIndividual rdf:about="http://semanticbible.org/ns/2006/NTNames#CorinthGeodata">
        <rdfs:label xml:lang="en">geodata for Corinth</rdfs:label>
    </owl:NamedIndividual>
    


    <!-- http://semanticbible.org/ns/2006/NTNames#Corinthians -->

    <owl:NamedIndividual rdf:about="http://semanticbible.org/ns/2006/NTNames#Corinthians">
        <rdfs:label xml:lang="en">Corinthians</rdfs:label>
    </owl:NamedIndividual>
    


    <!-- http://semanticbible.org/ns/2006/NTNames#Cornelius -->

    <owl:NamedIndividual rdf:about="http://semanticbible.org/ns/2006/NTNames#Cornelius">
        <rdfs:label xml:lang="en">Cornelius</rdfs:label>
    </owl:NamedIndividual>
    


    <!-- http://semanticbible.org/ns/2006/NTNames#Cos -->

    <owl:NamedIndividual rdf:about="http://semanticbible.org/ns/2006/NTNames#Cos">
        <rdfs:label xml:lang="en">Cos</rdfs:label>
    </owl:NamedIndividual>
    


    <!-- http://semanticbible.org/ns/2006/NTNames#CosGeodata -->

    <owl:NamedIndividual rdf:about="http://semanticbible.org/ns/2006/NTNames#CosGeodata">
        <rdfs:label xml:lang="en">geodata for Cos</rdfs:label>
        <altitude rdf:datatype="http://www.w3.org/2001/XMLSchema#int">0</altitude>
        <longitude rdf:datatype="http://www.w3.org/2001/XMLSchema#double">27.08847233780648</longitude>
    </owl:NamedIndividual>
    


    <!-- http://semanticbible.org/ns/2006/NTNames#Cosam -->

    <owl:NamedIndividual rdf:about="http://semanticbible.org/ns/2006/NTNames#Cosam">
        <rdfs:label xml:lang="en">Cosam</rdfs:label>
        <childOf rdf:resource="http://semanticbible.org/ns/2006/NTNames#Elmadam"/>
    </owl:NamedIndividual>
    


    <!-- http://semanticbible.org/ns/2006/NTNames#Crescens -->

    <owl:NamedIndividual rdf:about="http://semanticbible.org/ns/2006/NTNames#Crescens">
        <rdfs:label xml:lang="en">Crescens</rdfs:label>
        <rdfs:comment xml:lang="en">Crescens may have been from Rome originally</rdfs:comment>
    </owl:NamedIndividual>
    


    <!-- http://semanticbible.org/ns/2006/NTNames#Cretans -->

    <owl:NamedIndividual rdf:about="http://semanticbible.org/ns/2006/NTNames#Cretans">
        <rdfs:label xml:lang="en">Cretans</rdfs:label>
    </owl:NamedIndividual>
    


    <!-- http://semanticbible.org/ns/2006/NTNames#Crete -->

    <owl:NamedIndividual rdf:about="http://semanticbible.org/ns/2006/NTNames#Crete">
        <rdfs:label xml:lang="en">Crete</rdfs:label>
    </owl:NamedIndividual>
    


    <!-- http://semanticbible.org/ns/2006/NTNames#Crispus -->

    <owl:NamedIndividual rdf:about="http://semanticbible.org/ns/2006/NTNames#Crispus">
        <rdfs:label xml:lang="en">Crispus</rdfs:label>
        <rdfs:comment rdf:datatype="http://www.w3.org/2001/XMLSchema#string">As a prominent member of the church at Corinth, it seems reasonable to assume Crispus would know the other people from Corinth mentioned in the New Testament. </rdfs:comment>
    </owl:NamedIndividual>
    


    <!-- http://semanticbible.org/ns/2006/NTNames#Cyprus -->

    <owl:NamedIndividual rdf:about="http://semanticbible.org/ns/2006/NTNames#Cyprus">
        <rdfs:label xml:lang="en">Cyprus</rdfs:label>
    </owl:NamedIndividual>
    


    <!-- http://semanticbible.org/ns/2006/NTNames#Cyrene -->

    <owl:NamedIndividual rdf:about="http://semanticbible.org/ns/2006/NTNames#Cyrene">
        <rdfs:label xml:lang="en">Cyrene</rdfs:label>
    </owl:NamedIndividual>
    


    <!-- http://semanticbible.org/ns/2006/NTNames#Cyrenians -->

    <owl:NamedIndividual rdf:about="http://semanticbible.org/ns/2006/NTNames#Cyrenians">
        <rdfs:label xml:lang="en">Cyrenians</rdfs:label>
    </owl:NamedIndividual>
    


    <!-- http://semanticbible.org/ns/2006/NTNames#Dalmanutha -->

    <owl:NamedIndividual rdf:about="http://semanticbible.org/ns/2006/NTNames#Dalmanutha">
        <rdfs:label xml:lang="en">Dalmanutha</rdfs:label>
    </owl:NamedIndividual>
    


    <!-- http://semanticbible.org/ns/2006/NTNames#DalmanuthaGeodata -->

    <owl:NamedIndividual rdf:about="http://semanticbible.org/ns/2006/NTNames#DalmanuthaGeodata">
        <rdfs:label xml:lang="en">geodata for Dalmanutha</rdfs:label>
        <longitude rdf:datatype="http://www.w3.org/2001/XMLSchema#double">35.52350046026037</longitude>
    </owl:NamedIndividual>
    


    <!-- http://semanticbible.org/ns/2006/NTNames#Dalmatia -->

    <owl:NamedIndividual rdf:about="http://semanticbible.org/ns/2006/NTNames#Dalmatia">
        <rdfs:label xml:lang="en">Dalmatia</rdfs:label>
    </owl:NamedIndividual>
    


    <!-- http://semanticbible.org/ns/2006/NTNames#Damaris -->

    <owl:NamedIndividual rdf:about="http://semanticbible.org/ns/2006/NTNames#Damaris">
        <rdfs:label xml:lang="en">Damaris</rdfs:label>
        <rdfs:comment xml:lang="en">Damaris was converted through Paul&#39;s preaching in Athens.</rdfs:comment>
    </owl:NamedIndividual>
    


    <!-- http://semanticbible.org/ns/2006/NTNames#Damascus -->

    <owl:NamedIndividual rdf:about="http://semanticbible.org/ns/2006/NTNames#Damascus">
        <rdfs:label xml:lang="en">Damascus</rdfs:label>
    </owl:NamedIndividual>
    


    <!-- http://semanticbible.org/ns/2006/NTNames#Daniel -->

    <owl:NamedIndividual rdf:about="http://semanticbible.org/ns/2006/NTNames#Daniel">
        <rdfs:label xml:lang="en">Daniel</rdfs:label>
    </owl:NamedIndividual>
    


    <!-- http://semanticbible.org/ns/2006/NTNames#David -->

    <owl:NamedIndividual rdf:about="http://semanticbible.org/ns/2006/NTNames#David">
        <rdfs:label xml:lang="en">David</rdfs:label>
        <spouseOf rdf:resource="http://semanticbible.org/ns/2006/NTNames#Bathsheba"/>
    </owl:NamedIndividual>
    


    <!-- http://semanticbible.org/ns/2006/NTNames#Decapolis -->

    <owl:NamedIndividual rdf:about="http://semanticbible.org/ns/2006/NTNames#Decapolis">
        <rdfs:label xml:lang="en">Decapolis</rdfs:label>
    </owl:NamedIndividual>
    


    <!-- http://semanticbible.org/ns/2006/NTNames#Demas -->

    <owl:NamedIndividual rdf:about="http://semanticbible.org/ns/2006/NTNames#Demas">
        <rdfs:label xml:lang="en">Demas</rdfs:label>
        <rdfs:comment xml:lang="en">Though Paul describes Demas as &quot;my fellow worker&quot; in Philemon, later he apparently deserted him and went to Thessalonica. He was with Paul when he wrote his letter to  Philemon and the Colossians, but Paul&#39;s location when writing them is uncertain. </rdfs:comment>
    </owl:NamedIndividual>
    


    <!-- http://semanticbible.org/ns/2006/NTNames#Demetrius -->

    <owl:NamedIndividual rdf:about="http://semanticbible.org/ns/2006/NTNames#Demetrius">
        <rdfs:label xml:lang="en">Demetrius</rdfs:label>
        <rdfs:comment xml:lang="en">See comment on DemetriusTheSilversmith. Keener suggests that 3John is a letter of support which Demetrius carried to Gaius. </rdfs:comment>
        <collaboratesWith rdf:resource="http://semanticbible.org/ns/2006/NTNames#JohnSonOfZebedee"/>
    </owl:NamedIndividual>
    


    <!-- http://semanticbible.org/ns/2006/NTNames#DemetriusTheSilversmith -->

    <owl:NamedIndividual rdf:about="http://semanticbible.org/ns/2006/NTNames#DemetriusTheSilversmith">
        <rdfs:label xml:lang="en">Demetrius</rdfs:label>
        <description rdf:datatype="http://www.w3.org/2001/XMLSchema#string">a craftsman in Ephesus who made silver shrines of Artemis</description>
        <rdfs:comment xml:lang="en">Demetrius was a common name, so it&#39;s unlikely this man is the same as the disciple mentioned in 3John.1.12.</rdfs:comment>
    </owl:NamedIndividual>
    


    <!-- http://semanticbible.org/ns/2006/NTNames#Derbe -->

    <owl:NamedIndividual rdf:about="http://semanticbible.org/ns/2006/NTNames#Derbe">
        <rdfs:label xml:lang="en">Derbe</rdfs:label>
        <nativePlaceOf rdf:resource="http://semanticbible.org/ns/2006/NTNames#GaiusOfDerbe"/>
    </owl:NamedIndividual>
    


    <!-- http://semanticbible.org/ns/2006/NTNames#DerbeGeodata -->

    <owl:NamedIndividual rdf:about="http://semanticbible.org/ns/2006/NTNames#DerbeGeodata">
        <rdfs:label xml:lang="en">geodata for Derbe</rdfs:label>
    </owl:NamedIndividual>
    


    <!-- http://semanticbible.org/ns/2006/NTNames#Dionysius -->

    <owl:NamedIndividual rdf:about="http://semanticbible.org/ns/2006/NTNames#Dionysius">
        <rdf:type rdf:resource="http://semanticbible.org/ns/2006/NTNames#Man"/>
        <rdfs:label xml:lang="en">Dionysius</rdfs:label>
        <rdfs:comment xml:lang="en">Though nothing else is recorded about Dionysius, the exclusivity and prestige of the Areopagus makes his descriptive surname significant. </rdfs:comment>
    </owl:NamedIndividual>
    


    <!-- http://semanticbible.org/ns/2006/NTNames#Diotrephes -->

    <owl:NamedIndividual rdf:about="http://semanticbible.org/ns/2006/NTNames#Diotrephes">
        <rdfs:label xml:lang="en">Diotrephes</rdfs:label>
    </owl:NamedIndividual>
    


    <!-- http://semanticbible.org/ns/2006/NTNames#Drusilla -->

    <owl:NamedIndividual rdf:about="http://semanticbible.org/ns/2006/NTNames#Drusilla">
        <rdf:type rdf:resource="http://semanticbible.org/ns/2006/NTNames#Woman"/>
        <rdfs:label xml:lang="en">Drusilla</rdfs:label>
        <rdfs:comment rdf:datatype="http://www.w3.org/2001/XMLSchema#string">Drusilla&#39;s locations are inferred from those of her husband. According to Josephus, she was the daughter of Herod Agrippa I. </rdfs:comment>
        <siblingOf rdf:resource="http://semanticbible.org/ns/2006/NTNames#HerodAgrippaII"/>
    </owl:NamedIndividual>
    


    <!-- http://semanticbible.org/ns/2006/NTNames#Eber -->

    <owl:NamedIndividual rdf:about="http://semanticbible.org/ns/2006/NTNames#Eber">
        <rdfs:label xml:lang="en">Eber</rdfs:label>
    </owl:NamedIndividual>
    


    <!-- http://semanticbible.org/ns/2006/NTNames#Egypt -->

    <owl:NamedIndividual rdf:about="http://semanticbible.org/ns/2006/NTNames#Egypt">
        <rdfs:label xml:lang="en">Egypt</rdfs:label>
        <residentPlaceOf rdf:resource="http://semanticbible.org/ns/2006/NTNames#Mary"/>
    </owl:NamedIndividual>
    


    <!-- http://semanticbible.org/ns/2006/NTNames#Egyptian -->

    <owl:NamedIndividual rdf:about="http://semanticbible.org/ns/2006/NTNames#Egyptian">
        <rdfs:label xml:lang="en">Egyptian</rdfs:label>
        <rdfs:comment xml:lang="en">Only used in the New Testament to refer to those whose place of birth is Egypt. </rdfs:comment>
    </owl:NamedIndividual>
    


    <!-- http://semanticbible.org/ns/2006/NTNames#Egyptians -->

    <owl:NamedIndividual rdf:about="http://semanticbible.org/ns/2006/NTNames#Egyptians">
        <rdfs:label xml:lang="en">Egyptians</rdfs:label>
    </owl:NamedIndividual>
    


    <!-- http://semanticbible.org/ns/2006/NTNames#Elamites -->

    <owl:NamedIndividual rdf:about="http://semanticbible.org/ns/2006/NTNames#Elamites">
        <rdfs:label xml:lang="en">Elamites</rdfs:label>
    </owl:NamedIndividual>
    


    <!-- http://semanticbible.org/ns/2006/NTNames#Eleazar -->

    <owl:NamedIndividual rdf:about="http://semanticbible.org/ns/2006/NTNames#Eleazar">
        <rdfs:label xml:lang="en">Eleazar</rdfs:label>
        <ethnicity rdf:resource="http://semanticbible.org/ns/2006/NTNames#Jewish"/>
    </owl:NamedIndividual>
    


    <!-- http://semanticbible.org/ns/2006/NTNames#EliakimSonOfAbiud -->

    <owl:NamedIndividual rdf:about="http://semanticbible.org/ns/2006/NTNames#EliakimSonOfAbiud">
        <rdfs:label xml:lang="en">Eliakim</rdfs:label>
    </owl:NamedIndividual>
    


    <!-- http://semanticbible.org/ns/2006/NTNames#EliakimSonOfMelea -->

    <owl:NamedIndividual rdf:about="http://semanticbible.org/ns/2006/NTNames#EliakimSonOfMelea">
        <rdfs:label xml:lang="en">Eliakim</rdfs:label>
    </owl:NamedIndividual>
    


    <!-- http://semanticbible.org/ns/2006/NTNames#Eliezer -->

    <owl:NamedIndividual rdf:about="http://semanticbible.org/ns/2006/NTNames#Eliezer">
        <rdfs:label xml:lang="en">Eliezer</rdfs:label>
    </owl:NamedIndividual>
    


    <!-- http://semanticbible.org/ns/2006/NTNames#Elijah -->

    <owl:NamedIndividual rdf:about="http://semanticbible.org/ns/2006/NTNames#Elijah">
        <rdf:type rdf:resource="http://semanticbible.org/ns/2006/NTNames#Man"/>
        <rdfs:label xml:lang="en">Elijah</rdfs:label>
        <rdfs:comment xml:lang="en">John the Baptist represented Elijah returned to his contemporaries, and the name is sometimes therefore used to refer to John (e.g. Matt.17.12).</rdfs:comment>
    </owl:NamedIndividual>
    


    <!-- http://semanticbible.org/ns/2006/NTNames#Elisha -->

    <owl:NamedIndividual rdf:about="http://semanticbible.org/ns/2006/NTNames#Elisha">
        <rdfs:label xml:lang="en">Elisha</rdfs:label>
    </owl:NamedIndividual>
    


    <!-- http://semanticbible.org/ns/2006/NTNames#Eliud -->

    <owl:NamedIndividual rdf:about="http://semanticbible.org/ns/2006/NTNames#Eliud">
        <rdfs:label xml:lang="en">Eliud</rdfs:label>
        <ethnicity rdf:resource="http://semanticbible.org/ns/2006/NTNames#Jewish"/>
    </owl:NamedIndividual>
    


    <!-- http://semanticbible.org/ns/2006/NTNames#Elizabeth -->

    <owl:NamedIndividual rdf:about="http://semanticbible.org/ns/2006/NTNames#Elizabeth">
        <rdfs:label xml:lang="en">Elizabeth</rdfs:label>
        <rdfs:comment xml:lang="en">Elizabeth was a kinswoman to Mary the mother of Jesus. Luke&#39;s gospel records that Mary visited her in a town in Judah, and that she was &quot;of the daughters of Aaron&quot;.</rdfs:comment>
    </owl:NamedIndividual>
    


    <!-- http://semanticbible.org/ns/2006/NTNames#Elmadam -->

    <owl:NamedIndividual rdf:about="http://semanticbible.org/ns/2006/NTNames#Elmadam">
        <rdfs:label xml:lang="en">Elmadam</rdfs:label>
        <hasOnlyGenealogyMention rdf:datatype="http://www.w3.org/2001/XMLSchema#boolean">true</hasOnlyGenealogyMention>
    </owl:NamedIndividual>
    


    <!-- http://semanticbible.org/ns/2006/NTNames#Emmaus -->

    <owl:NamedIndividual rdf:about="http://semanticbible.org/ns/2006/NTNames#Emmaus">
        <rdfs:label xml:lang="en">Emmaus</rdfs:label>
        <rdfs:comment xml:lang="en">Emmaus is a village about seven miles from Jerusalem. Jesus joined two disciples who were walking here, though they did not recognize Him until the end of the journey. </rdfs:comment>
    </owl:NamedIndividual>
    


    <!-- http://semanticbible.org/ns/2006/NTNames#EmmausGeodata -->

    <owl:NamedIndividual rdf:about="http://semanticbible.org/ns/2006/NTNames#EmmausGeodata">
        <rdfs:label xml:lang="en">geodata for Emmaus</rdfs:label>
        <longitude rdf:datatype="http://www.w3.org/2001/XMLSchema#double">34.99550449459134</longitude>
    </owl:NamedIndividual>
    


    <!-- http://semanticbible.org/ns/2006/NTNames#Enoch -->

    <owl:NamedIndividual rdf:about="http://semanticbible.org/ns/2006/NTNames#Enoch">
        <rdfs:label xml:lang="en">Enoch</rdfs:label>
        <rdfs:comment xml:lang="en">Different from the eldest son of Cain (Gen.4:17)</rdfs:comment>
    </owl:NamedIndividual>
    


    <!-- http://semanticbible.org/ns/2006/NTNames#Enos -->

    <owl:NamedIndividual rdf:about="http://semanticbible.org/ns/2006/NTNames#Enos">
        <rdfs:label xml:lang="en">Enos</rdfs:label>
        <rdfs:comment xml:lang="en">Enosh in the NIV</rdfs:comment>
    </owl:NamedIndividual>
    


    <!-- http://semanticbible.org/ns/2006/NTNames#Epaenetus -->

    <owl:NamedIndividual rdf:about="http://semanticbible.org/ns/2006/NTNames#Epaenetus">
        <rdfs:label xml:lang="en">Epaenetus</rdfs:label>
    </owl:NamedIndividual>
    


    <!-- http://semanticbible.org/ns/2006/NTNames#Epaphras -->

    <owl:NamedIndividual rdf:about="http://semanticbible.org/ns/2006/NTNames#Epaphras">
        <rdf:type rdf:resource="http://semanticbible.org/ns/2006/NTNames#Man"/>
        <rdfs:label xml:lang="en">Epaphras</rdfs:label>
        <rdfs:comment xml:lang="en">Paul mentions that Epaphras &quot;worked hard&quot; for those in Laodicea and Hierapolis, so it&#39;s possible (but not certain) he visited there as well. </rdfs:comment>
    </owl:NamedIndividual>
    


    <!-- http://semanticbible.org/ns/2006/NTNames#Epaphroditus -->

    <owl:NamedIndividual rdf:about="http://semanticbible.org/ns/2006/NTNames#Epaphroditus">
        <rdfs:label xml:lang="en">Epaphroditus</rdfs:label>
        <rdfs:comment xml:lang="en">Though Epaphras is a contraction of Epaphroditus, this individual is distinct from the Epaphras mentioned in Colossians and Philemon.
Rome as a visitedPlace assumes Paul was there while writing Philippians. </rdfs:comment>
    </owl:NamedIndividual>
    


    <!-- http://semanticbible.org/ns/2006/NTNames#Ephesian -->

    <owl:NamedIndividual rdf:about="http://semanticbible.org/ns/2006/NTNames#Ephesian">
        <rdfs:label xml:lang="en">Ephesian</rdfs:label>
    </owl:NamedIndividual>
    


    <!-- http://semanticbible.org/ns/2006/NTNames#Ephesians -->

    <owl:NamedIndividual rdf:about="http://semanticbible.org/ns/2006/NTNames#Ephesians">
        <rdfs:label xml:lang="en">Ephesians</rdfs:label>
    </owl:NamedIndividual>
    


    <!-- http://semanticbible.org/ns/2006/NTNames#Ephesus -->

    <owl:NamedIndividual rdf:about="http://semanticbible.org/ns/2006/NTNames#Ephesus">
        <rdfs:label xml:lang="en">Ephesus</rdfs:label>
        <residentPlaceOf rdf:resource="http://semanticbible.org/ns/2006/NTNames#Paul"/>
    </owl:NamedIndividual>
    


    <!-- http://semanticbible.org/ns/2006/NTNames#EphesusGeodata -->

    <owl:NamedIndividual rdf:about="http://semanticbible.org/ns/2006/NTNames#EphesusGeodata">
        <rdf:type rdf:resource="http://semanticbible.org/ns/2006/NTNames#GeographicLocation"/>
        <rdfs:label xml:lang="en">geodata for Ephesus</rdfs:label>
    </owl:NamedIndividual>
    


    <!-- http://semanticbible.org/ns/2006/NTNames#Ephraim -->

    <owl:NamedIndividual rdf:about="http://semanticbible.org/ns/2006/NTNames#Ephraim">
        <rdfs:label xml:lang="en">Ephraim</rdfs:label>
        <rdfs:comment xml:lang="en">Jesus retreated to this town with his disciples when the Jews plotted to kill him after Lazarus was raised from the dead.</rdfs:comment>
        <subregionOf rdf:resource="http://semanticbible.org/ns/2006/NTNames#Judea"/>
    </owl:NamedIndividual>
    


    <!-- http://semanticbible.org/ns/2006/NTNames#EphraimGeodata -->

    <owl:NamedIndividual rdf:about="http://semanticbible.org/ns/2006/NTNames#EphraimGeodata">
        <rdfs:label xml:lang="en">geodata for Ephraim</rdfs:label>
    </owl:NamedIndividual>
    


    <!-- http://semanticbible.org/ns/2006/NTNames#Epicurean -->

    <owl:NamedIndividual rdf:about="http://semanticbible.org/ns/2006/NTNames#Epicurean">
        <rdfs:label xml:lang="en">Epicurean</rdfs:label>
    </owl:NamedIndividual>
    


    <!-- http://semanticbible.org/ns/2006/NTNames#Er -->

    <owl:NamedIndividual rdf:about="http://semanticbible.org/ns/2006/NTNames#Er">
        <rdfs:label xml:lang="en">Er</rdfs:label>
        <description rdf:datatype="http://www.w3.org/2001/XMLSchema#string">One of the ancestors of Jesus mentioned in Luke&#39;s geneaology</description>
    </owl:NamedIndividual>
    


    <!-- http://semanticbible.org/ns/2006/NTNames#Erastus -->

    <owl:NamedIndividual rdf:about="http://semanticbible.org/ns/2006/NTNames#Erastus">
        <rdfs:label xml:lang="en">Erastus</rdfs:label>
        <rdfs:comment xml:lang="en">There are two references to this Erastus: it&#39;s possible they represent two different people. See also the comment on ErastusTheTreasurer.	</rdfs:comment>
        <visitedPlace rdf:resource="http://semanticbible.org/ns/2006/NTNames#Ephesus"/>
    </owl:NamedIndividual>
    


    <!-- http://semanticbible.org/ns/2006/NTNames#ErastusTheTreasurer -->

    <owl:NamedIndividual rdf:about="http://semanticbible.org/ns/2006/NTNames#ErastusTheTreasurer">
        <rdfs:label rdf:datatype="http://www.w3.org/2001/XMLSchema#string">Erastus the city treasurer</rdfs:label>
        <rdfs:comment rdf:datatype="http://www.w3.org/2001/XMLSchema#string">It is uncertain whether this Erastus is the same as Paul&#39;s travelling companion and fellow minister, though possible. </rdfs:comment>
    </owl:NamedIndividual>
    


    <!-- http://semanticbible.org/ns/2006/NTNames#Esau -->

    <owl:NamedIndividual rdf:about="http://semanticbible.org/ns/2006/NTNames#Esau">
        <rdfs:label xml:lang="en">Esau</rdfs:label>
    </owl:NamedIndividual>
    


    <!-- http://semanticbible.org/ns/2006/NTNames#Esli -->

    <owl:NamedIndividual rdf:about="http://semanticbible.org/ns/2006/NTNames#Esli">
        <rdfs:label xml:lang="en">Esli</rdfs:label>
    </owl:NamedIndividual>
    


    <!-- http://semanticbible.org/ns/2006/NTNames#Ethiopia -->

    <owl:NamedIndividual rdf:about="http://semanticbible.org/ns/2006/NTNames#Ethiopia">
        <rdfs:comment xml:lang="en">Not named in the New Testament.</rdfs:comment>
    </owl:NamedIndividual>
    


    <!-- http://semanticbible.org/ns/2006/NTNames#Ethiopian -->

    <owl:NamedIndividual rdf:about="http://semanticbible.org/ns/2006/NTNames#Ethiopian">
        <rdfs:label xml:lang="en">Ethiopian</rdfs:label>
        <rdfs:comment xml:lang="en">Of the country of Ethiopia. </rdfs:comment>
    </owl:NamedIndividual>
    


    <!-- http://semanticbible.org/ns/2006/NTNames#Ethiopians -->

    <owl:NamedIndividual rdf:about="http://semanticbible.org/ns/2006/NTNames#Ethiopians">
        <rdfs:label xml:lang="en">Ethiopians</rdfs:label>
    </owl:NamedIndividual>
    


    <!-- http://semanticbible.org/ns/2006/NTNames#Eubulus -->

    <owl:NamedIndividual rdf:about="http://semanticbible.org/ns/2006/NTNames#Eubulus">
        <rdfs:label xml:lang="en">Eubulus</rdfs:label>
        <rdfs:comment rdf:datatype="http://www.w3.org/2001/XMLSchema#string">His residence in Rome assumes </rdfs:comment>
    </owl:NamedIndividual>
    


    <!-- http://semanticbible.org/ns/2006/NTNames#Eunice -->

    <owl:NamedIndividual rdf:about="http://semanticbible.org/ns/2006/NTNames#Eunice">
        <rdfs:label xml:lang="en">Eunice</rdfs:label>
        <rdfs:comment xml:lang="en">Eunice&#39;s residence in Lystra is implied by Acts.16.1, though Derbe is also possible. Her Christian faith is strongly implied by Paul&#39;s commendation of it in 2Tim.1.5. </rdfs:comment>
    </owl:NamedIndividual>
    


    <!-- http://semanticbible.org/ns/2006/NTNames#Euodia -->

    <owl:NamedIndividual rdf:about="http://semanticbible.org/ns/2006/NTNames#Euodia">
        <rdfs:label xml:lang="en">Euodia</rdfs:label>
    </owl:NamedIndividual>
    


    <!-- http://semanticbible.org/ns/2006/NTNames#Euphrates -->

    <owl:NamedIndividual rdf:about="http://semanticbible.org/ns/2006/NTNames#Euphrates">
        <rdfs:label xml:lang="en">Euphrates</rdfs:label>
    </owl:NamedIndividual>
    


    <!-- http://semanticbible.org/ns/2006/NTNames#Eutychus -->

    <owl:NamedIndividual rdf:about="http://semanticbible.org/ns/2006/NTNames#Eutychus">
        <rdfs:label xml:lang="en">Eutychus</rdfs:label>
        <residentPlace rdf:resource="http://semanticbible.org/ns/2006/NTNames#Troas"/>
    </owl:NamedIndividual>
    


    <!-- http://semanticbible.org/ns/2006/NTNames#Eve -->

    <owl:NamedIndividual rdf:about="http://semanticbible.org/ns/2006/NTNames#Eve">
        <rdfs:label xml:lang="en">Eve</rdfs:label>
    </owl:NamedIndividual>
    


    <!-- http://semanticbible.org/ns/2006/NTNames#FairHavens -->

    <owl:NamedIndividual rdf:about="http://semanticbible.org/ns/2006/NTNames#FairHavens">
        <rdfs:label xml:lang="en">Fair Havens</rdfs:label>
    </owl:NamedIndividual>
    


    <!-- http://semanticbible.org/ns/2006/NTNames#FairHavensGeodata -->

    <owl:NamedIndividual rdf:about="http://semanticbible.org/ns/2006/NTNames#FairHavensGeodata">
        <rdfs:label xml:lang="en">geodata for Fair Havens</rdfs:label>
        <longitude rdf:datatype="http://www.w3.org/2001/XMLSchema#double">24.73534424651286</longitude>
    </owl:NamedIndividual>
    


    <!-- http://semanticbible.org/ns/2006/NTNames#Felix -->

    <owl:NamedIndividual rdf:about="http://semanticbible.org/ns/2006/NTNames#Felix">
        <rdfs:label xml:lang="en">Felix</rdfs:label>
        <rdfs:comment rdf:datatype="http://www.w3.org/2001/XMLSchema#string">Properly Antonius Felix</rdfs:comment>
        <hasOnlyGenealogyMention rdf:datatype="http://www.w3.org/2001/XMLSchema#boolean">false</hasOnlyGenealogyMention>
        <residentPlace rdf:resource="http://semanticbible.org/ns/2006/NTNames#Caesarea"/>
    </owl:NamedIndividual>
    


    <!-- http://semanticbible.org/ns/2006/NTNames#Festus -->

    <owl:NamedIndividual rdf:about="http://semanticbible.org/ns/2006/NTNames#Festus">
        <rdfs:label xml:lang="en">Festus</rdfs:label>
    </owl:NamedIndividual>
    


    <!-- http://semanticbible.org/ns/2006/NTNames#Fortunatus -->

    <owl:NamedIndividual rdf:about="http://semanticbible.org/ns/2006/NTNames#Fortunatus">
        <rdfs:label xml:lang="en">Fortunatus</rdfs:label>
        <rdfs:comment rdf:datatype="http://www.w3.org/2001/XMLSchema#string">His residence in Corinth and visit to Ephesus follow from Paul&#39;s statement in 1Cor.16.17, and the assumption that Paul was in Ephesus when he wrote 1 Corinthians. </rdfs:comment>
    </owl:NamedIndividual>
    


    <!-- http://semanticbible.org/ns/2006/NTNames#Freedmen -->

    <owl:NamedIndividual rdf:about="http://semanticbible.org/ns/2006/NTNames#Freedmen">
        <rdfs:label xml:lang="en">Freedmen</rdfs:label>
    </owl:NamedIndividual>
    


    <!-- http://semanticbible.org/ns/2006/NTNames#Gabbatha -->

    <owl:NamedIndividual rdf:about="http://semanticbible.org/ns/2006/NTNames#Gabbatha">
        <rdfs:label xml:lang="en">Gabbatha</rdfs:label>
    </owl:NamedIndividual>
    


    <!-- http://semanticbible.org/ns/2006/NTNames#Gabriel -->

    <owl:NamedIndividual rdf:about="http://semanticbible.org/ns/2006/NTNames#Gabriel">
        <rdfs:label xml:lang="en">Gabriel</rdfs:label>
    </owl:NamedIndividual>
    


    <!-- http://semanticbible.org/ns/2006/NTNames#Gad -->

    <owl:NamedIndividual rdf:about="http://semanticbible.org/ns/2006/NTNames#Gad">
        <rdfs:label xml:lang="en">Gad</rdfs:label>
        <rdfs:comment rdf:datatype="http://www.w3.org/2001/XMLSchema#string">His mother Zilpah, Leah&#39;s servant, is not named in the New Testament. </rdfs:comment>
        <description rdf:datatype="http://www.w3.org/2001/XMLSchema#string">One of the 12 Patriarchs of Israel</description>
        <siblingOf rdf:resource="http://semanticbible.org/ns/2006/NTNames#Asher"/>
        <siblingOf rdf:resource="http://semanticbible.org/ns/2006/NTNames#Judah"/>
    </owl:NamedIndividual>
    


    <!-- http://semanticbible.org/ns/2006/NTNames#Gadara -->

    <owl:NamedIndividual rdf:about="http://semanticbible.org/ns/2006/NTNames#Gadara">
        <rdf:type rdf:resource="http://semanticbible.org/ns/2006/NTNames#City"/>
        <rdfs:label xml:lang="en">Gadara</rdfs:label>
        <rdfs:comment rdf:datatype="http://www.w3.org/2001/XMLSchema#string">City southeast of the Sea of Galilee. Not mentioned in Scripture as such, but &quot;the country of the Gadarenes&quot; (Matt 8.28) takes its name from this city. 
Part of the Decapolis.</rdfs:comment>
    </owl:NamedIndividual>
    


    <!-- http://semanticbible.org/ns/2006/NTNames#Gadarenes -->

    <owl:NamedIndividual rdf:about="http://semanticbible.org/ns/2006/NTNames#Gadarenes">
        <rdfs:label xml:lang="en">Gadarenes</rdfs:label>
    </owl:NamedIndividual>
    


    <!-- http://semanticbible.org/ns/2006/NTNames#GaiusOfCorinth -->

    <owl:NamedIndividual rdf:about="http://semanticbible.org/ns/2006/NTNames#GaiusOfCorinth">
        <rdfs:label xml:lang="en">Gaius</rdfs:label>
        <hasOnlyGenealogyMention rdf:datatype="http://www.w3.org/2001/XMLSchema#boolean">false</hasOnlyGenealogyMention>
        <rdfs:comment xml:lang="en">Since Paul&#39;s Epistle to the Romans was written from Corinth, this is assumed to be the one Paul describes as &quot;host to me and the whole church&quot;</rdfs:comment>
    </owl:NamedIndividual>
    


    <!-- http://semanticbible.org/ns/2006/NTNames#GaiusOfDerbe -->

    <owl:NamedIndividual rdf:about="http://semanticbible.org/ns/2006/NTNames#GaiusOfDerbe">
        <rdfs:label xml:lang="en">Gaius</rdfs:label>
        <rdfs:comment rdf:datatype="http://www.w3.org/2001/XMLSchema#string">Luke describes him as &quot;Gaius of Derbe&quot;: that could be either his place of birth, or place of residence. It&#39;s not clear whether he (and his other companions) accompanied Paul all the way to Jerusalem. Gaius being a common name, it seems plausible that the others of the same name are distinct individuals, though the closest possible identification is with GaiusOfMacedonia (see New Bible Dictionary for discussion).</rdfs:comment>
        <description rdf:datatype="http://www.w3.org/2001/XMLSchema#string">a travelling companion of Paul&#39;s</description>
    </owl:NamedIndividual>
    


    <!-- http://semanticbible.org/ns/2006/NTNames#GaiusOfMacedonia -->

    <owl:NamedIndividual rdf:about="http://semanticbible.org/ns/2006/NTNames#GaiusOfMacedonia">
        <rdfs:label xml:lang="en">Gaius</rdfs:label>
        <rdfs:comment xml:lang="en">It seems likely this Gaius was a Christian since he was Paul&#39;s &quot;companion in travel&quot;, though this is not explicitly stated. </rdfs:comment>
    </owl:NamedIndividual>
    


    <!-- http://semanticbible.org/ns/2006/NTNames#GaiusTheBeloved -->

    <owl:NamedIndividual rdf:about="http://semanticbible.org/ns/2006/NTNames#GaiusTheBeloved">
        <rdf:type rdf:resource="http://semanticbible.org/ns/2006/NTNames#Man"/>
        <rdfs:label xml:lang="en">Gaius</rdfs:label>
        <hasOnlyGenealogyMention rdf:datatype="http://www.w3.org/2001/XMLSchema#boolean">false</hasOnlyGenealogyMention>
    </owl:NamedIndividual>
    


    <!-- http://semanticbible.org/ns/2006/NTNames#Galatia -->

    <owl:NamedIndividual rdf:about="http://semanticbible.org/ns/2006/NTNames#Galatia">
        <rdfs:label xml:lang="en">Galatia</rdfs:label>
    </owl:NamedIndividual>
    


    <!-- http://semanticbible.org/ns/2006/NTNames#Galatians -->

    <owl:NamedIndividual rdf:about="http://semanticbible.org/ns/2006/NTNames#Galatians">
        <rdfs:label xml:lang="en">Galatians</rdfs:label>
    </owl:NamedIndividual>
    


    <!-- http://semanticbible.org/ns/2006/NTNames#Galilean -->

    <owl:NamedIndividual rdf:about="http://semanticbible.org/ns/2006/NTNames#Galilean">
        <rdfs:label xml:lang="en">Galilean</rdfs:label>
        <rdfs:comment xml:lang="en">In the time of Christ, Galilee was home to those of Jewish descent as well non-Jews. As used in the New Testament, the term is used primarily of Jews in distinction to Judean and Samaritan, the other major divisions of Jewish Palestine. It is therefore (in practice) a sub-ethnicity of Jewish.</rdfs:comment>
    </owl:NamedIndividual>
    


    <!-- http://semanticbible.org/ns/2006/NTNames#Galileans -->

    <owl:NamedIndividual rdf:about="http://semanticbible.org/ns/2006/NTNames#Galileans">
        <rdfs:label xml:lang="en">Galileans</rdfs:label>
    </owl:NamedIndividual>
    


    <!-- http://semanticbible.org/ns/2006/NTNames#Galilee -->

    <owl:NamedIndividual rdf:about="http://semanticbible.org/ns/2006/NTNames#Galilee">
        <rdfs:label xml:lang="en">Galilee</rdfs:label>
        <subregion rdf:resource="http://semanticbible.org/ns/2006/NTNames#Capernaum"/>
    </owl:NamedIndividual>
    


    <!-- http://semanticbible.org/ns/2006/NTNames#Gallio -->

    <owl:NamedIndividual rdf:about="http://semanticbible.org/ns/2006/NTNames#Gallio">
        <rdfs:label xml:lang="en">Gallio</rdfs:label>
        <rdfs:comment rdf:datatype="http://www.w3.org/2001/XMLSchema#string">He is not considered an antagonist of Paul because his only involvement was indifference. </rdfs:comment>
    </owl:NamedIndividual>
    


    <!-- http://semanticbible.org/ns/2006/NTNames#Gamaliel -->

    <owl:NamedIndividual rdf:about="http://semanticbible.org/ns/2006/NTNames#Gamaliel">
        <rdfs:label xml:lang="en">Gamaliel</rdfs:label>
    </owl:NamedIndividual>
    


    <!-- http://semanticbible.org/ns/2006/NTNames#Gaza -->

    <owl:NamedIndividual rdf:about="http://semanticbible.org/ns/2006/NTNames#Gaza">
        <rdfs:label xml:lang="en">Gaza</rdfs:label>
    </owl:NamedIndividual>
    


    <!-- http://semanticbible.org/ns/2006/NTNames#GazaGeodata -->

    <owl:NamedIndividual rdf:about="http://semanticbible.org/ns/2006/NTNames#GazaGeodata">
        <rdfs:label xml:lang="en">geodata for Gaza</rdfs:label>
        <latitude rdf:datatype="http://www.w3.org/2001/XMLSchema#double">31.52900696298234</latitude>
        <longitude rdf:datatype="http://www.w3.org/2001/XMLSchema#double">34.43673180421263</longitude>
    </owl:NamedIndividual>
    


    <!-- http://semanticbible.org/ns/2006/NTNames#Gennesaret -->

    <owl:NamedIndividual rdf:about="http://semanticbible.org/ns/2006/NTNames#Gennesaret">
        <rdfs:label xml:lang="en">Gennesaret</rdfs:label>
        <rdfs:comment xml:lang="en">An area on the west side of the Sea of Galilee, where Jesus healed the sick</rdfs:comment>
    </owl:NamedIndividual>
    


    <!-- http://semanticbible.org/ns/2006/NTNames#Gentile -->

    <owl:NamedIndividual rdf:about="http://semanticbible.org/ns/2006/NTNames#Gentile">
        <rdfs:label xml:lang="en">Gentile</rdfs:label>
        <rdfs:comment xml:lang="en">Essentially a &quot;non-ethnicity&quot; meaning not Jewish.</rdfs:comment>
    </owl:NamedIndividual>
    


    <!-- http://semanticbible.org/ns/2006/NTNames#Gentiles -->

    <owl:NamedIndividual rdf:about="http://semanticbible.org/ns/2006/NTNames#Gentiles">
        <rdfs:label xml:lang="en">Gentiles</rdfs:label>
    </owl:NamedIndividual>
    


    <!-- http://semanticbible.org/ns/2006/NTNames#Gethsemane -->

    <owl:NamedIndividual rdf:about="http://semanticbible.org/ns/2006/NTNames#Gethsemane">
        <rdfs:label xml:lang="en">Gethsemane</rdfs:label>
    </owl:NamedIndividual>
    


    <!-- http://semanticbible.org/ns/2006/NTNames#Gideon -->

    <owl:NamedIndividual rdf:about="http://semanticbible.org/ns/2006/NTNames#Gideon">
        <rdfs:label xml:lang="en">Gideon</rdfs:label>
    </owl:NamedIndividual>
    


    <!-- http://semanticbible.org/ns/2006/NTNames#Gog -->

    <owl:NamedIndividual rdf:about="http://semanticbible.org/ns/2006/NTNames#Gog">
        <rdfs:label xml:lang="en">Gog</rdfs:label>
        <rdfs:comment xml:lang="en">The historic background of the reference to Gog is most likely the Lydian king in the 7th Century BC. Its usage in Revelation seems to describe a group of people,  but it is hard to be certain what is intended in this apocalyptic context.</rdfs:comment>
    </owl:NamedIndividual>
    


    <!-- http://semanticbible.org/ns/2006/NTNames#Golgotha -->

    <owl:NamedIndividual rdf:about="http://semanticbible.org/ns/2006/NTNames#Golgotha">
        <rdfs:label xml:lang="en">Golgotha</rdfs:label>
    </owl:NamedIndividual>
    


    <!-- http://semanticbible.org/ns/2006/NTNames#Gomorrah -->

    <owl:NamedIndividual rdf:about="http://semanticbible.org/ns/2006/NTNames#Gomorrah">
        <rdfs:label xml:lang="en">Gomorrah</rdfs:label>
    </owl:NamedIndividual>
    


    <!-- http://semanticbible.org/ns/2006/NTNames#GomorrahGeodata -->

    <owl:NamedIndividual rdf:about="http://semanticbible.org/ns/2006/NTNames#GomorrahGeodata">
        <rdf:type rdf:resource="http://semanticbible.org/ns/2006/NTNames#GeographicLocation"/>
        <rdfs:label xml:lang="en">geodata for Gomorrah</rdfs:label>
    </owl:NamedIndividual>
    


    <!-- http://semanticbible.org/ns/2006/NTNames#Greece -->

    <owl:NamedIndividual rdf:about="http://semanticbible.org/ns/2006/NTNames#Greece">
        <rdfs:label xml:lang="en">Greece</rdfs:label>
    </owl:NamedIndividual>
    


    <!-- http://semanticbible.org/ns/2006/NTNames#Greek -->

    <owl:NamedIndividual rdf:about="http://semanticbible.org/ns/2006/NTNames#Greek">
        <rdfs:label xml:lang="en">Greek</rdfs:label>
        <rdfs:comment xml:lang="en">Sometimes used synomymously with Gentile, but certainly means non-Jewish in ethnicity.</rdfs:comment>
        <ethnicityOf rdf:resource="http://semanticbible.org/ns/2006/NTNames#Titius"/>
    </owl:NamedIndividual>
    


    <!-- http://semanticbible.org/ns/2006/NTNames#GreekLanguage -->

    <owl:NamedIndividual rdf:about="http://semanticbible.org/ns/2006/NTNames#GreekLanguage">
        <rdfs:label xml:lang="en">Greek</rdfs:label>
    </owl:NamedIndividual>
    


    <!-- http://semanticbible.org/ns/2006/NTNames#Greeks -->

    <owl:NamedIndividual rdf:about="http://semanticbible.org/ns/2006/NTNames#Greeks">
        <rdfs:label xml:lang="en">Greeks</rdfs:label>
    </owl:NamedIndividual>
    


    <!-- http://semanticbible.org/ns/2006/NTNames#Hades -->

    <owl:NamedIndividual rdf:about="http://semanticbible.org/ns/2006/NTNames#Hades">
        <rdfs:label xml:lang="en">Hades</rdfs:label>
        <rdfs:comment xml:lang="en">The state or place of the dead. SUO restricts use of GeographicArea to places on the earth.</rdfs:comment>
    </owl:NamedIndividual>
    


    <!-- http://semanticbible.org/ns/2006/NTNames#Hagar -->

    <owl:NamedIndividual rdf:about="http://semanticbible.org/ns/2006/NTNames#Hagar">
        <rdf:type rdf:resource="http://semanticbible.org/ns/2006/NTNames#Woman"/>
        <rdfs:label xml:lang="en">Hagar</rdfs:label>
        <hasOnlyGenealogyMention rdf:datatype="http://www.w3.org/2001/XMLSchema#boolean">false</hasOnlyGenealogyMention>
        <rdfs:comment rdf:datatype="http://www.w3.org/2001/XMLSchema#string">her son Ishmael is not named in the New Testament</rdfs:comment>
    </owl:NamedIndividual>
    


    <!-- http://semanticbible.org/ns/2006/NTNames#Hamor -->

    <owl:NamedIndividual rdf:about="http://semanticbible.org/ns/2006/NTNames#Hamor">
        <rdfs:label xml:lang="en">Hamor</rdfs:label>
    </owl:NamedIndividual>
    


    <!-- http://semanticbible.org/ns/2006/NTNames#Haran -->

    <owl:NamedIndividual rdf:about="http://semanticbible.org/ns/2006/NTNames#Haran">
        <rdfs:label xml:lang="en">Haran</rdfs:label>
        <rdfs:comment xml:lang="en">In his speech before the Council, Stephen refers to Haran as a place where Abraham lived. </rdfs:comment>
    </owl:NamedIndividual>
    


    <!-- http://semanticbible.org/ns/2006/NTNames#HaranGeodata -->

    <owl:NamedIndividual rdf:about="http://semanticbible.org/ns/2006/NTNames#HaranGeodata">
        <rdfs:label xml:lang="en">geodata for Haran</rdfs:label>
    </owl:NamedIndividual>
    


    <!-- http://semanticbible.org/ns/2006/NTNames#Hebrew -->

    <owl:NamedIndividual rdf:about="http://semanticbible.org/ns/2006/NTNames#Hebrew">
        <rdfs:label xml:lang="en">Hebrew</rdfs:label>
    </owl:NamedIndividual>
    


    <!-- http://semanticbible.org/ns/2006/NTNames#Hebrews -->

    <owl:NamedIndividual rdf:about="http://semanticbible.org/ns/2006/NTNames#Hebrews">
        <rdfs:label xml:lang="en">Hebrews</rdfs:label>
    </owl:NamedIndividual>
    


    <!-- http://semanticbible.org/ns/2006/NTNames#Heli -->

    <owl:NamedIndividual rdf:about="http://semanticbible.org/ns/2006/NTNames#Heli">
        <rdfs:label xml:lang="en">Heli</rdfs:label>
        <rdfs:comment xml:lang="en">See the comment on Joseph for why Heli is listed as parentOf Mary, not Joseph, despite Luke 3:23.</rdfs:comment>
    </owl:NamedIndividual>
    


    <!-- http://semanticbible.org/ns/2006/NTNames#Hellenists -->

    <owl:NamedIndividual rdf:about="http://semanticbible.org/ns/2006/NTNames#Hellenists">
        <rdfs:label xml:lang="en">Hellenists</rdfs:label>
    </owl:NamedIndividual>
    


    <!-- http://semanticbible.org/ns/2006/NTNames#Hermas -->

    <owl:NamedIndividual rdf:about="http://semanticbible.org/ns/2006/NTNames#Hermas">
        <rdfs:label xml:lang="en">Hermas</rdfs:label>
        <description rdf:datatype="http://www.w3.org/2001/XMLSchema#string">a Roman to whom Paul sent greetings</description>
    </owl:NamedIndividual>
    


    <!-- http://semanticbible.org/ns/2006/NTNames#Hermes -->

    <owl:NamedIndividual rdf:about="http://semanticbible.org/ns/2006/NTNames#Hermes">
        <rdfs:label xml:lang="en">Hermes</rdfs:label>
        <hasOnlyGenealogyMention rdf:datatype="http://www.w3.org/2001/XMLSchema#boolean">false</hasOnlyGenealogyMention>
    </owl:NamedIndividual>
    


    <!-- http://semanticbible.org/ns/2006/NTNames#Hermogenes -->

    <owl:NamedIndividual rdf:about="http://semanticbible.org/ns/2006/NTNames#Hermogenes">
        <rdfs:label xml:lang="en">Hermogenes</rdfs:label>
        <hasOnlyGenealogyMention rdf:datatype="http://www.w3.org/2001/XMLSchema#boolean">false</hasOnlyGenealogyMention>
        <rdfs:comment xml:lang="en">The circumstances behind his &quot;turning away&quot; from Paul are unknown. Likewise, Paul&#39;s description of him as being &quot;is Asia&quot; isn&#39;t specific enough to assign a place. </rdfs:comment>
    </owl:NamedIndividual>
    


    <!-- http://semanticbible.org/ns/2006/NTNames#HerodAgrippaI -->

    <owl:NamedIndividual rdf:about="http://semanticbible.org/ns/2006/NTNames#HerodAgrippaI">
        <rdfs:label xml:lang="en">Herod Agrippa I</rdfs:label>
        <parentOf rdf:resource="http://semanticbible.org/ns/2006/NTNames#Drusilla"/>
    </owl:NamedIndividual>
    


    <!-- http://semanticbible.org/ns/2006/NTNames#HerodAgrippaII -->

    <owl:NamedIndividual rdf:about="http://semanticbible.org/ns/2006/NTNames#HerodAgrippaII">
        <rdfs:label xml:lang="en">Herod Agrippa II</rdfs:label>
        <occupation rdf:datatype="http://www.w3.org/2001/XMLSchema#string">king</occupation>
    </owl:NamedIndividual>
    


    <!-- http://semanticbible.org/ns/2006/NTNames#HerodAntipas -->

    <owl:NamedIndividual rdf:about="http://semanticbible.org/ns/2006/NTNames#HerodAntipas">
        <rdfs:label xml:lang="en">Herod</rdfs:label>
        <rdfs:label xml:lang="en">Herod the tetrarch</rdfs:label>
        <rdfs:comment xml:lang="en">Herod the Great was Idumean, and Antipas&#39; mother was Samaritan. According to extra-biblical history, he was educated in Rome. </rdfs:comment>
        <enemyOf rdf:resource="http://semanticbible.org/ns/2006/NTNames#Jesus"/>
        <collaboratesWith rdf:resource="http://semanticbible.org/ns/2006/NTNames#PontiusPilate"/>
    </owl:NamedIndividual>
    


    <!-- http://semanticbible.org/ns/2006/NTNames#HerodTheGreat -->

    <owl:NamedIndividual rdf:about="http://semanticbible.org/ns/2006/NTNames#HerodTheGreat">
        <rdfs:label xml:lang="en">Herod</rdfs:label>
        <parentOf rdf:resource="http://semanticbible.org/ns/2006/NTNames#HerodAntipas"/>
    </owl:NamedIndividual>
    


    <!-- http://semanticbible.org/ns/2006/NTNames#Herodians -->

    <owl:NamedIndividual rdf:about="http://semanticbible.org/ns/2006/NTNames#Herodians">
        <rdfs:label xml:lang="en">Herodians</rdfs:label>
    </owl:NamedIndividual>
    


    <!-- http://semanticbible.org/ns/2006/NTNames#Herodias -->

    <owl:NamedIndividual rdf:about="http://semanticbible.org/ns/2006/NTNames#Herodias">
        <rdfs:label xml:lang="en">Herodias</rdfs:label>
        <rdfs:comment xml:lang="en">Herodias had John the Baptist put to death</rdfs:comment>
    </owl:NamedIndividual>
    


    <!-- http://semanticbible.org/ns/2006/NTNames#Herodion -->

    <owl:NamedIndividual rdf:about="http://semanticbible.org/ns/2006/NTNames#Herodion">
        <rdf:type rdf:resource="http://semanticbible.org/ns/2006/NTNames#Man"/>
        <rdfs:label xml:lang="en">Herodion</rdfs:label>
        <rdfs:comment rdf:datatype="http://www.w3.org/2001/XMLSchema#string">Paul&#39;s description of Herodian as &quot;my kinsman&quot; is taken in the general snese (e.g. coming from the same region), rather than literally. </rdfs:comment>
    </owl:NamedIndividual>
    


    <!-- http://semanticbible.org/ns/2006/NTNames#Hezekiah -->

    <owl:NamedIndividual rdf:about="http://semanticbible.org/ns/2006/NTNames#Hezekiah">
        <rdf:type rdf:resource="http://semanticbible.org/ns/2006/NTNames#Man"/>
        <rdfs:label xml:lang="en">Hezekiah</rdfs:label>
    </owl:NamedIndividual>
    


    <!-- http://semanticbible.org/ns/2006/NTNames#Hezron -->

    <owl:NamedIndividual rdf:about="http://semanticbible.org/ns/2006/NTNames#Hezron">
        <rdfs:label xml:lang="en">Hezron</rdfs:label>
        <ethnicity rdf:resource="http://semanticbible.org/ns/2006/NTNames#Jewish"/>
    </owl:NamedIndividual>
    


    <!-- http://semanticbible.org/ns/2006/NTNames#Hierapolis -->

    <owl:NamedIndividual rdf:about="http://semanticbible.org/ns/2006/NTNames#Hierapolis">
        <rdfs:label xml:lang="en">Hierapolis</rdfs:label>
    </owl:NamedIndividual>
    


    <!-- http://semanticbible.org/ns/2006/NTNames#Hosea -->

    <owl:NamedIndividual rdf:about="http://semanticbible.org/ns/2006/NTNames#Hosea">
        <rdfs:label xml:lang="en">Hosea</rdfs:label>
    </owl:NamedIndividual>
    


    <!-- http://semanticbible.org/ns/2006/NTNames#Hymenaeus -->

    <owl:NamedIndividual rdf:about="http://semanticbible.org/ns/2006/NTNames#Hymenaeus">
        <rdfs:label xml:lang="en">Hymenaeus</rdfs:label>
    </owl:NamedIndividual>
    


    <!-- http://semanticbible.org/ns/2006/NTNames#Iconium -->

    <owl:NamedIndividual rdf:about="http://semanticbible.org/ns/2006/NTNames#Iconium">
        <rdfs:label xml:lang="en">Iconium</rdfs:label>
    </owl:NamedIndividual>
    


    <!-- http://semanticbible.org/ns/2006/NTNames#IconiumGeodata -->

    <owl:NamedIndividual rdf:about="http://semanticbible.org/ns/2006/NTNames#IconiumGeodata">
        <rdfs:label xml:lang="en">geodata for Iconium</rdfs:label>
    </owl:NamedIndividual>
    


    <!-- http://semanticbible.org/ns/2006/NTNames#Idumea -->

    <owl:NamedIndividual rdf:about="http://semanticbible.org/ns/2006/NTNames#Idumea">
        <rdfs:label xml:lang="en">Idumea</rdfs:label>
    </owl:NamedIndividual>
    


    <!-- http://semanticbible.org/ns/2006/NTNames#Illyricum -->

    <owl:NamedIndividual rdf:about="http://semanticbible.org/ns/2006/NTNames#Illyricum">
        <rdfs:label xml:lang="en">Illyricum</rdfs:label>
    </owl:NamedIndividual>
    


    <!-- http://semanticbible.org/ns/2006/NTNames#Immanuel -->

    <owl:NamedIndividual rdf:about="http://semanticbible.org/ns/2006/NTNames#Immanuel">
        <rdfs:label xml:lang="en">Immanuel</rdfs:label>
    </owl:NamedIndividual>
    


    <!-- http://semanticbible.org/ns/2006/NTNames#Isaac -->

    <owl:NamedIndividual rdf:about="http://semanticbible.org/ns/2006/NTNames#Isaac">
        <rdfs:label xml:lang="en">Isaac</rdfs:label>
        <ethnicity rdf:resource="http://semanticbible.org/ns/2006/NTNames#Jewish"/>
    </owl:NamedIndividual>
    


    <!-- http://semanticbible.org/ns/2006/NTNames#Isaiah -->

    <owl:NamedIndividual rdf:about="http://semanticbible.org/ns/2006/NTNames#Isaiah">
        <rdf:type rdf:resource="http://semanticbible.org/ns/2006/NTNames#Man"/>
        <rdfs:label xml:lang="en">Isaiah</rdfs:label>
    </owl:NamedIndividual>
    


    <!-- http://semanticbible.org/ns/2006/NTNames#Iscariot -->

    <owl:NamedIndividual rdf:about="http://semanticbible.org/ns/2006/NTNames#Iscariot">
        <rdfs:label xml:lang="en">Iscariot</rdfs:label>
    </owl:NamedIndividual>
    


    <!-- http://semanticbible.org/ns/2006/NTNames#Israel -->

    <owl:NamedIndividual rdf:about="http://semanticbible.org/ns/2006/NTNames#Israel">
        <rdf:type rdf:resource="http://semanticbible.org/ns/2006/NTNames#Nation"/>
        <rdfs:label xml:lang="en">Israel</rdfs:label>
        <rdfs:comment xml:lang="en">This name designates the nation inhabited by the descendants of Jacob&#39;s twelve sons. For Israel the patriarch, see Jacob. For the inhabitants of this nation, see Israelites. </rdfs:comment>
    </owl:NamedIndividual>
    


    <!-- http://semanticbible.org/ns/2006/NTNames#Israelites -->

    <owl:NamedIndividual rdf:about="http://semanticbible.org/ns/2006/NTNames#Israelites">
        <rdfs:label xml:lang="en">Israelites</rdfs:label>
    </owl:NamedIndividual>
    


    <!-- http://semanticbible.org/ns/2006/NTNames#Issachar -->

    <owl:NamedIndividual rdf:about="http://semanticbible.org/ns/2006/NTNames#Issachar">
        <rdfs:label xml:lang="en">Issachar</rdfs:label>
    </owl:NamedIndividual>
    


    <!-- http://semanticbible.org/ns/2006/NTNames#ItalianCohort -->

    <owl:NamedIndividual rdf:about="http://semanticbible.org/ns/2006/NTNames#ItalianCohort">
        <rdfs:label xml:lang="en">Italian Cohort</rdfs:label>
        <rdfs:comment xml:lang="en">A Roman legion</rdfs:comment>
    </owl:NamedIndividual>
    


    <!-- http://semanticbible.org/ns/2006/NTNames#Italy -->

    <owl:NamedIndividual rdf:about="http://semanticbible.org/ns/2006/NTNames#Italy">
        <rdfs:label xml:lang="en">Italy</rdfs:label>
    </owl:NamedIndividual>
    


    <!-- http://semanticbible.org/ns/2006/NTNames#Ituraea -->

    <owl:NamedIndividual rdf:about="http://semanticbible.org/ns/2006/NTNames#Ituraea">
        <rdfs:label xml:lang="en">Ituraea</rdfs:label>
        <rdfs:comment xml:lang="en">An area to the NW of the Sea of Galilee. It&#39;s unclear whether this refers to a definite region or an undefined general area occupied by the Ituraeans, a migratory tribe.</rdfs:comment>
    </owl:NamedIndividual>
    


    <!-- http://semanticbible.org/ns/2006/NTNames#Jacob -->

    <owl:NamedIndividual rdf:about="http://semanticbible.org/ns/2006/NTNames#Jacob">
        <rdfs:label xml:lang="en">Israel</rdfs:label>
        <rdfs:label xml:lang="en">Jacob</rdfs:label>
        <rdfs:comment rdf:datatype="http://www.w3.org/2001/XMLSchema#string">Israel becomes a metonym describing the nation of descendants from Jacob, so it is used both for a individual, a nation, and the members of that nation. </rdfs:comment>
        <hasOnlyGenealogyMention rdf:datatype="http://www.w3.org/2001/XMLSchema#boolean">false</hasOnlyGenealogyMention>
        <siblingOf rdf:resource="http://semanticbible.org/ns/2006/NTNames#Esau"/>
    </owl:NamedIndividual>
    


    <!-- http://semanticbible.org/ns/2006/NTNames#JacobSonOfMatthan -->

    <owl:NamedIndividual rdf:about="http://semanticbible.org/ns/2006/NTNames#JacobSonOfMatthan">
        <rdfs:label xml:lang="en">Jacob</rdfs:label>
        <rdfs:comment xml:lang="en">Grandfather of Joseph, the husband of Mary, the mother of Jesus</rdfs:comment>
    </owl:NamedIndividual>
    


    <!-- http://semanticbible.org/ns/2006/NTNames#Jairus -->

    <owl:NamedIndividual rdf:about="http://semanticbible.org/ns/2006/NTNames#Jairus">
        <rdfs:label xml:lang="en">Jairus</rdfs:label>
    </owl:NamedIndividual>
    


    <!-- http://semanticbible.org/ns/2006/NTNames#Jambres -->

    <owl:NamedIndividual rdf:about="http://semanticbible.org/ns/2006/NTNames#Jambres">
        <rdf:type rdf:resource="http://semanticbible.org/ns/2006/NTNames#Man"/>
        <rdfs:label xml:lang="en">Jambres</rdfs:label>
    </owl:NamedIndividual>
    


    <!-- http://semanticbible.org/ns/2006/NTNames#James -->

    <owl:NamedIndividual rdf:about="http://semanticbible.org/ns/2006/NTNames#James">
        <rdfs:label xml:lang="en">James</rdfs:label>
    </owl:NamedIndividual>
    


    <!-- http://semanticbible.org/ns/2006/NTNames#JamesSonOfAlphaeus -->

    <owl:NamedIndividual rdf:about="http://semanticbible.org/ns/2006/NTNames#JamesSonOfAlphaeus">
        <rdfs:label xml:lang="en">James</rdfs:label>
    </owl:NamedIndividual>
    


    <!-- http://semanticbible.org/ns/2006/NTNames#JamesSonOfZebedee -->

    <owl:NamedIndividual rdf:about="http://semanticbible.org/ns/2006/NTNames#JamesSonOfZebedee">
        <rdfs:label xml:lang="en">James</rdfs:label>
    </owl:NamedIndividual>
    


    <!-- http://semanticbible.org/ns/2006/NTNames#Jannai -->

    <owl:NamedIndividual rdf:about="http://semanticbible.org/ns/2006/NTNames#Jannai">
        <rdfs:label xml:lang="en">Jannai</rdfs:label>
        <parentOf rdf:resource="http://semanticbible.org/ns/2006/NTNames#MelchiSonOfJannai"/>
    </owl:NamedIndividual>
    


    <!-- http://semanticbible.org/ns/2006/NTNames#Jannes -->

    <owl:NamedIndividual rdf:about="http://semanticbible.org/ns/2006/NTNames#Jannes">
        <rdfs:label xml:lang="en">Jannes</rdfs:label>
    </owl:NamedIndividual>
    


    <!-- http://semanticbible.org/ns/2006/NTNames#Jared -->

    <owl:NamedIndividual rdf:about="http://semanticbible.org/ns/2006/NTNames#Jared">
        <rdf:type rdf:resource="http://semanticbible.org/ns/2006/NTNames#Man"/>
        <rdfs:label xml:lang="en">Jared</rdfs:label>
    </owl:NamedIndividual>
    


    <!-- http://semanticbible.org/ns/2006/NTNames#Jason -->

    <owl:NamedIndividual rdf:about="http://semanticbible.org/ns/2006/NTNames#Jason">
        <rdfs:label xml:lang="en">Jason</rdfs:label>
        <description rdf:datatype="http://www.w3.org/2001/XMLSchema#string"> a companion of Paul&#39;s who sent greetings to the Roman church</description>
        <rdfs:comment rdf:datatype="http://www.w3.org/2001/XMLSchema#string">His residence in Corinth follows from the inference that Paul resided there when he wrote the letter to the Roman church.  &quot;kinsman&quot; here probably means that that he is a Jew, rather than an actual relative, given the number of people so designated in Romans 16. </rdfs:comment>
    </owl:NamedIndividual>
    


    <!-- http://semanticbible.org/ns/2006/NTNames#Jechoniah -->

    <owl:NamedIndividual rdf:about="http://semanticbible.org/ns/2006/NTNames#Jechoniah">
        <rdf:type rdf:resource="http://semanticbible.org/ns/2006/NTNames#Man"/>
        <rdfs:label xml:lang="en">Jechoniah</rdfs:label>
    </owl:NamedIndividual>
    


    <!-- http://semanticbible.org/ns/2006/NTNames#Jehoshaphat -->

    <owl:NamedIndividual rdf:about="http://semanticbible.org/ns/2006/NTNames#Jehoshaphat">
        <rdfs:label xml:lang="en">Jehoshaphat</rdfs:label>
    </owl:NamedIndividual>
    


    <!-- http://semanticbible.org/ns/2006/NTNames#Jephthah -->

    <owl:NamedIndividual rdf:about="http://semanticbible.org/ns/2006/NTNames#Jephthah">
        <rdf:type rdf:resource="http://semanticbible.org/ns/2006/NTNames#Man"/>
        <rdfs:label xml:lang="en">Jephthah</rdfs:label>
    </owl:NamedIndividual>
    


    <!-- http://semanticbible.org/ns/2006/NTNames#Jeremiah -->

    <owl:NamedIndividual rdf:about="http://semanticbible.org/ns/2006/NTNames#Jeremiah">
        <rdfs:label xml:lang="en">Jeremiah</rdfs:label>
    </owl:NamedIndividual>
    


    <!-- http://semanticbible.org/ns/2006/NTNames#Jericho -->

    <owl:NamedIndividual rdf:about="http://semanticbible.org/ns/2006/NTNames#Jericho">
        <rdfs:label xml:lang="en">Jericho</rdfs:label>
    </owl:NamedIndividual>
    


    <!-- http://semanticbible.org/ns/2006/NTNames#JerichoGeodata -->

    <owl:NamedIndividual rdf:about="http://semanticbible.org/ns/2006/NTNames#JerichoGeodata">
        <rdfs:label xml:lang="en">geodata for Jericho</rdfs:label>
    </owl:NamedIndividual>
    


    <!-- http://semanticbible.org/ns/2006/NTNames#Jerusalem -->

    <owl:NamedIndividual rdf:about="http://semanticbible.org/ns/2006/NTNames#Jerusalem">
        <rdfs:label xml:lang="en">Jerusalem</rdfs:label>
        <visitedPlaceOf rdf:resource="http://semanticbible.org/ns/2006/NTNames#HerodAntipas"/>
        <subregion rdf:resource="http://semanticbible.org/ns/2006/NTNames#Siloam"/>
    </owl:NamedIndividual>
    


    <!-- http://semanticbible.org/ns/2006/NTNames#JerusalemGeodata -->

    <owl:NamedIndividual rdf:about="http://semanticbible.org/ns/2006/NTNames#JerusalemGeodata">
        <rdfs:label xml:lang="en">geodata for Jerusalem</rdfs:label>
        <altitude rdf:datatype="http://www.w3.org/2001/XMLSchema#int">0</altitude>
    </owl:NamedIndividual>
    


    <!-- http://semanticbible.org/ns/2006/NTNames#Jesse -->

    <owl:NamedIndividual rdf:about="http://semanticbible.org/ns/2006/NTNames#Jesse">
        <rdfs:label xml:lang="en">Jesse</rdfs:label>
    </owl:NamedIndividual>
    


    <!-- http://semanticbible.org/ns/2006/NTNames#Jesus -->

    <owl:NamedIndividual rdf:about="http://semanticbible.org/ns/2006/NTNames#Jesus">
        <rdfs:label xml:lang="en">Jesus</rdfs:label>
        <rdfs:comment xml:lang="en">As the central figure of the New Testament, it is impossible to incorporate all the information about Jesus in this limited framework. </rdfs:comment>
    </owl:NamedIndividual>
    


    <!-- http://semanticbible.org/ns/2006/NTNames#Jew -->

    <owl:NamedIndividual rdf:about="http://semanticbible.org/ns/2006/NTNames#Jew">
        <rdfs:label xml:lang="en">Jew</rdfs:label>
    </owl:NamedIndividual>
    


    <!-- http://semanticbible.org/ns/2006/NTNames#Jewish -->

    <owl:NamedIndividual rdf:about="http://semanticbible.org/ns/2006/NTNames#Jewish">
        <rdfs:label xml:lang="en">Jewish</rdfs:label>
        <rdfs:comment xml:lang="en">The notion of &#39;Jewish&#39; as an ethnicity is problematic given the long history of God&#39;s chosen people and their many circumstances. Here it refers broadly to the Jewish identity, and is applied to all those from Abraham through Peter and Paul who would designate themselves as Jewish. In particular, no attempt is made to distinguish pre-Mosaic Jewish ethnicity from later forms. Israelite is only used a few times in the New Testament, and in those instances, it is treated synonymously with Jewish. </rdfs:comment>
        <ethnicityOf rdf:resource="http://semanticbible.org/ns/2006/NTNames#Aaron"/>
        <ethnicityOf rdf:resource="http://semanticbible.org/ns/2006/NTNames#Asaph"/>
        <ethnicityOf rdf:resource="http://semanticbible.org/ns/2006/NTNames#Drusilla"/>
        <ethnicityOf rdf:resource="http://semanticbible.org/ns/2006/NTNames#EliakimSonOfAbiud"/>
        <ethnicityOf rdf:resource="http://semanticbible.org/ns/2006/NTNames#Elisha"/>
        <ethnicityOf rdf:resource="http://semanticbible.org/ns/2006/NTNames#Eliud"/>
        <ethnicityOf rdf:resource="http://semanticbible.org/ns/2006/NTNames#Elizabeth"/>
        <ethnicityOf rdf:resource="http://semanticbible.org/ns/2006/NTNames#Hezekiah"/>
        <ethnicityOf rdf:resource="http://semanticbible.org/ns/2006/NTNames#Hezron"/>
        <ethnicityOf rdf:resource="http://semanticbible.org/ns/2006/NTNames#Jehoshaphat"/>
        <ethnicityOf rdf:resource="http://semanticbible.org/ns/2006/NTNames#JohnOfTheSanhedrin"/>
        <ethnicityOf rdf:resource="http://semanticbible.org/ns/2006/NTNames#Jonam"/>
        <ethnicityOf rdf:resource="http://semanticbible.org/ns/2006/NTNames#JosephThePatriarch"/>
        <ethnicityOf rdf:resource="http://semanticbible.org/ns/2006/NTNames#Lois"/>
        <ethnicityOf rdf:resource="http://semanticbible.org/ns/2006/NTNames#MatthatSonOfLeviSonOfMelki"/>
        <ethnicityOf rdf:resource="http://semanticbible.org/ns/2006/NTNames#MatthatSonOfLeviSonOfSimeon"/>
        <ethnicityOf rdf:resource="http://semanticbible.org/ns/2006/NTNames#Sapphira"/>
    </owl:NamedIndividual>
    


    <!-- http://semanticbible.org/ns/2006/NTNames#Jews -->

    <owl:NamedIndividual rdf:about="http://semanticbible.org/ns/2006/NTNames#Jews">
        <rdfs:label xml:lang="en">Jews</rdfs:label>
    </owl:NamedIndividual>
    


    <!-- http://semanticbible.org/ns/2006/NTNames#Jezebel -->

    <owl:NamedIndividual rdf:about="http://semanticbible.org/ns/2006/NTNames#Jezebel">
        <rdf:type rdf:resource="http://semanticbible.org/ns/2006/NTNames#Woman"/>
        <rdfs:label xml:lang="en">Jezebel</rdfs:label>
        <rdfs:comment xml:lang="en">This may be a figurative reference based on the pagan wife of Ahab in the Old Testament, rather than the actual name of a contemporary person.</rdfs:comment>
    </owl:NamedIndividual>
    


    <!-- http://semanticbible.org/ns/2006/NTNames#Joanan -->

    <owl:NamedIndividual rdf:about="http://semanticbible.org/ns/2006/NTNames#Joanan">
        <rdfs:label xml:lang="en">Joanan</rdfs:label>
    </owl:NamedIndividual>
    


    <!-- http://semanticbible.org/ns/2006/NTNames#Joanna -->

    <owl:NamedIndividual rdf:about="http://semanticbible.org/ns/2006/NTNames#Joanna">
        <rdf:type rdf:resource="http://semanticbible.org/ns/2006/NTNames#Woman"/>
        <rdfs:label xml:lang="en">Joanna</rdfs:label>
        <rdfs:comment xml:lang="en">Probably of Jewish ethnicity</rdfs:comment>
    </owl:NamedIndividual>
    


    <!-- http://semanticbible.org/ns/2006/NTNames#Job -->

    <owl:NamedIndividual rdf:about="http://semanticbible.org/ns/2006/NTNames#Job">
        <rdfs:label xml:lang="en">Job</rdfs:label>
    </owl:NamedIndividual>
    


    <!-- http://semanticbible.org/ns/2006/NTNames#Joda -->

    <owl:NamedIndividual rdf:about="http://semanticbible.org/ns/2006/NTNames#Joda">
        <rdfs:label xml:lang="en">Joda</rdfs:label>
    </owl:NamedIndividual>
    


    <!-- http://semanticbible.org/ns/2006/NTNames#Joel -->

    <owl:NamedIndividual rdf:about="http://semanticbible.org/ns/2006/NTNames#Joel">
        <rdfs:label xml:lang="en">Joel</rdfs:label>
    </owl:NamedIndividual>
    


    <!-- http://semanticbible.org/ns/2006/NTNames#JohnMark -->

    <owl:NamedIndividual rdf:about="http://semanticbible.org/ns/2006/NTNames#JohnMark">
        <rdfs:label xml:lang="en">John Mark</rdfs:label>
        <rdfs:comment xml:lang="en">One of Paul&#39;s companions</rdfs:comment>
        <relativeOf rdf:resource="http://semanticbible.org/ns/2006/NTNames#Barnabas"/>
    </owl:NamedIndividual>
    


    <!-- http://semanticbible.org/ns/2006/NTNames#JohnOfTheSanhedrin -->

    <owl:NamedIndividual rdf:about="http://semanticbible.org/ns/2006/NTNames#JohnOfTheSanhedrin">
        <rdfs:label xml:lang="en">John</rdfs:label>
    </owl:NamedIndividual>
    


    <!-- http://semanticbible.org/ns/2006/NTNames#JohnSonOfZebedee -->

    <owl:NamedIndividual rdf:about="http://semanticbible.org/ns/2006/NTNames#JohnSonOfZebedee">
        <rdfs:label xml:lang="en">John</rdfs:label>
        <collaboratesWith rdf:resource="http://semanticbible.org/ns/2006/NTNames#MaryMagdalene"/>
    </owl:NamedIndividual>
    


    <!-- http://semanticbible.org/ns/2006/NTNames#JohntheBaptist -->

    <owl:NamedIndividual rdf:about="http://semanticbible.org/ns/2006/NTNames#JohntheBaptist">
        <rdfs:label xml:lang="en">John</rdfs:label>
        <rdfs:label xml:lang="en">John the Baptist</rdfs:label>
        <rdfs:comment rdf:datatype="http://www.w3.org/2001/XMLSchema#string">John certainly understood Jesus to be the Messiah and was a person of faith, but he cannot be accounted a Christian since Jesus&#39; ministry was not yet accomplished when he was beheaded. 
The use of the name Elijah to refer to John the Baptist is figurative.</rdfs:comment>
        <childOf rdf:resource="http://semanticbible.org/ns/2006/NTNames#Elizabeth"/>
    </owl:NamedIndividual>
    


    <!-- http://semanticbible.org/ns/2006/NTNames#JonahOfBethsaida -->

    <owl:NamedIndividual rdf:about="http://semanticbible.org/ns/2006/NTNames#JonahOfBethsaida">
        <rdfs:label xml:lang="en">Jonah</rdfs:label>
        <rdfs:comment rdf:datatype="http://www.w3.org/2001/XMLSchema#string">Bethsaide is assumed as his place of residence because his sons were from there. He was probably a fisherman, though nothing else is said of him in the New Testament.</rdfs:comment>
    </owl:NamedIndividual>
    


    <!-- http://semanticbible.org/ns/2006/NTNames#JonahTheProphet -->

    <owl:NamedIndividual rdf:about="http://semanticbible.org/ns/2006/NTNames#JonahTheProphet">
        <rdfs:label xml:lang="en">Jonah</rdfs:label>
    </owl:NamedIndividual>
    


    <!-- http://semanticbible.org/ns/2006/NTNames#Jonam -->

    <owl:NamedIndividual rdf:about="http://semanticbible.org/ns/2006/NTNames#Jonam">
        <rdfs:label xml:lang="en">Jonam</rdfs:label>
    </owl:NamedIndividual>
    


    <!-- http://semanticbible.org/ns/2006/NTNames#Joppa -->

    <owl:NamedIndividual rdf:about="http://semanticbible.org/ns/2006/NTNames#Joppa">
        <rdfs:label xml:lang="en">Joppa</rdfs:label>
        <rdfs:comment xml:lang="en">In Joppa, Peter raised the woman Tabitha from the dead. Later, he had a vision while praying there that prepared him for the coming of the Holy Spirit to the first Gentiles.</rdfs:comment>
        <subregionOf rdf:resource="http://semanticbible.org/ns/2006/NTNames#Judea"/>
    </owl:NamedIndividual>
    


    <!-- http://semanticbible.org/ns/2006/NTNames#JoppaGeodata -->

    <owl:NamedIndividual rdf:about="http://semanticbible.org/ns/2006/NTNames#JoppaGeodata">
        <rdfs:label xml:lang="en">geodata for Joppa</rdfs:label>
    </owl:NamedIndividual>
    


    <!-- http://semanticbible.org/ns/2006/NTNames#Joram -->

    <owl:NamedIndividual rdf:about="http://semanticbible.org/ns/2006/NTNames#Joram">
        <rdfs:label xml:lang="en">Joram</rdfs:label>
        <rdfs:comment rdf:datatype="http://www.w3.org/2001/XMLSchema#string">His occupation as King comes from Old Testament sources. </rdfs:comment>
        <description rdf:datatype="http://www.w3.org/2001/XMLSchema#string">One of the ancestors of Jesus mentioned in Matthew&#39;s geneaology</description>
    </owl:NamedIndividual>
    


    <!-- http://semanticbible.org/ns/2006/NTNames#Jordan -->

    <owl:NamedIndividual rdf:about="http://semanticbible.org/ns/2006/NTNames#Jordan">
        <rdfs:label xml:lang="en">Jordan</rdfs:label>
    </owl:NamedIndividual>
    


    <!-- http://semanticbible.org/ns/2006/NTNames#Jorim -->

    <owl:NamedIndividual rdf:about="http://semanticbible.org/ns/2006/NTNames#Jorim">
        <rdfs:label xml:lang="en">Jorim</rdfs:label>
    </owl:NamedIndividual>
    


    <!-- http://semanticbible.org/ns/2006/NTNames#Josech -->

    <owl:NamedIndividual rdf:about="http://semanticbible.org/ns/2006/NTNames#Josech">
        <rdfs:label xml:lang="en">Josech</rdfs:label>
        <ethnicity rdf:resource="http://semanticbible.org/ns/2006/NTNames#Jewish"/>
    </owl:NamedIndividual>
    


    <!-- http://semanticbible.org/ns/2006/NTNames#Joseph -->

    <owl:NamedIndividual rdf:about="http://semanticbible.org/ns/2006/NTNames#Joseph">
        <rdfs:label xml:lang="en">Joseph</rdfs:label>
        <rdfs:comment xml:lang="en">Joseph was Jesus&#39; parent in the normal sense, even though not his biological father.
Luke 3:23 has &quot;Joseph, son of Heli&quot;, though Matthew has Joseph&#39;s father named Jacob. Here I&#39;ve represented the opinion that Joseph was actually son-in-law of Heli, and that Luke&#39;s geneaology describes Mary&#39;s lineage rather than Joseph&#39;s. </rdfs:comment>
    </owl:NamedIndividual>
    


    <!-- http://semanticbible.org/ns/2006/NTNames#JosephBarsabbas -->

    <owl:NamedIndividual rdf:about="http://semanticbible.org/ns/2006/NTNames#JosephBarsabbas">
        <rdfs:label xml:lang="en">Joseph Barsabbas</rdfs:label>
        <collaboratesWith rdf:resource="http://semanticbible.org/ns/2006/NTNames#SimonPeter"/>
    </owl:NamedIndividual>
    


    <!-- http://semanticbible.org/ns/2006/NTNames#JosephOfArimathea -->

    <owl:NamedIndividual rdf:about="http://semanticbible.org/ns/2006/NTNames#JosephOfArimathea">
        <rdfs:label xml:lang="en">Joseph of Arimathea</rdfs:label>
        <rdfs:comment xml:lang="en">Joseph was a member of the Jewish ruling council, and a follower of Jesus. He put Jesus&#39; body in his own tomb after the crucifixion. {en}</rdfs:comment>
    </owl:NamedIndividual>
    


    <!-- http://semanticbible.org/ns/2006/NTNames#JosephSonOfJonam -->

    <owl:NamedIndividual rdf:about="http://semanticbible.org/ns/2006/NTNames#JosephSonOfJonam">
        <rdfs:label xml:lang="en">Joseph</rdfs:label>
        <ethnicity rdf:resource="http://semanticbible.org/ns/2006/NTNames#Jewish"/>
    </owl:NamedIndividual>
    


    <!-- http://semanticbible.org/ns/2006/NTNames#JosephSonOfMattathias -->

    <owl:NamedIndividual rdf:about="http://semanticbible.org/ns/2006/NTNames#JosephSonOfMattathias">
        <rdfs:label xml:lang="en">Joseph</rdfs:label>
    </owl:NamedIndividual>
    


    <!-- http://semanticbible.org/ns/2006/NTNames#JosephThePatriarch -->

    <owl:NamedIndividual rdf:about="http://semanticbible.org/ns/2006/NTNames#JosephThePatriarch">
        <rdfs:label xml:lang="en">Joseph</rdfs:label>
    </owl:NamedIndividual>
    


    <!-- http://semanticbible.org/ns/2006/NTNames#Joses -->

    <owl:NamedIndividual rdf:about="http://semanticbible.org/ns/2006/NTNames#Joses">
        <rdfs:label xml:lang="en">Joses</rdfs:label>
    </owl:NamedIndividual>
    


    <!-- http://semanticbible.org/ns/2006/NTNames#Joshua -->

    <owl:NamedIndividual rdf:about="http://semanticbible.org/ns/2006/NTNames#Joshua">
        <rdf:type rdf:resource="http://semanticbible.org/ns/2006/NTNames#Man"/>
        <rdfs:label xml:lang="en">Joshua</rdfs:label>
    </owl:NamedIndividual>
    


    <!-- http://semanticbible.org/ns/2006/NTNames#JoshuaSonOfEliezer -->

    <owl:NamedIndividual rdf:about="http://semanticbible.org/ns/2006/NTNames#JoshuaSonOfEliezer">
        <rdfs:label xml:lang="en">Joshua</rdfs:label>
    </owl:NamedIndividual>
    


    <!-- http://semanticbible.org/ns/2006/NTNames#Josiah -->

    <owl:NamedIndividual rdf:about="http://semanticbible.org/ns/2006/NTNames#Josiah">
        <rdfs:label xml:lang="en">Josiah</rdfs:label>
    </owl:NamedIndividual>
    


    <!-- http://semanticbible.org/ns/2006/NTNames#Jotham -->

    <owl:NamedIndividual rdf:about="http://semanticbible.org/ns/2006/NTNames#Jotham">
        <rdfs:label xml:lang="en">Jotham</rdfs:label>
        <rdfs:comment rdf:datatype="http://www.w3.org/2001/XMLSchema#string">His occupation as King comes from Old Testament sources, 2Chron.26-27. </rdfs:comment>
        <description rdf:datatype="http://www.w3.org/2001/XMLSchema#string">One of the ancestors of Jesus mentioned in Matthew&#39;s geneaology</description>
        <hasOnlyGenealogyMention rdf:datatype="http://www.w3.org/2001/XMLSchema#boolean">true</hasOnlyGenealogyMention>
    </owl:NamedIndividual>
    


    <!-- http://semanticbible.org/ns/2006/NTNames#Judah -->

    <owl:NamedIndividual rdf:about="http://semanticbible.org/ns/2006/NTNames#Judah">
        <rdfs:label xml:lang="en">Judah</rdfs:label>
        <rdfs:comment rdf:datatype="http://www.w3.org/2001/XMLSchema#string">Tamar was not actually his spouse, but his daughter-in-law (Gen 38).
</rdfs:comment>
        <hasOnlyGenealogyMention rdf:datatype="http://www.w3.org/2001/XMLSchema#boolean">false</hasOnlyGenealogyMention>
    </owl:NamedIndividual>
    


    <!-- http://semanticbible.org/ns/2006/NTNames#JudahSonOfJoseph -->

    <owl:NamedIndividual rdf:about="http://semanticbible.org/ns/2006/NTNames#JudahSonOfJoseph">
        <rdfs:label xml:lang="en">Judah</rdfs:label>
    </owl:NamedIndividual>
    


    <!-- http://semanticbible.org/ns/2006/NTNames#Judaism -->

    <owl:NamedIndividual rdf:about="http://semanticbible.org/ns/2006/NTNames#Judaism">
        <rdf:type rdf:resource="http://semanticbible.org/ns/2006/NTNames#ReligiousBeliefSystem"/>
        <rdfs:label xml:lang="en">Judaism</rdfs:label>
        <rdfs:comment xml:lang="en">This is distinct from Jewish as an ethnic heritage, which implies birth: one can have a ReligiousBelief of Judaism through conversion, despite not having Jewish ethnicity. Those who convert to other beliefs (most notably for the New Testament, Christianity) are typically designated as having Jewish ethnicity, but Christianity as a ReligiousBelief. There is no implication of faithful devotion to the Jewish faith. </rdfs:comment>
    </owl:NamedIndividual>
    


    <!-- http://semanticbible.org/ns/2006/NTNames#Judas -->

    <owl:NamedIndividual rdf:about="http://semanticbible.org/ns/2006/NTNames#Judas">
        <rdfs:label xml:lang="en">Judas</rdfs:label>
    </owl:NamedIndividual>
    


    <!-- http://semanticbible.org/ns/2006/NTNames#JudasOfAntioch -->

    <owl:NamedIndividual rdf:about="http://semanticbible.org/ns/2006/NTNames#JudasOfAntioch">
        <rdfs:label xml:lang="en">Judas</rdfs:label>
    </owl:NamedIndividual>
    


    <!-- http://semanticbible.org/ns/2006/NTNames#Jude -->

    <owl:NamedIndividual rdf:about="http://semanticbible.org/ns/2006/NTNames#Jude">
        <rdfs:label xml:lang="en">Jude</rdfs:label>
    </owl:NamedIndividual>
    


    <!-- http://semanticbible.org/ns/2006/NTNames#Judea -->

    <owl:NamedIndividual rdf:about="http://semanticbible.org/ns/2006/NTNames#Judea">
        <rdfs:label xml:lang="en">Judea</rdfs:label>
        <nativePlaceOf rdf:resource="http://semanticbible.org/ns/2006/NTNames#Elizabeth"/>
    </owl:NamedIndividual>
    


    <!-- http://semanticbible.org/ns/2006/NTNames#Judean -->

    <owl:NamedIndividual rdf:about="http://semanticbible.org/ns/2006/NTNames#Judean">
        <rdfs:label xml:lang="en">Judean</rdfs:label>
        <rdfs:comment xml:lang="en">The main subgroup of Jewish Palestine at the time of Christ: to be Judean therefore implies being Jewish as well. This is distinct from describing those of the tribe and lineage of Judah.</rdfs:comment>
    </owl:NamedIndividual>
    


    <!-- http://semanticbible.org/ns/2006/NTNames#Julia -->

    <owl:NamedIndividual rdf:about="http://semanticbible.org/ns/2006/NTNames#Julia">
        <rdfs:label xml:lang="en">Julia</rdfs:label>
        <rdfs:comment rdf:datatype="http://www.w3.org/2001/XMLSchema#string">Julia may be the spouse or sister of Philologus, given their mention together in Rom.16.15</rdfs:comment>
        <hasOnlyGenealogyMention rdf:datatype="http://www.w3.org/2001/XMLSchema#boolean">false</hasOnlyGenealogyMention>
        <knows rdf:resource="http://semanticbible.org/ns/2006/NTNames#Paul"/>
    </owl:NamedIndividual>
    


    <!-- http://semanticbible.org/ns/2006/NTNames#Julius -->

    <owl:NamedIndividual rdf:about="http://semanticbible.org/ns/2006/NTNames#Julius">
        <rdfs:label xml:lang="en">Julius</rdfs:label>
    </owl:NamedIndividual>
    


    <!-- http://semanticbible.org/ns/2006/NTNames#Junia -->

    <owl:NamedIndividual rdf:about="http://semanticbible.org/ns/2006/NTNames#Junia">
        <rdfs:label xml:lang="en">Junia</rdfs:label>
        <rdfs:comment xml:lang="en">Given their joint mention by Paul, it seems likely that Junia was Andronicus&#39; spouse, though this is not explicitly stated. Paul&#39;s description of Andronicus and Junia as &quot;my kinsmen&quot; is taken in the general sense (e.g. coming from the same region), rather than literally. 
Given they were Christians before Paul, their conversion must have been relatively early in the history of the church, and so it is quite likely they also visited Jerusalem (though this is nowhere stated). 
Much controversy rests on whether this description means they were well-known _to_ the apostles, or well-known _as_ apostles. </rdfs:comment>
    </owl:NamedIndividual>
    


    <!-- http://semanticbible.org/ns/2006/NTNames#Kidron -->

    <owl:NamedIndividual rdf:about="http://semanticbible.org/ns/2006/NTNames#Kidron">
        <rdfs:label xml:lang="en">Kidron</rdfs:label>
        <rdfs:comment xml:lang="en">The Kidron Brook/Valley is just outside the walls of Jerusalem</rdfs:comment>
    </owl:NamedIndividual>
    


    <!-- http://semanticbible.org/ns/2006/NTNames#Kish -->

    <owl:NamedIndividual rdf:about="http://semanticbible.org/ns/2006/NTNames#Kish">
        <rdfs:label xml:lang="en">Kish</rdfs:label>
    </owl:NamedIndividual>
    


    <!-- http://semanticbible.org/ns/2006/NTNames#Korah -->

    <owl:NamedIndividual rdf:about="http://semanticbible.org/ns/2006/NTNames#Korah">
        <rdfs:label xml:lang="en">Korah</rdfs:label>
    </owl:NamedIndividual>
    


    <!-- http://semanticbible.org/ns/2006/NTNames#Lamech -->

    <owl:NamedIndividual rdf:about="http://semanticbible.org/ns/2006/NTNames#Lamech">
        <rdfs:label xml:lang="en">Lamech</rdfs:label>
    </owl:NamedIndividual>
    


    <!-- http://semanticbible.org/ns/2006/NTNames#Laodicea -->

    <owl:NamedIndividual rdf:about="http://semanticbible.org/ns/2006/NTNames#Laodicea">
        <rdfs:label xml:lang="en">Laodicea</rdfs:label>
    </owl:NamedIndividual>
    


    <!-- http://semanticbible.org/ns/2006/NTNames#LaodiceaGeodata -->

    <owl:NamedIndividual rdf:about="http://semanticbible.org/ns/2006/NTNames#LaodiceaGeodata">
        <rdfs:label xml:lang="en">geodata for Laodicea</rdfs:label>
        <longitude rdf:datatype="http://www.w3.org/2001/XMLSchema#double">29.09677098362944</longitude>
    </owl:NamedIndividual>
    


    <!-- http://semanticbible.org/ns/2006/NTNames#Laodiceans -->

    <owl:NamedIndividual rdf:about="http://semanticbible.org/ns/2006/NTNames#Laodiceans">
        <rdfs:label xml:lang="en">Laodiceans</rdfs:label>
    </owl:NamedIndividual>
    


    <!-- http://semanticbible.org/ns/2006/NTNames#Lasea -->

    <owl:NamedIndividual rdf:about="http://semanticbible.org/ns/2006/NTNames#Lasea">
        <rdfs:label xml:lang="en">Lasea</rdfs:label>
    </owl:NamedIndividual>
    


    <!-- http://semanticbible.org/ns/2006/NTNames#LaseaGeodata -->

    <owl:NamedIndividual rdf:about="http://semanticbible.org/ns/2006/NTNames#LaseaGeodata">
        <rdfs:label xml:lang="en">geodata for Lasea</rdfs:label>
    </owl:NamedIndividual>
    


    <!-- http://semanticbible.org/ns/2006/NTNames#Latin -->

    <owl:NamedIndividual rdf:about="http://semanticbible.org/ns/2006/NTNames#Latin">
        <rdfs:label xml:lang="en">Latin</rdfs:label>
    </owl:NamedIndividual>
    


    <!-- http://semanticbible.org/ns/2006/NTNames#Lazarus -->

    <owl:NamedIndividual rdf:about="http://semanticbible.org/ns/2006/NTNames#Lazarus">
        <rdfs:label xml:lang="en">Lazarus</rdfs:label>
        <rdfs:comment xml:lang="en">There&#39;s no evidence to suggest a connection between Lazarus of Bethany and the same-named subject of Jesus&#39; parable.</rdfs:comment>
    </owl:NamedIndividual>
    


    <!-- http://semanticbible.org/ns/2006/NTNames#Levi -->

    <owl:NamedIndividual rdf:about="http://semanticbible.org/ns/2006/NTNames#Levi">
        <rdfs:label xml:lang="en">Levi</rdfs:label>
        <rdfs:comment xml:lang="en">One of the Twelve, also known as Matthew. </rdfs:comment>
    </owl:NamedIndividual>
    


    <!-- http://semanticbible.org/ns/2006/NTNames#LeviSonOfMelki -->

    <owl:NamedIndividual rdf:about="http://semanticbible.org/ns/2006/NTNames#LeviSonOfMelki">
        <rdfs:label xml:lang="en">Levi</rdfs:label>
        <childOf rdf:resource="http://semanticbible.org/ns/2006/NTNames#MelchiSonOfJannai"/>
    </owl:NamedIndividual>
    


    <!-- http://semanticbible.org/ns/2006/NTNames#LeviSonOfSimeon -->

    <owl:NamedIndividual rdf:about="http://semanticbible.org/ns/2006/NTNames#LeviSonOfSimeon">
        <rdfs:label xml:lang="en">Levi</rdfs:label>
    </owl:NamedIndividual>
    


    <!-- http://semanticbible.org/ns/2006/NTNames#Levite -->

    <owl:NamedIndividual rdf:about="http://semanticbible.org/ns/2006/NTNames#Levite">
        <rdfs:label xml:lang="en">Levite</rdfs:label>
        <rdfs:comment xml:lang="en">All Levites are Jewish by definition.</rdfs:comment>
    </owl:NamedIndividual>
    


    <!-- http://semanticbible.org/ns/2006/NTNames#Levites -->

    <owl:NamedIndividual rdf:about="http://semanticbible.org/ns/2006/NTNames#Levites">
        <rdfs:label xml:lang="en">Levites</rdfs:label>
        <rdfs:comment xml:lang="en">Distinguished from Jews not by different beliefs, but by special roles related to observation of temple worship.</rdfs:comment>
    </owl:NamedIndividual>
    


    <!-- http://semanticbible.org/ns/2006/NTNames#Libya -->

    <owl:NamedIndividual rdf:about="http://semanticbible.org/ns/2006/NTNames#Libya">
        <rdfs:label xml:lang="en">Libya</rdfs:label>
    </owl:NamedIndividual>
    


    <!-- http://semanticbible.org/ns/2006/NTNames#Linus -->

    <owl:NamedIndividual rdf:about="http://semanticbible.org/ns/2006/NTNames#Linus">
        <rdfs:label xml:lang="en">Linus</rdfs:label>
    </owl:NamedIndividual>
    


    <!-- http://semanticbible.org/ns/2006/NTNames#Lois -->

    <owl:NamedIndividual rdf:about="http://semanticbible.org/ns/2006/NTNames#Lois">
        <rdfs:label xml:lang="en">Lois</rdfs:label>
        <rdfs:comment rdf:datatype="http://www.w3.org/2001/XMLSchema#string">Her Christian belief is implied by Paul&#39;s commendation of her faith. Her daughter Eunice lived in Lystra, but her residence is unknown. </rdfs:comment>
        <description rdf:datatype="http://www.w3.org/2001/XMLSchema#string">the grandmother of Timothy</description>
        <religiousBelief rdf:resource="http://semanticbible.org/ns/2006/NTNames#Christianity"/>
    </owl:NamedIndividual>
    


    <!-- http://semanticbible.org/ns/2006/NTNames#Lot -->

    <owl:NamedIndividual rdf:about="http://semanticbible.org/ns/2006/NTNames#Lot">
        <rdfs:label xml:lang="en">Lot</rdfs:label>
    </owl:NamedIndividual>
    


    <!-- http://semanticbible.org/ns/2006/NTNames#Lucius -->

    <owl:NamedIndividual rdf:about="http://semanticbible.org/ns/2006/NTNames#Lucius">
        <rdfs:label xml:lang="en">Lucius</rdfs:label>
        <rdfs:comment rdf:datatype="http://www.w3.org/2001/XMLSchema#string">This person may be the same as Lucius of Cyrene, but there&#39;s no clear evidence other than the name. His residence in Corinth follows from the inference that Paul resided there when he wrote the letter to the Roman church.  &quot;kinsman&quot; here probably means that that he is a Jew, rather than an actual relation, given the number of people so designated in Romans 16. </rdfs:comment>
        <knows rdf:resource="http://semanticbible.org/ns/2006/NTNames#Timothy"/>
    </owl:NamedIndividual>
    


    <!-- http://semanticbible.org/ns/2006/NTNames#LuciusOfCyrene -->

    <owl:NamedIndividual rdf:about="http://semanticbible.org/ns/2006/NTNames#LuciusOfCyrene">
        <rdfs:label xml:lang="en">Lucius</rdfs:label>
        <rdfs:comment rdf:datatype="http://www.w3.org/2001/XMLSchema#string">This person may be the same as the Lucius in Rome, but there&#39;s no clear evidence other than the name.</rdfs:comment>
        <collaboratesWith rdf:resource="http://semanticbible.org/ns/2006/NTNames#Manaen"/>
    </owl:NamedIndividual>
    


    <!-- http://semanticbible.org/ns/2006/NTNames#Luke -->

    <owl:NamedIndividual rdf:about="http://semanticbible.org/ns/2006/NTNames#Luke">
        <rdfs:label xml:lang="en">Luke</rdfs:label>
    </owl:NamedIndividual>
    


    <!-- http://semanticbible.org/ns/2006/NTNames#Lycaonia -->

    <owl:NamedIndividual rdf:about="http://semanticbible.org/ns/2006/NTNames#Lycaonia">
        <rdfs:label xml:lang="en">Lycaonia</rdfs:label>
    </owl:NamedIndividual>
    


    <!-- http://semanticbible.org/ns/2006/NTNames#Lycaonian -->

    <owl:NamedIndividual rdf:about="http://semanticbible.org/ns/2006/NTNames#Lycaonian">
        <rdfs:label xml:lang="en">Lycaonian</rdfs:label>
    </owl:NamedIndividual>
    


    <!-- http://semanticbible.org/ns/2006/NTNames#Lycia -->

    <owl:NamedIndividual rdf:about="http://semanticbible.org/ns/2006/NTNames#Lycia">
        <rdfs:label xml:lang="en">Lycia</rdfs:label>
    </owl:NamedIndividual>
    


    <!-- http://semanticbible.org/ns/2006/NTNames#Lydda -->

    <owl:NamedIndividual rdf:about="http://semanticbible.org/ns/2006/NTNames#Lydda">
        <rdfs:label xml:lang="en">Lydda</rdfs:label>
    </owl:NamedIndividual>
    


    <!-- http://semanticbible.org/ns/2006/NTNames#LyddaGeodata -->

    <owl:NamedIndividual rdf:about="http://semanticbible.org/ns/2006/NTNames#LyddaGeodata">
        <rdfs:label xml:lang="en">geodata for Lydda</rdfs:label>
    </owl:NamedIndividual>
    


    <!-- http://semanticbible.org/ns/2006/NTNames#Lydia -->

    <owl:NamedIndividual rdf:about="http://semanticbible.org/ns/2006/NTNames#Lydia">
        <rdfs:label xml:lang="en">Lydia</rdfs:label>
        <religiousBelief rdf:resource="http://semanticbible.org/ns/2006/NTNames#Christianity"/>
    </owl:NamedIndividual>
    


    <!-- http://semanticbible.org/ns/2006/NTNames#Lysanias -->

    <owl:NamedIndividual rdf:about="http://semanticbible.org/ns/2006/NTNames#Lysanias">
        <rdfs:label xml:lang="en">Lysanias</rdfs:label>
    </owl:NamedIndividual>
    


    <!-- http://semanticbible.org/ns/2006/NTNames#Lysias -->

    <owl:NamedIndividual rdf:about="http://semanticbible.org/ns/2006/NTNames#Lysias">
        <rdfs:label xml:lang="en">Lysias</rdfs:label>
    </owl:NamedIndividual>
    


    <!-- http://semanticbible.org/ns/2006/NTNames#Lystra -->

    <owl:NamedIndividual rdf:about="http://semanticbible.org/ns/2006/NTNames#Lystra">
        <rdfs:label xml:lang="en">Lystra</rdfs:label>
    </owl:NamedIndividual>
    


    <!-- http://semanticbible.org/ns/2006/NTNames#LystraGeodata -->

    <owl:NamedIndividual rdf:about="http://semanticbible.org/ns/2006/NTNames#LystraGeodata">
        <rdfs:label xml:lang="en">geodata for Lystra</rdfs:label>
    </owl:NamedIndividual>
    


    <!-- http://semanticbible.org/ns/2006/NTNames#Maath -->

    <owl:NamedIndividual rdf:about="http://semanticbible.org/ns/2006/NTNames#Maath">
        <rdfs:label xml:lang="en">Maath</rdfs:label>
    </owl:NamedIndividual>
    


    <!-- http://semanticbible.org/ns/2006/NTNames#Macedonia -->

    <owl:NamedIndividual rdf:about="http://semanticbible.org/ns/2006/NTNames#Macedonia">
        <rdfs:label xml:lang="en">Macedonia</rdfs:label>
    </owl:NamedIndividual>
    


    <!-- http://semanticbible.org/ns/2006/NTNames#Macedonian -->

    <owl:NamedIndividual rdf:about="http://semanticbible.org/ns/2006/NTNames#Macedonian">
        <rdfs:label xml:lang="en">Macedonian</rdfs:label>
        <rdfs:comment xml:lang="en">Of the region of Macedonia (and therefore also Greek).</rdfs:comment>
    </owl:NamedIndividual>
    


    <!-- http://semanticbible.org/ns/2006/NTNames#Macedonians -->

    <owl:NamedIndividual rdf:about="http://semanticbible.org/ns/2006/NTNames#Macedonians">
        <rdfs:label xml:lang="en">Macedonians</rdfs:label>
    </owl:NamedIndividual>
    


    <!-- http://semanticbible.org/ns/2006/NTNames#Magadan -->

    <owl:NamedIndividual rdf:about="http://semanticbible.org/ns/2006/NTNames#Magadan">
        <rdfs:label xml:lang="en">Magadan</rdfs:label>
    </owl:NamedIndividual>
    


    <!-- http://semanticbible.org/ns/2006/NTNames#Magog -->

    <owl:NamedIndividual rdf:about="http://semanticbible.org/ns/2006/NTNames#Magog">
        <rdfs:label xml:lang="en">Magog</rdfs:label>
        <rdfs:comment rdf:datatype="http://www.w3.org/2001/XMLSchema#string">Though in its original Old Testament context Magog  referred to a region, its New Testament usage seems to describe a group of people. </rdfs:comment>
    </owl:NamedIndividual>
    


    <!-- http://semanticbible.org/ns/2006/NTNames#Mahalaleel -->

    <owl:NamedIndividual rdf:about="http://semanticbible.org/ns/2006/NTNames#Mahalaleel">
        <rdfs:label xml:lang="en">Mahalaleel</rdfs:label>
        <parentOf rdf:resource="http://semanticbible.org/ns/2006/NTNames#Jared"/>
    </owl:NamedIndividual>
    


    <!-- http://semanticbible.org/ns/2006/NTNames#Malchus -->

    <owl:NamedIndividual rdf:about="http://semanticbible.org/ns/2006/NTNames#Malchus">
        <rdfs:label xml:lang="en">Malchus</rdfs:label>
    </owl:NamedIndividual>
    


    <!-- http://semanticbible.org/ns/2006/NTNames#Malta -->

    <owl:NamedIndividual rdf:about="http://semanticbible.org/ns/2006/NTNames#Malta">
        <rdf:type rdf:resource="http://semanticbible.org/ns/2006/NTNames#Island"/>
        <rdfs:label xml:lang="en">Malta</rdfs:label>
    </owl:NamedIndividual>
    


    <!-- http://semanticbible.org/ns/2006/NTNames#MaltaGeodata -->

    <owl:NamedIndividual rdf:about="http://semanticbible.org/ns/2006/NTNames#MaltaGeodata">
        <rdfs:label xml:lang="en">geodata for Malta</rdfs:label>
    </owl:NamedIndividual>
    


    <!-- http://semanticbible.org/ns/2006/NTNames#Manaen -->

    <owl:NamedIndividual rdf:about="http://semanticbible.org/ns/2006/NTNames#Manaen">
        <rdfs:label xml:lang="en">Manaen</rdfs:label>
        <rdfs:comment rdf:datatype="http://www.w3.org/2001/XMLSchema#string">The term translated &quot;foster-brother&quot; means Manaen and Herod Antipas were raised together, though not literally relatives.</rdfs:comment>
    </owl:NamedIndividual>
    


    <!-- http://semanticbible.org/ns/2006/NTNames#Manasseh -->

    <owl:NamedIndividual rdf:about="http://semanticbible.org/ns/2006/NTNames#Manasseh">
        <rdfs:label xml:lang="en">Manasseh</rdfs:label>
    </owl:NamedIndividual>
    


    <!-- http://semanticbible.org/ns/2006/NTNames#ManassehThePatriarch -->

    <owl:NamedIndividual rdf:about="http://semanticbible.org/ns/2006/NTNames#ManassehThePatriarch">
        <rdfs:label xml:lang="en">Manasseh</rdfs:label>
    </owl:NamedIndividual>
    


    <!-- http://semanticbible.org/ns/2006/NTNames#Martha -->

    <owl:NamedIndividual rdf:about="http://semanticbible.org/ns/2006/NTNames#Martha">
        <rdfs:label xml:lang="en">Martha</rdfs:label>
    </owl:NamedIndividual>
    


    <!-- http://semanticbible.org/ns/2006/NTNames#Mary -->

    <owl:NamedIndividual rdf:about="http://semanticbible.org/ns/2006/NTNames#Mary">
        <rdfs:label xml:lang="en">Mary</rdfs:label>
        <description rdf:datatype="http://www.w3.org/2001/XMLSchema#string">the mother of Jesus</description>
        <rdfs:comment xml:lang="en">See the note on Joseph for why Mary is childOf Heli. She is described by John as standing at the foot of Jesus&#39; cross with two other Marys. Her relationship to John assumes he is the &quot;beloved discipled&quot; described in John&#39;s gospel. </rdfs:comment>
    </owl:NamedIndividual>
    


    <!-- http://semanticbible.org/ns/2006/NTNames#MaryMagdalene -->

    <owl:NamedIndividual rdf:about="http://semanticbible.org/ns/2006/NTNames#MaryMagdalene">
        <rdfs:label xml:lang="en">Mary Magdalene</rdfs:label>
        <description rdf:datatype="http://www.w3.org/2001/XMLSchema#string">A woman from whom seven demons had been exorcised</description>
        <rdfs:comment xml:lang="en">From Magdala, a town in Galilee not mentioned in the New Testament</rdfs:comment>
        <knows rdf:resource="http://semanticbible.org/ns/2006/NTNames#MaryWifeOfClopas"/>
    </owl:NamedIndividual>
    


    <!-- http://semanticbible.org/ns/2006/NTNames#MaryMotherOfJohnMark -->

    <owl:NamedIndividual rdf:about="http://semanticbible.org/ns/2006/NTNames#MaryMotherOfJohnMark">
        <rdfs:label xml:lang="en">Mary</rdfs:label>
    </owl:NamedIndividual>
    


    <!-- http://semanticbible.org/ns/2006/NTNames#MaryOfBethany -->

    <owl:NamedIndividual rdf:about="http://semanticbible.org/ns/2006/NTNames#MaryOfBethany">
        <rdfs:label xml:lang="en">Mary</rdfs:label>
        <rdfs:comment rdf:datatype="http://www.w3.org/2001/XMLSchema#string">There are other accounts of an unnamed woman annointing Jesus with oil, and various arguments about whether these were the same or different women. </rdfs:comment>
        <ethnicity rdf:resource="http://semanticbible.org/ns/2006/NTNames#Jewish"/>
    </owl:NamedIndividual>
    


    <!-- http://semanticbible.org/ns/2006/NTNames#MaryOfRome -->

    <owl:NamedIndividual rdf:about="http://semanticbible.org/ns/2006/NTNames#MaryOfRome">
        <rdfs:label xml:lang="en">Mary</rdfs:label>
        <description rdf:datatype="http://www.w3.org/2001/XMLSchema#string">a woman to whom Paul sent greetings in his letter to the Romans</description>
    </owl:NamedIndividual>
    


    <!-- http://semanticbible.org/ns/2006/NTNames#MaryWifeOfClopas -->

    <owl:NamedIndividual rdf:about="http://semanticbible.org/ns/2006/NTNames#MaryWifeOfClopas">
        <rdfs:label xml:lang="en">Mary</rdfs:label>
        <rdfs:comment xml:lang="en">Comparing the Gospel accounts in John.19.25 and Mark.15.40, this Mary appears to be the same woman as the mother of James and Joseph/Joses, and therefore sister of Mary the mother of Jesus.</rdfs:comment>
    </owl:NamedIndividual>
    


    <!-- http://semanticbible.org/ns/2006/NTNames#Mattatha -->

    <owl:NamedIndividual rdf:about="http://semanticbible.org/ns/2006/NTNames#Mattatha">
        <rdf:type rdf:resource="http://semanticbible.org/ns/2006/NTNames#Man"/>
        <rdfs:label xml:lang="en">Mattatha</rdfs:label>
        <childOf rdf:resource="http://semanticbible.org/ns/2006/NTNames#Nathan"/>
    </owl:NamedIndividual>
    


    <!-- http://semanticbible.org/ns/2006/NTNames#MattathaisSonOfAmos -->

    <owl:NamedIndividual rdf:about="http://semanticbible.org/ns/2006/NTNames#MattathaisSonOfAmos">
        <rdfs:label xml:lang="en">Mattathias</rdfs:label>
    </owl:NamedIndividual>
    


    <!-- http://semanticbible.org/ns/2006/NTNames#MattathiasSonOfSemein -->

    <owl:NamedIndividual rdf:about="http://semanticbible.org/ns/2006/NTNames#MattathiasSonOfSemein">
        <rdfs:label xml:lang="en">Mattathias</rdfs:label>
        <parentOf rdf:resource="http://semanticbible.org/ns/2006/NTNames#Maath"/>
    </owl:NamedIndividual>
    


    <!-- http://semanticbible.org/ns/2006/NTNames#Matthan -->

    <owl:NamedIndividual rdf:about="http://semanticbible.org/ns/2006/NTNames#Matthan">
        <rdf:type rdf:resource="http://semanticbible.org/ns/2006/NTNames#Man"/>
        <rdfs:label xml:lang="en">Matthan</rdfs:label>
    </owl:NamedIndividual>
    


    <!-- http://semanticbible.org/ns/2006/NTNames#MatthatSonOfLeviSonOfMelki -->

    <owl:NamedIndividual rdf:about="http://semanticbible.org/ns/2006/NTNames#MatthatSonOfLeviSonOfMelki">
        <rdfs:label xml:lang="en">Matthat</rdfs:label>
    </owl:NamedIndividual>
    


    <!-- http://semanticbible.org/ns/2006/NTNames#MatthatSonOfLeviSonOfSimeon -->

    <owl:NamedIndividual rdf:about="http://semanticbible.org/ns/2006/NTNames#MatthatSonOfLeviSonOfSimeon">
        <rdfs:label xml:lang="en">Matthat</rdfs:label>
        <childOf rdf:resource="http://semanticbible.org/ns/2006/NTNames#LeviSonOfSimeon"/>
    </owl:NamedIndividual>
    


    <!-- http://semanticbible.org/ns/2006/NTNames#Matthias -->

    <owl:NamedIndividual rdf:about="http://semanticbible.org/ns/2006/NTNames#Matthias">
        <rdfs:label xml:lang="en">Matthias</rdfs:label>
    </owl:NamedIndividual>
    


    <!-- http://semanticbible.org/ns/2006/NTNames#Medes -->

    <owl:NamedIndividual rdf:about="http://semanticbible.org/ns/2006/NTNames#Medes">
        <rdfs:label xml:lang="en">Medes</rdfs:label>
    </owl:NamedIndividual>
    


    <!-- http://semanticbible.org/ns/2006/NTNames#MelchiSonOfAddi -->

    <owl:NamedIndividual rdf:about="http://semanticbible.org/ns/2006/NTNames#MelchiSonOfAddi">
        <rdfs:label xml:lang="en">Melchi</rdfs:label>
    </owl:NamedIndividual>
    


    <!-- http://semanticbible.org/ns/2006/NTNames#MelchiSonOfJannai -->

    <owl:NamedIndividual rdf:about="http://semanticbible.org/ns/2006/NTNames#MelchiSonOfJannai">
        <rdf:type rdf:resource="http://semanticbible.org/ns/2006/NTNames#Man"/>
        <rdfs:label xml:lang="en">Melchi</rdfs:label>
    </owl:NamedIndividual>
    


    <!-- http://semanticbible.org/ns/2006/NTNames#Melchizedek -->

    <owl:NamedIndividual rdf:about="http://semanticbible.org/ns/2006/NTNames#Melchizedek">
        <rdfs:label xml:lang="en">Melchizedek</rdfs:label>
    </owl:NamedIndividual>
    


    <!-- http://semanticbible.org/ns/2006/NTNames#Melea -->

    <owl:NamedIndividual rdf:about="http://semanticbible.org/ns/2006/NTNames#Melea">
        <rdfs:label xml:lang="en">Melea</rdfs:label>
    </owl:NamedIndividual>
    


    <!-- http://semanticbible.org/ns/2006/NTNames#Menna -->

    <owl:NamedIndividual rdf:about="http://semanticbible.org/ns/2006/NTNames#Menna">
        <rdf:type rdf:resource="http://semanticbible.org/ns/2006/NTNames#Man"/>
        <rdfs:label xml:lang="en">Menna</rdfs:label>
        <childOf rdf:resource="http://semanticbible.org/ns/2006/NTNames#Mattatha"/>
    </owl:NamedIndividual>
    


    <!-- http://semanticbible.org/ns/2006/NTNames#Mesopotamia -->

    <owl:NamedIndividual rdf:about="http://semanticbible.org/ns/2006/NTNames#Mesopotamia">
        <rdfs:label xml:lang="en">Mesopotamia</rdfs:label>
    </owl:NamedIndividual>
    


    <!-- http://semanticbible.org/ns/2006/NTNames#Methuselah -->

    <owl:NamedIndividual rdf:about="http://semanticbible.org/ns/2006/NTNames#Methuselah">
        <rdfs:label xml:lang="en">Methuselah</rdfs:label>
    </owl:NamedIndividual>
    


    <!-- http://semanticbible.org/ns/2006/NTNames#Michael -->

    <owl:NamedIndividual rdf:about="http://semanticbible.org/ns/2006/NTNames#Michael">
        <rdf:type rdf:resource="http://semanticbible.org/ns/2006/NTNames#Angel"/>
        <rdfs:label xml:lang="en">Michael</rdfs:label>
    </owl:NamedIndividual>
    


    <!-- http://semanticbible.org/ns/2006/NTNames#Midian -->

    <owl:NamedIndividual rdf:about="http://semanticbible.org/ns/2006/NTNames#Midian">
        <rdfs:label xml:lang="en">Midian</rdfs:label>
    </owl:NamedIndividual>
    


    <!-- http://semanticbible.org/ns/2006/NTNames#Miletus -->

    <owl:NamedIndividual rdf:about="http://semanticbible.org/ns/2006/NTNames#Miletus">
        <rdfs:label xml:lang="en">Miletus</rdfs:label>
    </owl:NamedIndividual>
    


    <!-- http://semanticbible.org/ns/2006/NTNames#MiletusGeodata -->

    <owl:NamedIndividual rdf:about="http://semanticbible.org/ns/2006/NTNames#MiletusGeodata">
        <rdfs:label xml:lang="en">geodata for Miletus</rdfs:label>
    </owl:NamedIndividual>
    


    <!-- http://semanticbible.org/ns/2006/NTNames#Mitylene -->

    <owl:NamedIndividual rdf:about="http://semanticbible.org/ns/2006/NTNames#Mitylene">
        <rdfs:label xml:lang="en">Mitylene</rdfs:label>
    </owl:NamedIndividual>
    


    <!-- http://semanticbible.org/ns/2006/NTNames#MityleneGeodata -->

    <owl:NamedIndividual rdf:about="http://semanticbible.org/ns/2006/NTNames#MityleneGeodata">
        <rdfs:label xml:lang="en">geodata for Mitylene</rdfs:label>
    </owl:NamedIndividual>
    


    <!-- http://semanticbible.org/ns/2006/NTNames#Mnason -->

    <owl:NamedIndividual rdf:about="http://semanticbible.org/ns/2006/NTNames#Mnason">
        <rdfs:label xml:lang="en">Mnason</rdfs:label>
    </owl:NamedIndividual>
    


    <!-- http://semanticbible.org/ns/2006/NTNames#Moabite -->

    <owl:NamedIndividual rdf:about="http://semanticbible.org/ns/2006/NTNames#Moabite">
        <rdfs:label xml:lang="en">Moabite</rdfs:label>
        <rdfs:comment xml:lang="en">Not mentioned in the New Testament: of the people of Moab, a non-Jewish group.</rdfs:comment>
    </owl:NamedIndividual>
    


    <!-- http://semanticbible.org/ns/2006/NTNames#Moloch -->

    <owl:NamedIndividual rdf:about="http://semanticbible.org/ns/2006/NTNames#Moloch">
        <rdfs:label xml:lang="en">Moloch</rdfs:label>
    </owl:NamedIndividual>
    


    <!-- http://semanticbible.org/ns/2006/NTNames#Moses -->

    <owl:NamedIndividual rdf:about="http://semanticbible.org/ns/2006/NTNames#Moses">
        <rdfs:label xml:lang="en">Moses</rdfs:label>
    </owl:NamedIndividual>
    


    <!-- http://semanticbible.org/ns/2006/NTNames#MountofOlivesGeodata -->

    <owl:NamedIndividual rdf:about="http://semanticbible.org/ns/2006/NTNames#MountofOlivesGeodata">
        <rdfs:label xml:lang="en">geodata for Mount of Olives</rdfs:label>
    </owl:NamedIndividual>
    


    <!-- http://semanticbible.org/ns/2006/NTNames#Myra -->

    <owl:NamedIndividual rdf:about="http://semanticbible.org/ns/2006/NTNames#Myra">
        <rdfs:label xml:lang="en">Myra</rdfs:label>
    </owl:NamedIndividual>
    


    <!-- http://semanticbible.org/ns/2006/NTNames#MyraGeodata -->

    <owl:NamedIndividual rdf:about="http://semanticbible.org/ns/2006/NTNames#MyraGeodata">
        <rdf:type rdf:resource="http://semanticbible.org/ns/2006/NTNames#GeographicLocation"/>
        <rdfs:label xml:lang="en">geodata for Myra</rdfs:label>
    </owl:NamedIndividual>
    


    <!-- http://semanticbible.org/ns/2006/NTNames#Mysia -->

    <owl:NamedIndividual rdf:about="http://semanticbible.org/ns/2006/NTNames#Mysia">
        <rdfs:label xml:lang="en">Mysia</rdfs:label>
    </owl:NamedIndividual>
    


    <!-- http://semanticbible.org/ns/2006/NTNames#Naaman -->

    <owl:NamedIndividual rdf:about="http://semanticbible.org/ns/2006/NTNames#Naaman">
        <rdfs:label xml:lang="en">Naaman</rdfs:label>
    </owl:NamedIndividual>
    


    <!-- http://semanticbible.org/ns/2006/NTNames#Naggai -->

    <owl:NamedIndividual rdf:about="http://semanticbible.org/ns/2006/NTNames#Naggai">
        <rdfs:label xml:lang="en">Naggai</rdfs:label>
    </owl:NamedIndividual>
    


    <!-- http://semanticbible.org/ns/2006/NTNames#Nahor -->

    <owl:NamedIndividual rdf:about="http://semanticbible.org/ns/2006/NTNames#Nahor">
        <rdfs:label xml:lang="en">Nahor</rdfs:label>
        <hasOnlyGenealogyMention rdf:datatype="http://www.w3.org/2001/XMLSchema#boolean">true</hasOnlyGenealogyMention>
    </owl:NamedIndividual>
    


    <!-- http://semanticbible.org/ns/2006/NTNames#Nahshon -->

    <owl:NamedIndividual rdf:about="http://semanticbible.org/ns/2006/NTNames#Nahshon">
        <rdfs:label xml:lang="en">Nahshon</rdfs:label>
    </owl:NamedIndividual>
    


    <!-- http://semanticbible.org/ns/2006/NTNames#Nahum -->

    <owl:NamedIndividual rdf:about="http://semanticbible.org/ns/2006/NTNames#Nahum">
        <rdfs:label xml:lang="en">Nahum</rdfs:label>
    </owl:NamedIndividual>
    


    <!-- http://semanticbible.org/ns/2006/NTNames#Nain -->

    <owl:NamedIndividual rdf:about="http://semanticbible.org/ns/2006/NTNames#Nain">
        <rdfs:label xml:lang="en">Nain</rdfs:label>
        <location rdf:resource="http://semanticbible.org/ns/2006/NTNames#NainGeodata"/>
    </owl:NamedIndividual>
    


    <!-- http://semanticbible.org/ns/2006/NTNames#NainGeodata -->

    <owl:NamedIndividual rdf:about="http://semanticbible.org/ns/2006/NTNames#NainGeodata">
        <rdfs:label xml:lang="en">geodata for Nain</rdfs:label>
    </owl:NamedIndividual>
    


    <!-- http://semanticbible.org/ns/2006/NTNames#Naphtali -->

    <owl:NamedIndividual rdf:about="http://semanticbible.org/ns/2006/NTNames#Naphtali">
        <rdfs:label xml:lang="en">Naphtali</rdfs:label>
        <siblingOf rdf:resource="http://semanticbible.org/ns/2006/NTNames#Gad"/>
    </owl:NamedIndividual>
    


    <!-- http://semanticbible.org/ns/2006/NTNames#Narcissus -->

    <owl:NamedIndividual rdf:about="http://semanticbible.org/ns/2006/NTNames#Narcissus">
        <rdf:type rdf:resource="http://semanticbible.org/ns/2006/NTNames#Man"/>
        <rdfs:label xml:lang="en">Narcissus</rdfs:label>
        <rdfs:comment rdf:datatype="http://www.w3.org/2001/XMLSchema#string">Paul addresses &quot;the family/household of Narcissus&quot;, which may refer to slaves: so we have no evidence about the beliefs or other attributes of Narcissus himself, other than his residence in Rome. </rdfs:comment>
    </owl:NamedIndividual>
    


    <!-- http://semanticbible.org/ns/2006/NTNames#Nathan -->

    <owl:NamedIndividual rdf:about="http://semanticbible.org/ns/2006/NTNames#Nathan">
        <rdfs:label xml:lang="en">Nathan</rdfs:label>
        <rdfs:comment xml:lang="en">This is not the prophet contemporary with King David, but David&#39;s son.</rdfs:comment>
    </owl:NamedIndividual>
    


    <!-- http://semanticbible.org/ns/2006/NTNames#Nazarene -->

    <owl:NamedIndividual rdf:about="http://semanticbible.org/ns/2006/NTNames#Nazarene">
        <rdfs:label xml:lang="en">Nazarene</rdfs:label>
    </owl:NamedIndividual>
    


    <!-- http://semanticbible.org/ns/2006/NTNames#Nazarenes -->

    <owl:NamedIndividual rdf:about="http://semanticbible.org/ns/2006/NTNames#Nazarenes">
        <rdfs:label xml:lang="en">Nazarenes</rdfs:label>
    </owl:NamedIndividual>
    


    <!-- http://semanticbible.org/ns/2006/NTNames#Nazareth -->

    <owl:NamedIndividual rdf:about="http://semanticbible.org/ns/2006/NTNames#Nazareth">
        <rdfs:label xml:lang="en">Nazareth</rdfs:label>
    </owl:NamedIndividual>
    


    <!-- http://semanticbible.org/ns/2006/NTNames#NazarethGeodata -->

    <owl:NamedIndividual rdf:about="http://semanticbible.org/ns/2006/NTNames#NazarethGeodata">
        <rdfs:label xml:lang="en">geodata for Nazareth</rdfs:label>
    </owl:NamedIndividual>
    


    <!-- http://semanticbible.org/ns/2006/NTNames#Neapolis -->

    <owl:NamedIndividual rdf:about="http://semanticbible.org/ns/2006/NTNames#Neapolis">
        <rdfs:label xml:lang="en">Neapolis</rdfs:label>
        <location rdf:resource="http://semanticbible.org/ns/2006/NTNames#NeapolisGeodata"/>
    </owl:NamedIndividual>
    


    <!-- http://semanticbible.org/ns/2006/NTNames#NeapolisGeodata -->

    <owl:NamedIndividual rdf:about="http://semanticbible.org/ns/2006/NTNames#NeapolisGeodata">
        <rdfs:label xml:lang="en">geodata for Neapolis</rdfs:label>
    </owl:NamedIndividual>
    


    <!-- http://semanticbible.org/ns/2006/NTNames#Nereus -->

    <owl:NamedIndividual rdf:about="http://semanticbible.org/ns/2006/NTNames#Nereus">
        <rdfs:label xml:lang="en">Nereus</rdfs:label>
    </owl:NamedIndividual>
    


    <!-- http://semanticbible.org/ns/2006/NTNames#Neri -->

    <owl:NamedIndividual rdf:about="http://semanticbible.org/ns/2006/NTNames#Neri">
        <rdfs:label xml:lang="en">Neri</rdfs:label>
    </owl:NamedIndividual>
    


    <!-- http://semanticbible.org/ns/2006/NTNames#Nicanor -->

    <owl:NamedIndividual rdf:about="http://semanticbible.org/ns/2006/NTNames#Nicanor">
        <rdfs:label xml:lang="en">Nicanor</rdfs:label>
    </owl:NamedIndividual>
    


    <!-- http://semanticbible.org/ns/2006/NTNames#Nicodemus -->

    <owl:NamedIndividual rdf:about="http://semanticbible.org/ns/2006/NTNames#Nicodemus">
        <rdfs:label xml:lang="en">Nicodemus</rdfs:label>
    </owl:NamedIndividual>
    


    <!-- http://semanticbible.org/ns/2006/NTNames#Nicolaitans -->

    <owl:NamedIndividual rdf:about="http://semanticbible.org/ns/2006/NTNames#Nicolaitans">
        <rdfs:label xml:lang="en">Nicolaitans</rdfs:label>
    </owl:NamedIndividual>
    


    <!-- http://semanticbible.org/ns/2006/NTNames#Nicolatianism -->

    <owl:NamedIndividual rdf:about="http://semanticbible.org/ns/2006/NTNames#Nicolatianism">
        <rdfs:label xml:lang="en">Nicolatianism</rdfs:label>
        <rdfs:comment xml:lang="en">Not referenced as a belief system in the New Testament.</rdfs:comment>
    </owl:NamedIndividual>
    


    <!-- http://semanticbible.org/ns/2006/NTNames#Nicolaus -->

    <owl:NamedIndividual rdf:about="http://semanticbible.org/ns/2006/NTNames#Nicolaus">
        <rdfs:label xml:lang="en">Nicolaus</rdfs:label>
    </owl:NamedIndividual>
    


    <!-- http://semanticbible.org/ns/2006/NTNames#Nicopolis -->

    <owl:NamedIndividual rdf:about="http://semanticbible.org/ns/2006/NTNames#Nicopolis">
        <rdfs:label xml:lang="en">Nicopolis</rdfs:label>
    </owl:NamedIndividual>
    


    <!-- http://semanticbible.org/ns/2006/NTNames#Niger -->

    <owl:NamedIndividual rdf:about="http://semanticbible.org/ns/2006/NTNames#Niger">
        <rdfs:label xml:lang="en">Niger</rdfs:label>
    </owl:NamedIndividual>
    


    <!-- http://semanticbible.org/ns/2006/NTNames#Nineveh -->

    <owl:NamedIndividual rdf:about="http://semanticbible.org/ns/2006/NTNames#Nineveh">
        <rdfs:label xml:lang="en">Nineveh</rdfs:label>
    </owl:NamedIndividual>
    


    <!-- http://semanticbible.org/ns/2006/NTNames#NinevehGeodata -->

    <owl:NamedIndividual rdf:about="http://semanticbible.org/ns/2006/NTNames#NinevehGeodata">
        <rdfs:label xml:lang="en">geodata for Nineveh</rdfs:label>
    </owl:NamedIndividual>
    


    <!-- http://semanticbible.org/ns/2006/NTNames#Noah -->

    <owl:NamedIndividual rdf:about="http://semanticbible.org/ns/2006/NTNames#Noah">
        <rdfs:label xml:lang="en">Noah</rdfs:label>
    </owl:NamedIndividual>
    


    <!-- http://semanticbible.org/ns/2006/NTNames#Nympha -->

    <owl:NamedIndividual rdf:about="http://semanticbible.org/ns/2006/NTNames#Nympha">
        <rdfs:label xml:lang="en">Nympha</rdfs:label>
        <rdfs:comment rdf:datatype="http://www.w3.org/2001/XMLSchema#string">The Church in Laodicea met in her house. Some manuscript variants indicate a man rather than a woman. </rdfs:comment>
        <collaboratesWith rdf:resource="http://semanticbible.org/ns/2006/NTNames#Paul"/>
    </owl:NamedIndividual>
    


    <!-- http://semanticbible.org/ns/2006/NTNames#Obed -->

    <owl:NamedIndividual rdf:about="http://semanticbible.org/ns/2006/NTNames#Obed">
        <rdfs:label xml:lang="en">Obed</rdfs:label>
        <parentOf rdf:resource="http://semanticbible.org/ns/2006/NTNames#Jesse"/>
        <ethnicity rdf:resource="http://semanticbible.org/ns/2006/NTNames#Jewish"/>
        <childOf rdf:resource="http://semanticbible.org/ns/2006/NTNames#Ruth"/>
    </owl:NamedIndividual>
    


    <!-- http://semanticbible.org/ns/2006/NTNames#Olivet -->

    <owl:NamedIndividual rdf:about="http://semanticbible.org/ns/2006/NTNames#Olivet">
        <rdfs:label xml:lang="en">Mount of Olives</rdfs:label>
        <rdfs:label xml:lang="en">Olivet</rdfs:label>
    </owl:NamedIndividual>
    


    <!-- http://semanticbible.org/ns/2006/NTNames#Olympas -->

    <owl:NamedIndividual rdf:about="http://semanticbible.org/ns/2006/NTNames#Olympas">
        <rdfs:label xml:lang="en">Olympas</rdfs:label>
    </owl:NamedIndividual>
    


    <!-- http://semanticbible.org/ns/2006/NTNames#Omega -->

    <owl:NamedIndividual rdf:about="http://semanticbible.org/ns/2006/NTNames#Omega">
        <rdfs:label xml:lang="en">Omega</rdfs:label>
    </owl:NamedIndividual>
    


    <!-- http://semanticbible.org/ns/2006/NTNames#Onesimus -->

    <owl:NamedIndividual rdf:about="http://semanticbible.org/ns/2006/NTNames#Onesimus">
        <rdfs:label xml:lang="en">Onesimus</rdfs:label>
    </owl:NamedIndividual>
    


    <!-- http://semanticbible.org/ns/2006/NTNames#Onesiphorus -->

    <owl:NamedIndividual rdf:about="http://semanticbible.org/ns/2006/NTNames#Onesiphorus">
        <rdfs:label xml:lang="en">Onesiphorus</rdfs:label>
    </owl:NamedIndividual>
    


    <!-- http://semanticbible.org/ns/2006/NTNames#Pamphylia -->

    <owl:NamedIndividual rdf:about="http://semanticbible.org/ns/2006/NTNames#Pamphylia">
        <rdfs:label xml:lang="en">Pamphylia</rdfs:label>
    </owl:NamedIndividual>
    


    <!-- http://semanticbible.org/ns/2006/NTNames#Paphos -->

    <owl:NamedIndividual rdf:about="http://semanticbible.org/ns/2006/NTNames#Paphos">
        <rdfs:label xml:lang="en">Paphos</rdfs:label>
    </owl:NamedIndividual>
    


    <!-- http://semanticbible.org/ns/2006/NTNames#PaphosGeodata -->

    <owl:NamedIndividual rdf:about="http://semanticbible.org/ns/2006/NTNames#PaphosGeodata">
        <rdfs:label xml:lang="en">geodata for Paphos</rdfs:label>
    </owl:NamedIndividual>
    


    <!-- http://semanticbible.org/ns/2006/NTNames#Parmenas -->

    <owl:NamedIndividual rdf:about="http://semanticbible.org/ns/2006/NTNames#Parmenas">
        <rdf:type rdf:resource="http://semanticbible.org/ns/2006/NTNames#Man"/>
        <rdfs:label xml:lang="en">Parmenas</rdfs:label>
    </owl:NamedIndividual>
    


    <!-- http://semanticbible.org/ns/2006/NTNames#Parthia -->

    <owl:NamedIndividual rdf:about="http://semanticbible.org/ns/2006/NTNames#Parthia">
        <rdfs:comment rdf:datatype="http://www.w3.org/2001/XMLSchema#string">Part of the ancient empire of Persia, though under Roman domination in New Testmament times.</rdfs:comment>
    </owl:NamedIndividual>
    


    <!-- http://semanticbible.org/ns/2006/NTNames#Parthians -->

    <owl:NamedIndividual rdf:about="http://semanticbible.org/ns/2006/NTNames#Parthians">
        <rdfs:label xml:lang="en">Parthians</rdfs:label>
    </owl:NamedIndividual>
    


    <!-- http://semanticbible.org/ns/2006/NTNames#PartyOfZealots -->

    <owl:NamedIndividual rdf:about="http://semanticbible.org/ns/2006/NTNames#PartyOfZealots">
        <rdf:type rdf:resource="http://semanticbible.org/ns/2006/NTNames#PoliticalBeliefSystem"/>
        <rdfs:label xml:lang="en">Party of Zealots</rdfs:label>
    </owl:NamedIndividual>
    


    <!-- http://semanticbible.org/ns/2006/NTNames#Passover -->

    <owl:NamedIndividual rdf:about="http://semanticbible.org/ns/2006/NTNames#Passover">
        <rdfs:label xml:lang="en">Passover</rdfs:label>
    </owl:NamedIndividual>
    


    <!-- http://semanticbible.org/ns/2006/NTNames#Patara -->

    <owl:NamedIndividual rdf:about="http://semanticbible.org/ns/2006/NTNames#Patara">
        <rdfs:label xml:lang="en">Patara</rdfs:label>
    </owl:NamedIndividual>
    


    <!-- http://semanticbible.org/ns/2006/NTNames#PataraGeodata -->

    <owl:NamedIndividual rdf:about="http://semanticbible.org/ns/2006/NTNames#PataraGeodata">
        <rdf:type rdf:resource="http://semanticbible.org/ns/2006/NTNames#GeographicLocation"/>
        <rdfs:label xml:lang="en">geodata for Patara</rdfs:label>
    </owl:NamedIndividual>
    


    <!-- http://semanticbible.org/ns/2006/NTNames#Patmos -->

    <owl:NamedIndividual rdf:about="http://semanticbible.org/ns/2006/NTNames#Patmos">
        <rdfs:label xml:lang="en">Patmos</rdfs:label>
    </owl:NamedIndividual>
    


    <!-- http://semanticbible.org/ns/2006/NTNames#Patrobas -->

    <owl:NamedIndividual rdf:about="http://semanticbible.org/ns/2006/NTNames#Patrobas">
        <rdfs:label xml:lang="en">Patrobas</rdfs:label>
    </owl:NamedIndividual>
    


    <!-- http://semanticbible.org/ns/2006/NTNames#Paul -->

    <owl:NamedIndividual rdf:about="http://semanticbible.org/ns/2006/NTNames#Paul">
        <rdfs:label xml:lang="en">Paul</rdfs:label>
        <rdfs:comment xml:lang="en">The Apostle Paul was known earlier as Saul: he was given the name Paul when he was converted.</rdfs:comment>
        <knows rdf:resource="http://semanticbible.org/ns/2006/NTNames#Epaenetus"/>
        <hasEnemy rdf:resource="http://semanticbible.org/ns/2006/NTNames#Felix"/>
        <collaboratesWith rdf:resource="http://semanticbible.org/ns/2006/NTNames#GaiusOfDerbe"/>
        <knows rdf:resource="http://semanticbible.org/ns/2006/NTNames#Nereus"/>
        <collaboratesWith rdf:resource="http://semanticbible.org/ns/2006/NTNames#Nympha"/>
        <collaboratesWith rdf:resource="http://semanticbible.org/ns/2006/NTNames#Syntyche"/>
    </owl:NamedIndividual>
    


    <!-- http://semanticbible.org/ns/2006/NTNames#Peleg -->

    <owl:NamedIndividual rdf:about="http://semanticbible.org/ns/2006/NTNames#Peleg">
        <rdfs:label xml:lang="en">Peleg</rdfs:label>
        <description rdf:datatype="http://www.w3.org/2001/XMLSchema#string">One of the ancestors of Jesus mentioned in Luke&#39;s geneaology</description>
    </owl:NamedIndividual>
    


    <!-- http://semanticbible.org/ns/2006/NTNames#Pentecost -->

    <owl:NamedIndividual rdf:about="http://semanticbible.org/ns/2006/NTNames#Pentecost">
        <rdfs:label xml:lang="en">Pentecost</rdfs:label>
    </owl:NamedIndividual>
    


    <!-- http://semanticbible.org/ns/2006/NTNames#Perez -->

    <owl:NamedIndividual rdf:about="http://semanticbible.org/ns/2006/NTNames#Perez">
        <rdfs:label xml:lang="en">Perez</rdfs:label>
        <hasOnlyGenealogyMention rdf:datatype="http://www.w3.org/2001/XMLSchema#boolean">true</hasOnlyGenealogyMention>
    </owl:NamedIndividual>
    


    <!-- http://semanticbible.org/ns/2006/NTNames#Perga -->

    <owl:NamedIndividual rdf:about="http://semanticbible.org/ns/2006/NTNames#Perga">
        <rdfs:label xml:lang="en">Perga</rdfs:label>
    </owl:NamedIndividual>
    


    <!-- http://semanticbible.org/ns/2006/NTNames#PergaGeodata -->

    <owl:NamedIndividual rdf:about="http://semanticbible.org/ns/2006/NTNames#PergaGeodata">
        <rdfs:label xml:lang="en">geodata for Perga</rdfs:label>
    </owl:NamedIndividual>
    


    <!-- http://semanticbible.org/ns/2006/NTNames#Pergamum -->

    <owl:NamedIndividual rdf:about="http://semanticbible.org/ns/2006/NTNames#Pergamum">
        <rdfs:label xml:lang="en">Pergamum</rdfs:label>
    </owl:NamedIndividual>
    


    <!-- http://semanticbible.org/ns/2006/NTNames#Persis -->

    <owl:NamedIndividual rdf:about="http://semanticbible.org/ns/2006/NTNames#Persis">
        <rdfs:label xml:lang="en">Persis</rdfs:label>
        <description rdf:datatype="http://www.w3.org/2001/XMLSchema#string">One who worked hard in the Lord among the Roman Christians</description>
        <knows rdf:resource="http://semanticbible.org/ns/2006/NTNames#Priscilla"/>
    </owl:NamedIndividual>
    


    <!-- http://semanticbible.org/ns/2006/NTNames#Phanuel -->

    <owl:NamedIndividual rdf:about="http://semanticbible.org/ns/2006/NTNames#Phanuel">
        <rdfs:label xml:lang="en">Phanuel</rdfs:label>
    </owl:NamedIndividual>
    


    <!-- http://semanticbible.org/ns/2006/NTNames#Pharaoh -->

    <owl:NamedIndividual rdf:about="http://semanticbible.org/ns/2006/NTNames#Pharaoh">
        <rdfs:label xml:lang="en">Pharaoh</rdfs:label>
        <rdfs:comment xml:lang="en">Pharaoh is actually a title rather than a personal name, but in the New Testament it refers to a single individual.</rdfs:comment>
    </owl:NamedIndividual>
    


    <!-- http://semanticbible.org/ns/2006/NTNames#Pharisee -->

    <owl:NamedIndividual rdf:about="http://semanticbible.org/ns/2006/NTNames#Pharisee">
        <rdfs:label xml:lang="en">Pharisee</rdfs:label>
        <rdfs:comment rdf:datatype="http://www.w3.org/2001/XMLSchema#string">Having a ReligiousBelief of Pharisee implies the belief of Jew as well. </rdfs:comment>
    </owl:NamedIndividual>
    


    <!-- http://semanticbible.org/ns/2006/NTNames#Phariseeism -->

    <owl:NamedIndividual rdf:about="http://semanticbible.org/ns/2006/NTNames#Phariseeism">
        <rdfs:label xml:lang="en">Phariseeism</rdfs:label>
        <rdfs:comment xml:lang="en">The beliefs of one of the main Jewish sects during the life of Jesus. In the New Testament the name of the sect is used, though not the belief system per se.</rdfs:comment>
    </owl:NamedIndividual>
    


    <!-- http://semanticbible.org/ns/2006/NTNames#Pharisees -->

    <owl:NamedIndividual rdf:about="http://semanticbible.org/ns/2006/NTNames#Pharisees">
        <rdfs:label xml:lang="en">Pharisees</rdfs:label>
    </owl:NamedIndividual>
    


    <!-- http://semanticbible.org/ns/2006/NTNames#Philadelphia -->

    <owl:NamedIndividual rdf:about="http://semanticbible.org/ns/2006/NTNames#Philadelphia">
        <rdfs:label xml:lang="en">Philadelphia</rdfs:label>
    </owl:NamedIndividual>
    


    <!-- http://semanticbible.org/ns/2006/NTNames#PhiladelphiaGeodata -->

    <owl:NamedIndividual rdf:about="http://semanticbible.org/ns/2006/NTNames#PhiladelphiaGeodata">
        <rdfs:label xml:lang="en">geodata for Philadelphia</rdfs:label>
    </owl:NamedIndividual>
    


    <!-- http://semanticbible.org/ns/2006/NTNames#Philemon -->

    <owl:NamedIndividual rdf:about="http://semanticbible.org/ns/2006/NTNames#Philemon">
        <rdfs:label xml:lang="en">Philemon</rdfs:label>
        <rdfs:comment xml:lang="en">His residence in Colossae is implied from his relationship to Archippus and Onesimus (Col.4.9; Col.4.17). He may have been been a native as well. 
Paul describes him as &quot;our beloved fellow worker&quot;.</rdfs:comment>
    </owl:NamedIndividual>
    


    <!-- http://semanticbible.org/ns/2006/NTNames#Philetus -->

    <owl:NamedIndividual rdf:about="http://semanticbible.org/ns/2006/NTNames#Philetus">
        <rdfs:label xml:lang="en">Philetus</rdfs:label>
    </owl:NamedIndividual>
    


    <!-- http://semanticbible.org/ns/2006/NTNames#Philip -->

    <owl:NamedIndividual rdf:about="http://semanticbible.org/ns/2006/NTNames#Philip">
        <rdfs:label xml:lang="en">Philip</rdfs:label>
    </owl:NamedIndividual>
    


    <!-- http://semanticbible.org/ns/2006/NTNames#PhilipSonOfHerod -->

    <owl:NamedIndividual rdf:about="http://semanticbible.org/ns/2006/NTNames#PhilipSonOfHerod">
        <rdf:type rdf:resource="http://semanticbible.org/ns/2006/NTNames#Man"/>
        <rdfs:label xml:lang="en">Philip</rdfs:label>
        <spouseOf rdf:resource="http://semanticbible.org/ns/2006/NTNames#Herodias"/>
    </owl:NamedIndividual>
    


    <!-- http://semanticbible.org/ns/2006/NTNames#Philippi -->

    <owl:NamedIndividual rdf:about="http://semanticbible.org/ns/2006/NTNames#Philippi">
        <rdfs:label xml:lang="en">Philippi</rdfs:label>
        <location rdf:resource="http://semanticbible.org/ns/2006/NTNames#PhilippiGeodata"/>
    </owl:NamedIndividual>
    


    <!-- http://semanticbible.org/ns/2006/NTNames#PhilippiGeodata -->

    <owl:NamedIndividual rdf:about="http://semanticbible.org/ns/2006/NTNames#PhilippiGeodata">
        <rdfs:label xml:lang="en">geodata for Philippi</rdfs:label>
        <longitude rdf:datatype="http://www.w3.org/2001/XMLSchema#double">24.28828605219695</longitude>
    </owl:NamedIndividual>
    


    <!-- http://semanticbible.org/ns/2006/NTNames#Philippians -->

    <owl:NamedIndividual rdf:about="http://semanticbible.org/ns/2006/NTNames#Philippians">
        <rdfs:label xml:lang="en">Philippians</rdfs:label>
    </owl:NamedIndividual>
    


    <!-- http://semanticbible.org/ns/2006/NTNames#Philologus -->

    <owl:NamedIndividual rdf:about="http://semanticbible.org/ns/2006/NTNames#Philologus">
        <rdfs:label xml:lang="en">Philologus</rdfs:label>
    </owl:NamedIndividual>
    


    <!-- http://semanticbible.org/ns/2006/NTNames#Phlegon -->

    <owl:NamedIndividual rdf:about="http://semanticbible.org/ns/2006/NTNames#Phlegon">
        <rdfs:label xml:lang="en">Phlegon</rdfs:label>
        <hasOnlyGenealogyMention rdf:datatype="http://www.w3.org/2001/XMLSchema#boolean">false</hasOnlyGenealogyMention>
    </owl:NamedIndividual>
    


    <!-- http://semanticbible.org/ns/2006/NTNames#Phoebe -->

    <owl:NamedIndividual rdf:about="http://semanticbible.org/ns/2006/NTNames#Phoebe">
        <rdfs:label xml:lang="en">Phoebe</rdfs:label>
        <rdfs:comment xml:lang="en">Paul&#39;s commendation of Phoebe in Romans strongly suggests she delivered the letter</rdfs:comment>
    </owl:NamedIndividual>
    


    <!-- http://semanticbible.org/ns/2006/NTNames#Phoenicia -->

    <owl:NamedIndividual rdf:about="http://semanticbible.org/ns/2006/NTNames#Phoenicia">
        <rdfs:label xml:lang="en">Phoenicia</rdfs:label>
    </owl:NamedIndividual>
    


    <!-- http://semanticbible.org/ns/2006/NTNames#Phoenix -->

    <owl:NamedIndividual rdf:about="http://semanticbible.org/ns/2006/NTNames#Phoenix">
        <rdfs:label xml:lang="en">Phoenix</rdfs:label>
    </owl:NamedIndividual>
    


    <!-- http://semanticbible.org/ns/2006/NTNames#PhoenixGeodata -->

    <owl:NamedIndividual rdf:about="http://semanticbible.org/ns/2006/NTNames#PhoenixGeodata">
        <rdfs:label xml:lang="en">geodata for Phoenix</rdfs:label>
        <longitude rdf:datatype="http://www.w3.org/2001/XMLSchema#double">24.01414490625663</longitude>
    </owl:NamedIndividual>
    


    <!-- http://semanticbible.org/ns/2006/NTNames#Phrygia -->

    <owl:NamedIndividual rdf:about="http://semanticbible.org/ns/2006/NTNames#Phrygia">
        <rdf:type rdf:resource="http://semanticbible.org/ns/2006/NTNames#Region"/>
        <rdfs:label xml:lang="en">Phrygia</rdfs:label>
    </owl:NamedIndividual>
    


    <!-- http://semanticbible.org/ns/2006/NTNames#Phygelus -->

    <owl:NamedIndividual rdf:about="http://semanticbible.org/ns/2006/NTNames#Phygelus">
        <rdfs:label xml:lang="en">Phygelus</rdfs:label>
        <rdfs:comment xml:lang="en">The circumstances behind his &quot;turning away&quot; from Paul are unknown. Likewise, Paul&#39;s description of him as being &quot;is Asia&quot; isn&#39;t specific enough to assign a place. </rdfs:comment>
    </owl:NamedIndividual>
    


    <!-- http://semanticbible.org/ns/2006/NTNames#Pilate -->

    <owl:NamedIndividual rdf:about="http://semanticbible.org/ns/2006/NTNames#Pilate">
        <rdfs:label xml:lang="en">Pilate</rdfs:label>
    </owl:NamedIndividual>
    


    <!-- http://semanticbible.org/ns/2006/NTNames#Pisidia -->

    <owl:NamedIndividual rdf:about="http://semanticbible.org/ns/2006/NTNames#Pisidia">
        <rdfs:label xml:lang="en">Pisidia</rdfs:label>
    </owl:NamedIndividual>
    


    <!-- http://semanticbible.org/ns/2006/NTNames#PontiusPilate -->

    <owl:NamedIndividual rdf:about="http://semanticbible.org/ns/2006/NTNames#PontiusPilate">
        <rdfs:label xml:lang="en">Pontius Pilate</rdfs:label>
        <collaboratesWith rdf:resource="http://semanticbible.org/ns/2006/NTNames#HerodAntipas"/>
    </owl:NamedIndividual>
    


    <!-- http://semanticbible.org/ns/2006/NTNames#Pontus -->

    <owl:NamedIndividual rdf:about="http://semanticbible.org/ns/2006/NTNames#Pontus">
        <rdfs:label xml:lang="en">Pontus</rdfs:label>
    </owl:NamedIndividual>
    


    <!-- http://semanticbible.org/ns/2006/NTNames#Porcius -->

    <owl:NamedIndividual rdf:about="http://semanticbible.org/ns/2006/NTNames#Porcius">
        <rdfs:label xml:lang="en">Porcius</rdfs:label>
    </owl:NamedIndividual>
    


    <!-- http://semanticbible.org/ns/2006/NTNames#Priscilla -->

    <owl:NamedIndividual rdf:about="http://semanticbible.org/ns/2006/NTNames#Priscilla">
        <rdf:type rdf:resource="http://semanticbible.org/ns/2006/NTNames#Woman"/>
        <rdfs:label xml:lang="en">Prisca</rdfs:label>
        <rdfs:label xml:lang="en">Priscilla</rdfs:label>
        <rdfs:comment rdf:datatype="http://www.w3.org/2001/XMLSchema#string">Prisca is the diminutive form of Priscilla. Brownrigg notes that Paul always uses this form.</rdfs:comment>
        <knows rdf:resource="http://semanticbible.org/ns/2006/NTNames#Epaenetus"/>
        <knows rdf:resource="http://semanticbible.org/ns/2006/NTNames#Persis"/>
        <knows rdf:resource="http://semanticbible.org/ns/2006/NTNames#Stachys"/>
        <knows rdf:resource="http://semanticbible.org/ns/2006/NTNames#Urbanus"/>
    </owl:NamedIndividual>
    


    <!-- http://semanticbible.org/ns/2006/NTNames#Prochorus -->

    <owl:NamedIndividual rdf:about="http://semanticbible.org/ns/2006/NTNames#Prochorus">
        <rdfs:label xml:lang="en">Prochorus</rdfs:label>
    </owl:NamedIndividual>
    


    <!-- http://semanticbible.org/ns/2006/NTNames#Ptolemais -->

    <owl:NamedIndividual rdf:about="http://semanticbible.org/ns/2006/NTNames#Ptolemais">
        <rdfs:label xml:lang="en">Ptolemais</rdfs:label>
    </owl:NamedIndividual>
    


    <!-- http://semanticbible.org/ns/2006/NTNames#Publius -->

    <owl:NamedIndividual rdf:about="http://semanticbible.org/ns/2006/NTNames#Publius">
        <rdf:type rdf:resource="http://semanticbible.org/ns/2006/NTNames#Man"/>
        <rdfs:label xml:lang="en">Publius</rdfs:label>
    </owl:NamedIndividual>
    


    <!-- http://semanticbible.org/ns/2006/NTNames#Pudens -->

    <owl:NamedIndividual rdf:about="http://semanticbible.org/ns/2006/NTNames#Pudens">
        <rdfs:label xml:lang="en">Pudens</rdfs:label>
    </owl:NamedIndividual>
    


    <!-- http://semanticbible.org/ns/2006/NTNames#Puteoli -->

    <owl:NamedIndividual rdf:about="http://semanticbible.org/ns/2006/NTNames#Puteoli">
        <rdfs:label xml:lang="en">Puteoli</rdfs:label>
        <location rdf:resource="http://semanticbible.org/ns/2006/NTNames#PuteoliGeodata"/>
    </owl:NamedIndividual>
    


    <!-- http://semanticbible.org/ns/2006/NTNames#PuteoliGeodata -->

    <owl:NamedIndividual rdf:about="http://semanticbible.org/ns/2006/NTNames#PuteoliGeodata">
        <rdfs:label xml:lang="en">geodata for Puteoli</rdfs:label>
    </owl:NamedIndividual>
    


    <!-- http://semanticbible.org/ns/2006/NTNames#Pyrrhus -->

    <owl:NamedIndividual rdf:about="http://semanticbible.org/ns/2006/NTNames#Pyrrhus">
        <rdfs:label xml:lang="en">Pyrrhus</rdfs:label>
    </owl:NamedIndividual>
    


    <!-- http://semanticbible.org/ns/2006/NTNames#Quartus -->

    <owl:NamedIndividual rdf:about="http://semanticbible.org/ns/2006/NTNames#Quartus">
        <rdfs:label xml:lang="en">Quartus</rdfs:label>
    </owl:NamedIndividual>
    


    <!-- http://semanticbible.org/ns/2006/NTNames#Quirinius -->

    <owl:NamedIndividual rdf:about="http://semanticbible.org/ns/2006/NTNames#Quirinius">
        <rdfs:label xml:lang="en">Quirinius</rdfs:label>
    </owl:NamedIndividual>
    


    <!-- http://semanticbible.org/ns/2006/NTNames#Rachel -->

    <owl:NamedIndividual rdf:about="http://semanticbible.org/ns/2006/NTNames#Rachel">
        <rdf:type rdf:resource="http://semanticbible.org/ns/2006/NTNames#Woman"/>
        <rdfs:label xml:lang="en">Rachel</rdfs:label>
        <rdfs:comment xml:lang="en">Daughter of Laban and sister of Leah, who are not named in the New Testament. </rdfs:comment>
    </owl:NamedIndividual>
    


    <!-- http://semanticbible.org/ns/2006/NTNames#Rahab -->

    <owl:NamedIndividual rdf:about="http://semanticbible.org/ns/2006/NTNames#Rahab">
        <rdfs:label xml:lang="en">Rahab</rdfs:label>
        <parentOf rdf:resource="http://semanticbible.org/ns/2006/NTNames#Boaz"/>
    </owl:NamedIndividual>
    


    <!-- http://semanticbible.org/ns/2006/NTNames#Ram -->

    <owl:NamedIndividual rdf:about="http://semanticbible.org/ns/2006/NTNames#Ram">
        <rdfs:label xml:lang="en">Ram</rdfs:label>
        <parentOf rdf:resource="http://semanticbible.org/ns/2006/NTNames#Amminadab"/>
        <ethnicity rdf:resource="http://semanticbible.org/ns/2006/NTNames#Jewish"/>
    </owl:NamedIndividual>
    


    <!-- http://semanticbible.org/ns/2006/NTNames#Ramah -->

    <owl:NamedIndividual rdf:about="http://semanticbible.org/ns/2006/NTNames#Ramah">
        <rdfs:label xml:lang="en">Ramah</rdfs:label>
        <rdfs:comment rdf:datatype="http://www.w3.org/2001/XMLSchema#string">The only NT reference is a quotation from Jer 31:15: this presumably refers to Ramah near Bethel. </rdfs:comment>
        <location rdf:resource="http://semanticbible.org/ns/2006/NTNames#RamahGeodata"/>
    </owl:NamedIndividual>
    


    <!-- http://semanticbible.org/ns/2006/NTNames#RamahGeodata -->

    <owl:NamedIndividual rdf:about="http://semanticbible.org/ns/2006/NTNames#RamahGeodata">
        <rdfs:label xml:lang="en">geodata for Ramah</rdfs:label>
    </owl:NamedIndividual>
    


    <!-- http://semanticbible.org/ns/2006/NTNames#Rebecca -->

    <owl:NamedIndividual rdf:about="http://semanticbible.org/ns/2006/NTNames#Rebecca">
        <rdfs:label xml:lang="en">Rebecca</rdfs:label>
        <rdfs:comment rdf:datatype="http://www.w3.org/2001/XMLSchema#string">Brother of Laban, who is not named in the New Testament. </rdfs:comment>
        <parentOf rdf:resource="http://semanticbible.org/ns/2006/NTNames#Esau"/>
    </owl:NamedIndividual>
    


    <!-- http://semanticbible.org/ns/2006/NTNames#Rehoboam -->

    <owl:NamedIndividual rdf:about="http://semanticbible.org/ns/2006/NTNames#Rehoboam">
        <rdfs:label xml:lang="en">Rehoboam</rdfs:label>
        <rdfs:comment rdf:datatype="http://www.w3.org/2001/XMLSchema#string">His occupation as king comes from the Old Testament, 1Kgs.12-14</rdfs:comment>
    </owl:NamedIndividual>
    


    <!-- http://semanticbible.org/ns/2006/NTNames#Rephan -->

    <owl:NamedIndividual rdf:about="http://semanticbible.org/ns/2006/NTNames#Rephan">
        <rdfs:label xml:lang="en">Rephan</rdfs:label>
    </owl:NamedIndividual>
    


    <!-- http://semanticbible.org/ns/2006/NTNames#Reu -->

    <owl:NamedIndividual rdf:about="http://semanticbible.org/ns/2006/NTNames#Reu">
        <rdfs:label xml:lang="en">Reu</rdfs:label>
        <childOf rdf:resource="http://semanticbible.org/ns/2006/NTNames#Peleg"/>
        <parentOf rdf:resource="http://semanticbible.org/ns/2006/NTNames#Serug"/>
    </owl:NamedIndividual>
    


    <!-- http://semanticbible.org/ns/2006/NTNames#Reuben -->

    <owl:NamedIndividual rdf:about="http://semanticbible.org/ns/2006/NTNames#Reuben">
        <rdf:type rdf:resource="http://semanticbible.org/ns/2006/NTNames#Man"/>
        <rdfs:label xml:lang="en">Reuben</rdfs:label>
    </owl:NamedIndividual>
    


    <!-- http://semanticbible.org/ns/2006/NTNames#Rhegium -->

    <owl:NamedIndividual rdf:about="http://semanticbible.org/ns/2006/NTNames#Rhegium">
        <rdfs:label xml:lang="en">Rhegium</rdfs:label>
    </owl:NamedIndividual>
    


    <!-- http://semanticbible.org/ns/2006/NTNames#RhegiumGeodata -->

    <owl:NamedIndividual rdf:about="http://semanticbible.org/ns/2006/NTNames#RhegiumGeodata">
        <rdfs:label xml:lang="en">geodata for Rhegium</rdfs:label>
    </owl:NamedIndividual>
    


    <!-- http://semanticbible.org/ns/2006/NTNames#Rhesa -->

    <owl:NamedIndividual rdf:about="http://semanticbible.org/ns/2006/NTNames#Rhesa">
        <rdfs:label xml:lang="en">Rhesa</rdfs:label>
    </owl:NamedIndividual>
    


    <!-- http://semanticbible.org/ns/2006/NTNames#Rhoda -->

    <owl:NamedIndividual rdf:about="http://semanticbible.org/ns/2006/NTNames#Rhoda">
        <rdfs:label xml:lang="en">Rhoda</rdfs:label>
        <rdfs:comment rdf:datatype="http://www.w3.org/2001/XMLSchema#string">One might infer Rhoda was a Christian because of her mistress&#39; faith, and her joy in seeing Peter after his release.</rdfs:comment>
    </owl:NamedIndividual>
    


    <!-- http://semanticbible.org/ns/2006/NTNames#Rhodes -->

    <owl:NamedIndividual rdf:about="http://semanticbible.org/ns/2006/NTNames#Rhodes">
        <rdf:type rdf:resource="http://semanticbible.org/ns/2006/NTNames#Island"/>
        <rdfs:label xml:lang="en">Rhodes</rdfs:label>
        <location rdf:resource="http://semanticbible.org/ns/2006/NTNames#RhodesGeodata"/>
    </owl:NamedIndividual>
    


    <!-- http://semanticbible.org/ns/2006/NTNames#RhodesGeodata -->

    <owl:NamedIndividual rdf:about="http://semanticbible.org/ns/2006/NTNames#RhodesGeodata">
        <rdf:type rdf:resource="http://semanticbible.org/ns/2006/NTNames#GeographicLocation"/>
        <rdfs:label xml:lang="en">geodata for Rhodes</rdfs:label>
        <altitude rdf:datatype="http://www.w3.org/2001/XMLSchema#int">0</altitude>
    </owl:NamedIndividual>
    


    <!-- http://semanticbible.org/ns/2006/NTNames#Roman -->

    <owl:NamedIndividual rdf:about="http://semanticbible.org/ns/2006/NTNames#Roman">
        <rdfs:label xml:lang="en">Roman</rdfs:label>
        <ethnicityOf rdf:resource="http://semanticbible.org/ns/2006/NTNames#CaesarNero"/>
    </owl:NamedIndividual>
    


    <!-- http://semanticbible.org/ns/2006/NTNames#RomanCitizenship -->

    <owl:NamedIndividual rdf:about="http://semanticbible.org/ns/2006/NTNames#RomanCitizenship">
        <rdfs:label xml:lang="en">Roman</rdfs:label>
    </owl:NamedIndividual>
    


    <!-- http://semanticbible.org/ns/2006/NTNames#Romans -->

    <owl:NamedIndividual rdf:about="http://semanticbible.org/ns/2006/NTNames#Romans">
        <rdfs:label xml:lang="en">Romans</rdfs:label>
    </owl:NamedIndividual>
    


    <!-- http://semanticbible.org/ns/2006/NTNames#Rome -->

    <owl:NamedIndividual rdf:about="http://semanticbible.org/ns/2006/NTNames#Rome">
        <rdfs:label xml:lang="en">Rome</rdfs:label>
        <residentPlaceOf rdf:resource="http://semanticbible.org/ns/2006/NTNames#Claudia"/>
        <residentPlaceOf rdf:resource="http://semanticbible.org/ns/2006/NTNames#Eubulus"/>
        <residentPlaceOf rdf:resource="http://semanticbible.org/ns/2006/NTNames#Patrobas"/>
        <residentPlaceOf rdf:resource="http://semanticbible.org/ns/2006/NTNames#Priscilla"/>
    </owl:NamedIndividual>
    


    <!-- http://semanticbible.org/ns/2006/NTNames#Rufus -->

    <owl:NamedIndividual rdf:about="http://semanticbible.org/ns/2006/NTNames#Rufus">
        <rdfs:label xml:lang="en">Rufus</rdfs:label>
        <siblingOf rdf:resource="http://semanticbible.org/ns/2006/NTNames#Alexander"/>
    </owl:NamedIndividual>
    


    <!-- http://semanticbible.org/ns/2006/NTNames#RufusOfRome -->

    <owl:NamedIndividual rdf:about="http://semanticbible.org/ns/2006/NTNames#RufusOfRome">
        <rdfs:comment rdf:datatype="http://www.w3.org/2001/XMLSchema#string">There are no firm grounds for identifying this Rufus as the same person as the son of Simon of Cyrene mentioned in Mark 15 (though the tradition that Mark&#39;s Gospel was written in Rome makes this an intriguing possibility). </rdfs:comment>
        <possiblySamePersonAs rdf:resource="http://semanticbible.org/ns/2006/NTNames#Rufus"/>
    </owl:NamedIndividual>
    


    <!-- http://semanticbible.org/ns/2006/NTNames#Ruth -->

    <owl:NamedIndividual rdf:about="http://semanticbible.org/ns/2006/NTNames#Ruth">
        <rdfs:label xml:lang="en">Ruth</rdfs:label>
        <rdfs:comment xml:lang="en">An Old Testament figure</rdfs:comment>
    </owl:NamedIndividual>
    


    <!-- http://semanticbible.org/ns/2006/NTNames#Sabbath -->

    <owl:NamedIndividual rdf:about="http://semanticbible.org/ns/2006/NTNames#Sabbath">
        <rdfs:label xml:lang="en">Sabbath</rdfs:label>
    </owl:NamedIndividual>
    


    <!-- http://semanticbible.org/ns/2006/NTNames#Sadduceanism -->

    <owl:NamedIndividual rdf:about="http://semanticbible.org/ns/2006/NTNames#Sadduceanism">
        <rdfs:label xml:lang="en">Sadduceanism</rdfs:label>
        <rdfs:comment xml:lang="en">The beliefs of one of the main Jewish sects during the life of Jesus. In the New Testament the name of the sect is used, though not the belief system per se.</rdfs:comment>
    </owl:NamedIndividual>
    


    <!-- http://semanticbible.org/ns/2006/NTNames#Sadducees -->

    <owl:NamedIndividual rdf:about="http://semanticbible.org/ns/2006/NTNames#Sadducees">
        <rdfs:label xml:lang="en">Sadducees</rdfs:label>
    </owl:NamedIndividual>
    


    <!-- http://semanticbible.org/ns/2006/NTNames#Salamis -->

    <owl:NamedIndividual rdf:about="http://semanticbible.org/ns/2006/NTNames#Salamis">
        <rdfs:label xml:lang="en">Salamis</rdfs:label>
        <location rdf:resource="http://semanticbible.org/ns/2006/NTNames#SalamisGeodata"/>
    </owl:NamedIndividual>
    


    <!-- http://semanticbible.org/ns/2006/NTNames#SalamisGeodata -->

    <owl:NamedIndividual rdf:about="http://semanticbible.org/ns/2006/NTNames#SalamisGeodata">
        <rdfs:label xml:lang="en">geodata for Salamis</rdfs:label>
    </owl:NamedIndividual>
    


    <!-- http://semanticbible.org/ns/2006/NTNames#Salem -->

    <owl:NamedIndividual rdf:about="http://semanticbible.org/ns/2006/NTNames#Salem">
        <rdfs:label xml:lang="en">Salem</rdfs:label>
        <rdfs:comment rdf:datatype="http://www.w3.org/2001/XMLSchema#string">Geodata assumes this is an earlier name for Jerusalem, though this is not certain. </rdfs:comment>
    </owl:NamedIndividual>
    


    <!-- http://semanticbible.org/ns/2006/NTNames#SalemGeodata -->

    <owl:NamedIndividual rdf:about="http://semanticbible.org/ns/2006/NTNames#SalemGeodata">
        <rdfs:label xml:lang="en">geodata for Salem</rdfs:label>
        <latitude rdf:datatype="http://www.w3.org/2001/XMLSchema#double">31.77451070780678</latitude>
    </owl:NamedIndividual>
    


    <!-- http://semanticbible.org/ns/2006/NTNames#Salim -->

    <owl:NamedIndividual rdf:about="http://semanticbible.org/ns/2006/NTNames#Salim">
        <rdfs:label xml:lang="en">Salim</rdfs:label>
    </owl:NamedIndividual>
    


    <!-- http://semanticbible.org/ns/2006/NTNames#SalimGeodata -->

    <owl:NamedIndividual rdf:about="http://semanticbible.org/ns/2006/NTNames#SalimGeodata">
        <rdfs:label xml:lang="en">geodata for Salim</rdfs:label>
    </owl:NamedIndividual>
    


    <!-- http://semanticbible.org/ns/2006/NTNames#Salmon -->

    <owl:NamedIndividual rdf:about="http://semanticbible.org/ns/2006/NTNames#Salmon">
        <rdfs:label xml:lang="en">Salmon</rdfs:label>
        <rdfs:comment rdf:datatype="http://www.w3.org/2001/XMLSchema#string">Luke&#39;s genealogy has Sala, a minor variant, but the relationships make clear it is the same person.</rdfs:comment>
        <childOf rdf:resource="http://semanticbible.org/ns/2006/NTNames#Nahshon"/>
    </owl:NamedIndividual>
    


    <!-- http://semanticbible.org/ns/2006/NTNames#Salmone -->

    <owl:NamedIndividual rdf:about="http://semanticbible.org/ns/2006/NTNames#Salmone">
        <rdfs:label xml:lang="en">Salmone</rdfs:label>
    </owl:NamedIndividual>
    


    <!-- http://semanticbible.org/ns/2006/NTNames#SalmoneGeodata -->

    <owl:NamedIndividual rdf:about="http://semanticbible.org/ns/2006/NTNames#SalmoneGeodata">
        <rdfs:label xml:lang="en">geodata for Salmone</rdfs:label>
    </owl:NamedIndividual>
    


    <!-- http://semanticbible.org/ns/2006/NTNames#Salome -->

    <owl:NamedIndividual rdf:about="http://semanticbible.org/ns/2006/NTNames#Salome">
        <rdfs:label xml:lang="en">Salome</rdfs:label>
        <rdfs:comment xml:lang="en">Matthew and Mark&#39;s accounts of the crucifixion together identify Salome as the mother of the sons of Zebedee. 
This is also the traditional name of the daughter of Herodias, whose dance before King Herod led to the beheading of John the Baptist. But this woman is not named in the New Testament. </rdfs:comment>
    </owl:NamedIndividual>
    


    <!-- http://semanticbible.org/ns/2006/NTNames#Samaria -->

    <owl:NamedIndividual rdf:about="http://semanticbible.org/ns/2006/NTNames#Samaria">
        <rdfs:label xml:lang="en">Samaria</rdfs:label>
    </owl:NamedIndividual>
    


    <!-- http://semanticbible.org/ns/2006/NTNames#SamariaGeodata -->

    <owl:NamedIndividual rdf:about="http://semanticbible.org/ns/2006/NTNames#SamariaGeodata">
        <rdfs:label xml:lang="en">geodata for Samaria</rdfs:label>
        <rdfs:comment xml:lang="en">This may be overly precise positioning for a region</rdfs:comment>
    </owl:NamedIndividual>
    


    <!-- http://semanticbible.org/ns/2006/NTNames#SamariaTheCity -->

    <owl:NamedIndividual rdf:about="http://semanticbible.org/ns/2006/NTNames#SamariaTheCity">
        <rdfs:label xml:lang="en">Samaria</rdfs:label>
        <rdfs:comment xml:lang="en">Samaria was both a province in Palestine and a city of the same name.</rdfs:comment>
    </owl:NamedIndividual>
    


    <!-- http://semanticbible.org/ns/2006/NTNames#Samaritan -->

    <owl:NamedIndividual rdf:about="http://semanticbible.org/ns/2006/NTNames#Samaritan">
        <rdfs:label xml:lang="en">Samaritan</rdfs:label>
        <rdfs:comment xml:lang="en">A Jewish sect centered around the city of Samaria: in New Testament times, there was great emnity between Samaritans and Jews.</rdfs:comment>
    </owl:NamedIndividual>
    


    <!-- http://semanticbible.org/ns/2006/NTNames#Samaritans -->

    <owl:NamedIndividual rdf:about="http://semanticbible.org/ns/2006/NTNames#Samaritans">
        <rdfs:label xml:lang="en">Samaritans</rdfs:label>
    </owl:NamedIndividual>
    


    <!-- http://semanticbible.org/ns/2006/NTNames#Samos -->

    <owl:NamedIndividual rdf:about="http://semanticbible.org/ns/2006/NTNames#Samos">
        <rdfs:label xml:lang="en">Samos</rdfs:label>
    </owl:NamedIndividual>
    


    <!-- http://semanticbible.org/ns/2006/NTNames#Samothrace -->

    <owl:NamedIndividual rdf:about="http://semanticbible.org/ns/2006/NTNames#Samothrace">
        <rdfs:label xml:lang="en">Samothrace</rdfs:label>
    </owl:NamedIndividual>
    


    <!-- http://semanticbible.org/ns/2006/NTNames#Samson -->

    <owl:NamedIndividual rdf:about="http://semanticbible.org/ns/2006/NTNames#Samson">
        <rdfs:label xml:lang="en">Samson</rdfs:label>
    </owl:NamedIndividual>
    


    <!-- http://semanticbible.org/ns/2006/NTNames#Samuel -->

    <owl:NamedIndividual rdf:about="http://semanticbible.org/ns/2006/NTNames#Samuel">
        <rdfs:label xml:lang="en">Samuel</rdfs:label>
    </owl:NamedIndividual>
    


    <!-- http://semanticbible.org/ns/2006/NTNames#Sanhedrin -->

    <owl:NamedIndividual rdf:about="http://semanticbible.org/ns/2006/NTNames#Sanhedrin">
        <rdfs:label xml:lang="en">Sanhedrin</rdfs:label>
        <rdfs:comment xml:lang="en">The Jewish supreme council</rdfs:comment>
    </owl:NamedIndividual>
    


    <!-- http://semanticbible.org/ns/2006/NTNames#Sapphira -->

    <owl:NamedIndividual rdf:about="http://semanticbible.org/ns/2006/NTNames#Sapphira">
        <rdfs:label xml:lang="en">Sapphira</rdfs:label>
    </owl:NamedIndividual>
    


    <!-- http://semanticbible.org/ns/2006/NTNames#Sarah -->

    <owl:NamedIndividual rdf:about="http://semanticbible.org/ns/2006/NTNames#Sarah">
        <rdfs:label xml:lang="en">Sarah</rdfs:label>
        <rdfs:comment xml:lang="en">An important Old Testament figure. Curiously enough, both Abraham and Sarah are described as having Terah as father, presumably by different mothers. </rdfs:comment>
        <childOf rdf:resource="http://semanticbible.org/ns/2006/NTNames#Terah"/>
    </owl:NamedIndividual>
    


    <!-- http://semanticbible.org/ns/2006/NTNames#Sardis -->

    <owl:NamedIndividual rdf:about="http://semanticbible.org/ns/2006/NTNames#Sardis">
        <rdfs:label xml:lang="en">Sardis</rdfs:label>
    </owl:NamedIndividual>
    


    <!-- http://semanticbible.org/ns/2006/NTNames#SardisGeodata -->

    <owl:NamedIndividual rdf:about="http://semanticbible.org/ns/2006/NTNames#SardisGeodata">
        <rdfs:label xml:lang="en">geodata for Sardis</rdfs:label>
    </owl:NamedIndividual>
    


    <!-- http://semanticbible.org/ns/2006/NTNames#Satan -->

    <owl:NamedIndividual rdf:about="http://semanticbible.org/ns/2006/NTNames#Satan">
        <rdfs:label xml:lang="en">Satan</rdfs:label>
    </owl:NamedIndividual>
    


    <!-- http://semanticbible.org/ns/2006/NTNames#SaulSonOfKish -->

    <owl:NamedIndividual rdf:about="http://semanticbible.org/ns/2006/NTNames#SaulSonOfKish">
        <rdfs:label xml:lang="en">Saul</rdfs:label>
    </owl:NamedIndividual>
    


    <!-- http://semanticbible.org/ns/2006/NTNames#Sceva -->

    <owl:NamedIndividual rdf:about="http://semanticbible.org/ns/2006/NTNames#Sceva">
        <rdfs:label xml:lang="en">Sceva</rdfs:label>
    </owl:NamedIndividual>
    


    <!-- http://semanticbible.org/ns/2006/NTNames#Scripture -->

    <owl:NamedIndividual rdf:about="http://semanticbible.org/ns/2006/NTNames#Scripture">
        <rdf:type rdf:resource="http://semanticbible.org/ns/2006/NTNames#Series"/>
        <rdfs:label xml:lang="en">Scripture</rdfs:label>
    </owl:NamedIndividual>
    


    <!-- http://semanticbible.org/ns/2006/NTNames#Scriptures -->

    <owl:NamedIndividual rdf:about="http://semanticbible.org/ns/2006/NTNames#Scriptures">
        <rdfs:label xml:lang="en">Scriptures</rdfs:label>
    </owl:NamedIndividual>
    


    <!-- http://semanticbible.org/ns/2006/NTNames#Scythian -->

    <owl:NamedIndividual rdf:about="http://semanticbible.org/ns/2006/NTNames#Scythian">
        <rdfs:label xml:lang="en">Scythian</rdfs:label>
        <rdfs:comment xml:lang="en">Herodotus describes the Scythians as a savage race of nomads, living generally north of the Black and Caspain Seas. Paul&#39;s single use of the term seems largely synonymous with them as a type of barbarians. </rdfs:comment>
    </owl:NamedIndividual>
    


    <!-- http://semanticbible.org/ns/2006/NTNames#SeaOfGalilee -->

    <owl:NamedIndividual rdf:about="http://semanticbible.org/ns/2006/NTNames#SeaOfGalilee">
        <rdfs:label xml:lang="en">Sea of Galilee</rdfs:label>
    </owl:NamedIndividual>
    


    <!-- http://semanticbible.org/ns/2006/NTNames#SeaofGalileeGeodata -->

    <owl:NamedIndividual rdf:about="http://semanticbible.org/ns/2006/NTNames#SeaofGalileeGeodata">
        <rdfs:label xml:lang="en">geodata for Sea of Galilee</rdfs:label>
        <latitude rdf:datatype="http://www.w3.org/2001/XMLSchema#double">32.77589768765405</latitude>
    </owl:NamedIndividual>
    


    <!-- http://semanticbible.org/ns/2006/NTNames#Secundus -->

    <owl:NamedIndividual rdf:about="http://semanticbible.org/ns/2006/NTNames#Secundus">
        <rdfs:label xml:lang="en">Secundus</rdfs:label>
        <rdfs:comment rdf:datatype="http://www.w3.org/2001/XMLSchema#string">Luke describes him as &quot;of the Thessalonians&quot;, which could mean either his residence or his origin. </rdfs:comment>
        <collaboratesWith rdf:resource="http://semanticbible.org/ns/2006/NTNames#Timothy"/>
    </owl:NamedIndividual>
    


    <!-- http://semanticbible.org/ns/2006/NTNames#Seleucia -->

    <owl:NamedIndividual rdf:about="http://semanticbible.org/ns/2006/NTNames#Seleucia">
        <rdfs:label xml:lang="en">Seleucia</rdfs:label>
        <location rdf:resource="http://semanticbible.org/ns/2006/NTNames#SeleuciaGeodata"/>
    </owl:NamedIndividual>
    


    <!-- http://semanticbible.org/ns/2006/NTNames#SeleuciaGeodata -->

    <owl:NamedIndividual rdf:about="http://semanticbible.org/ns/2006/NTNames#SeleuciaGeodata">
        <rdfs:label xml:lang="en">geodata for Seleucia</rdfs:label>
    </owl:NamedIndividual>
    


    <!-- http://semanticbible.org/ns/2006/NTNames#Semein -->

    <owl:NamedIndividual rdf:about="http://semanticbible.org/ns/2006/NTNames#Semein">
        <rdfs:label xml:lang="en">Semein</rdfs:label>
        <ethnicity rdf:resource="http://semanticbible.org/ns/2006/NTNames#Jewish"/>
    </owl:NamedIndividual>
    


    <!-- http://semanticbible.org/ns/2006/NTNames#SergiusPaulus -->

    <owl:NamedIndividual rdf:about="http://semanticbible.org/ns/2006/NTNames#SergiusPaulus">
        <rdfs:label xml:lang="en">Sergius Paulus</rdfs:label>
        <description rdf:datatype="http://www.w3.org/2001/XMLSchema#string">procounsul of Cyprus and &#39;a man of intelligence&#39;</description>
    </owl:NamedIndividual>
    


    <!-- http://semanticbible.org/ns/2006/NTNames#Serug -->

    <owl:NamedIndividual rdf:about="http://semanticbible.org/ns/2006/NTNames#Serug">
        <rdfs:label xml:lang="en">Serug</rdfs:label>
        <parentOf rdf:resource="http://semanticbible.org/ns/2006/NTNames#Nahor"/>
    </owl:NamedIndividual>
    


    <!-- http://semanticbible.org/ns/2006/NTNames#Seth -->

    <owl:NamedIndividual rdf:about="http://semanticbible.org/ns/2006/NTNames#Seth">
        <rdfs:label xml:lang="en">Seth</rdfs:label>
        <parentOf rdf:resource="http://semanticbible.org/ns/2006/NTNames#Enos"/>
    </owl:NamedIndividual>
    


    <!-- http://semanticbible.org/ns/2006/NTNames#Sharon -->

    <owl:NamedIndividual rdf:about="http://semanticbible.org/ns/2006/NTNames#Sharon">
        <rdfs:label xml:lang="en">Sharon</rdfs:label>
    </owl:NamedIndividual>
    


    <!-- http://semanticbible.org/ns/2006/NTNames#Shealtiel -->

    <owl:NamedIndividual rdf:about="http://semanticbible.org/ns/2006/NTNames#Shealtiel">
        <rdf:type rdf:resource="http://semanticbible.org/ns/2006/NTNames#Man"/>
        <rdfs:label xml:lang="en">Shealtiel</rdfs:label>
    </owl:NamedIndividual>
    


    <!-- http://semanticbible.org/ns/2006/NTNames#ShealtielSonOfNeri -->

    <owl:NamedIndividual rdf:about="http://semanticbible.org/ns/2006/NTNames#ShealtielSonOfNeri">
        <rdf:type rdf:resource="http://semanticbible.org/ns/2006/NTNames#Man"/>
        <rdfs:label xml:lang="en">Shealtiel</rdfs:label>
    </owl:NamedIndividual>
    


    <!-- http://semanticbible.org/ns/2006/NTNames#Shechem -->

    <owl:NamedIndividual rdf:about="http://semanticbible.org/ns/2006/NTNames#Shechem">
        <rdfs:label xml:lang="en">Shechem</rdfs:label>
        <rdfs:comment rdf:datatype="http://www.w3.org/2001/XMLSchema#string">A subregion of Canaan.</rdfs:comment>
    </owl:NamedIndividual>
    


    <!-- http://semanticbible.org/ns/2006/NTNames#ShechemGeodata -->

    <owl:NamedIndividual rdf:about="http://semanticbible.org/ns/2006/NTNames#ShechemGeodata">
        <rdfs:label xml:lang="en">geodata for Shechem</rdfs:label>
    </owl:NamedIndividual>
    


    <!-- http://semanticbible.org/ns/2006/NTNames#Shelah -->

    <owl:NamedIndividual rdf:about="http://semanticbible.org/ns/2006/NTNames#Shelah">
        <rdfs:label xml:lang="en">Shelah</rdfs:label>
    </owl:NamedIndividual>
    


    <!-- http://semanticbible.org/ns/2006/NTNames#Shem -->

    <owl:NamedIndividual rdf:about="http://semanticbible.org/ns/2006/NTNames#Shem">
        <rdfs:label xml:lang="en">Shem</rdfs:label>
        <hasOnlyGenealogyMention rdf:datatype="http://www.w3.org/2001/XMLSchema#boolean">true</hasOnlyGenealogyMention>
    </owl:NamedIndividual>
    


    <!-- http://semanticbible.org/ns/2006/NTNames#Sidon -->

    <owl:NamedIndividual rdf:about="http://semanticbible.org/ns/2006/NTNames#Sidon">
        <rdfs:label xml:lang="en">Sidon</rdfs:label>
    </owl:NamedIndividual>
    


    <!-- http://semanticbible.org/ns/2006/NTNames#SidonGeodata -->

    <owl:NamedIndividual rdf:about="http://semanticbible.org/ns/2006/NTNames#SidonGeodata">
        <rdfs:label xml:lang="en">geodata for Sidon</rdfs:label>
    </owl:NamedIndividual>
    


    <!-- http://semanticbible.org/ns/2006/NTNames#Silas -->

    <owl:NamedIndividual rdf:about="http://semanticbible.org/ns/2006/NTNames#Silas">
        <rdf:type rdf:resource="http://semanticbible.org/ns/2006/NTNames#Man"/>
        <rdfs:label xml:lang="en">Silas</rdfs:label>
    </owl:NamedIndividual>
    


    <!-- http://semanticbible.org/ns/2006/NTNames#Siloam -->

    <owl:NamedIndividual rdf:about="http://semanticbible.org/ns/2006/NTNames#Siloam">
        <rdfs:label xml:lang="en">Siloam</rdfs:label>
        <rdfs:comment xml:lang="en">A pool outside the walls of Jerusalem.</rdfs:comment>
        <subregionOf rdf:resource="http://semanticbible.org/ns/2006/NTNames#Jerusalem"/>
    </owl:NamedIndividual>
    


    <!-- http://semanticbible.org/ns/2006/NTNames#Silvanus -->

    <owl:NamedIndividual rdf:about="http://semanticbible.org/ns/2006/NTNames#Silvanus">
        <rdfs:label xml:lang="en">Silvanus</rdfs:label>
    </owl:NamedIndividual>
    


    <!-- http://semanticbible.org/ns/2006/NTNames#SimeonNiger -->

    <owl:NamedIndividual rdf:about="http://semanticbible.org/ns/2006/NTNames#SimeonNiger">
        <rdfs:label xml:lang="en">Simeon</rdfs:label>
    </owl:NamedIndividual>
    


    <!-- http://semanticbible.org/ns/2006/NTNames#SimeonSonOfJudah -->

    <owl:NamedIndividual rdf:about="http://semanticbible.org/ns/2006/NTNames#SimeonSonOfJudah">
        <rdfs:label xml:lang="en">Simeon</rdfs:label>
    </owl:NamedIndividual>
    


    <!-- http://semanticbible.org/ns/2006/NTNames#SimeonThePatriarch -->

    <owl:NamedIndividual rdf:about="http://semanticbible.org/ns/2006/NTNames#SimeonThePatriarch">
        <rdfs:label xml:lang="en">Simeon</rdfs:label>
        <siblingOf rdf:resource="http://semanticbible.org/ns/2006/NTNames#Gad"/>
    </owl:NamedIndividual>
    


    <!-- http://semanticbible.org/ns/2006/NTNames#SimeonTheProphet -->

    <owl:NamedIndividual rdf:about="http://semanticbible.org/ns/2006/NTNames#SimeonTheProphet">
        <rdf:type rdf:resource="http://semanticbible.org/ns/2006/NTNames#Man"/>
        <rdfs:label xml:lang="en">Simeon</rdfs:label>
    </owl:NamedIndividual>
    


    <!-- http://semanticbible.org/ns/2006/NTNames#SimonOfCyrene -->

    <owl:NamedIndividual rdf:about="http://semanticbible.org/ns/2006/NTNames#SimonOfCyrene">
        <rdfs:label xml:lang="en">Simon</rdfs:label>
        <rdfs:comment xml:lang="en">Identified as a Jew because, though a foreigner, he was in Jerusalem at the time of Passover</rdfs:comment>
    </owl:NamedIndividual>
    


    <!-- http://semanticbible.org/ns/2006/NTNames#SimonPeter -->

    <owl:NamedIndividual rdf:about="http://semanticbible.org/ns/2006/NTNames#SimonPeter">
        <rdfs:label xml:lang="en">Simon Peter</rdfs:label>
        <rdfs:comment rdf:datatype="http://www.w3.org/2001/XMLSchema#string">The main definition for the Apostle Peter.</rdfs:comment>
        <antagonistOf rdf:resource="http://semanticbible.org/ns/2006/NTNames#Sapphira"/>
    </owl:NamedIndividual>
    


    <!-- http://semanticbible.org/ns/2006/NTNames#SimonTheTanner -->

    <owl:NamedIndividual rdf:about="http://semanticbible.org/ns/2006/NTNames#SimonTheTanner">
        <rdfs:label xml:lang="en">Simon</rdfs:label>
    </owl:NamedIndividual>
    


    <!-- http://semanticbible.org/ns/2006/NTNames#SimonTheZealot -->

    <owl:NamedIndividual rdf:about="http://semanticbible.org/ns/2006/NTNames#SimonTheZealot">
        <rdfs:label xml:lang="en">Simon</rdfs:label>
        <rdfs:comment xml:lang="en">Simon the Zealot was also known as Simon the Cananaean (but the term is one of political, not geographic, affiliation).</rdfs:comment>
    </owl:NamedIndividual>
    


    <!-- http://semanticbible.org/ns/2006/NTNames#Sinai -->

    <owl:NamedIndividual rdf:about="http://semanticbible.org/ns/2006/NTNames#Sinai">
        <rdfs:label xml:lang="en">Sinai</rdfs:label>
    </owl:NamedIndividual>
    


    <!-- http://semanticbible.org/ns/2006/NTNames#Smyrna -->

    <owl:NamedIndividual rdf:about="http://semanticbible.org/ns/2006/NTNames#Smyrna">
        <rdfs:label xml:lang="en">Smyrna</rdfs:label>
    </owl:NamedIndividual>
    


    <!-- http://semanticbible.org/ns/2006/NTNames#SmyrnaGeodata -->

    <owl:NamedIndividual rdf:about="http://semanticbible.org/ns/2006/NTNames#SmyrnaGeodata">
        <rdfs:label xml:lang="en">geodata for Smyrna</rdfs:label>
        <latitude rdf:datatype="http://www.w3.org/2001/XMLSchema#double">38.32512200511864</latitude>
    </owl:NamedIndividual>
    


    <!-- http://semanticbible.org/ns/2006/NTNames#Sodom -->

    <owl:NamedIndividual rdf:about="http://semanticbible.org/ns/2006/NTNames#Sodom">
        <rdfs:label xml:lang="en">Sodom</rdfs:label>
    </owl:NamedIndividual>
    


    <!-- http://semanticbible.org/ns/2006/NTNames#SodomGeodata -->

    <owl:NamedIndividual rdf:about="http://semanticbible.org/ns/2006/NTNames#SodomGeodata">
        <rdfs:label xml:lang="en">geodata for Sodom</rdfs:label>
    </owl:NamedIndividual>
    


    <!-- http://semanticbible.org/ns/2006/NTNames#Solomon -->

    <owl:NamedIndividual rdf:about="http://semanticbible.org/ns/2006/NTNames#Solomon">
        <rdfs:label xml:lang="en">Solomon</rdfs:label>
        <ethnicity rdf:resource="http://semanticbible.org/ns/2006/NTNames#Jewish"/>
    </owl:NamedIndividual>
    


    <!-- http://semanticbible.org/ns/2006/NTNames#Sopater -->

    <owl:NamedIndividual rdf:about="http://semanticbible.org/ns/2006/NTNames#Sopater">
        <rdfs:label xml:lang="en">Sopater</rdfs:label>
        <childOf rdf:resource="http://semanticbible.org/ns/2006/NTNames#Pyrrhus"/>
    </owl:NamedIndividual>
    


    <!-- http://semanticbible.org/ns/2006/NTNames#Sosipater -->

    <owl:NamedIndividual rdf:about="http://semanticbible.org/ns/2006/NTNames#Sosipater">
        <rdfs:label xml:lang="en">Sosipater</rdfs:label>
        <rdfs:comment xml:lang="en">&quot;kinsman&quot; here probably means that that he is a Jew, rather than an actual relation, given the number of people so designated in Romans 16. His residence in Corinth follows from the inference that Paul resided there when he wrote the letter to the Roman church.  </rdfs:comment>
        <residentPlace rdf:resource="http://semanticbible.org/ns/2006/NTNames#Corinth"/>
    </owl:NamedIndividual>
    


    <!-- http://semanticbible.org/ns/2006/NTNames#Sosthenes -->

    <owl:NamedIndividual rdf:about="http://semanticbible.org/ns/2006/NTNames#Sosthenes">
        <rdfs:label xml:lang="en">Sosthenes</rdfs:label>
    </owl:NamedIndividual>
    


    <!-- http://semanticbible.org/ns/2006/NTNames#Spain -->

    <owl:NamedIndividual rdf:about="http://semanticbible.org/ns/2006/NTNames#Spain">
        <rdfs:label xml:lang="en">Spain</rdfs:label>
    </owl:NamedIndividual>
    


    <!-- http://semanticbible.org/ns/2006/NTNames#Stachys -->

    <owl:NamedIndividual rdf:about="http://semanticbible.org/ns/2006/NTNames#Stachys">
        <rdf:type rdf:resource="http://semanticbible.org/ns/2006/NTNames#Man"/>
        <rdfs:label xml:lang="en">Stachys</rdfs:label>
    </owl:NamedIndividual>
    


    <!-- http://semanticbible.org/ns/2006/NTNames#Stephanas -->

    <owl:NamedIndividual rdf:about="http://semanticbible.org/ns/2006/NTNames#Stephanas">
        <rdfs:label xml:lang="en">Stephanas</rdfs:label>
        <rdfs:comment xml:lang="en">His residence in Corinth and visit to Ephesus follow from Paul&#39;s statement in 1Cor.16.17, and the assumption that Paul was in Ephesus when he wrote 1 Corinthians. </rdfs:comment>
        <residentPlace rdf:resource="http://semanticbible.org/ns/2006/NTNames#Corinth"/>
    </owl:NamedIndividual>
    


    <!-- http://semanticbible.org/ns/2006/NTNames#Stephen -->

    <owl:NamedIndividual rdf:about="http://semanticbible.org/ns/2006/NTNames#Stephen">
        <rdfs:label xml:lang="en">Stephen</rdfs:label>
    </owl:NamedIndividual>
    


    <!-- http://semanticbible.org/ns/2006/NTNames#Stoic -->

    <owl:NamedIndividual rdf:about="http://semanticbible.org/ns/2006/NTNames#Stoic">
        <rdfs:label xml:lang="en">Stoic</rdfs:label>
    </owl:NamedIndividual>
    


    <!-- http://semanticbible.org/ns/2006/NTNames#Susanna -->

    <owl:NamedIndividual rdf:about="http://semanticbible.org/ns/2006/NTNames#Susanna">
        <rdfs:label xml:lang="en">Susanna</rdfs:label>
        <collaboratesWith rdf:resource="http://semanticbible.org/ns/2006/NTNames#Jesus"/>
    </owl:NamedIndividual>
    


    <!-- http://semanticbible.org/ns/2006/NTNames#Sychar -->

    <owl:NamedIndividual rdf:about="http://semanticbible.org/ns/2006/NTNames#Sychar">
        <rdfs:label xml:lang="en">Sychar</rdfs:label>
        <rdfs:comment xml:lang="en">Jesus spoke here with a Samaritan woman about living water</rdfs:comment>
    </owl:NamedIndividual>
    


    <!-- http://semanticbible.org/ns/2006/NTNames#SycharGeodata -->

    <owl:NamedIndividual rdf:about="http://semanticbible.org/ns/2006/NTNames#SycharGeodata">
        <rdfs:label xml:lang="en">geodata for Sychar</rdfs:label>
    </owl:NamedIndividual>
    


    <!-- http://semanticbible.org/ns/2006/NTNames#Syntyche -->

    <owl:NamedIndividual rdf:about="http://semanticbible.org/ns/2006/NTNames#Syntyche">
        <rdfs:label xml:lang="en">Syntyche</rdfs:label>
    </owl:NamedIndividual>
    


    <!-- http://semanticbible.org/ns/2006/NTNames#Syracuse -->

    <owl:NamedIndividual rdf:about="http://semanticbible.org/ns/2006/NTNames#Syracuse">
        <rdfs:label xml:lang="en">Syracuse</rdfs:label>
    </owl:NamedIndividual>
    


    <!-- http://semanticbible.org/ns/2006/NTNames#SyracuseGeodata -->

    <owl:NamedIndividual rdf:about="http://semanticbible.org/ns/2006/NTNames#SyracuseGeodata">
        <rdfs:label xml:lang="en">geodata for Syracuse</rdfs:label>
    </owl:NamedIndividual>
    


    <!-- http://semanticbible.org/ns/2006/NTNames#Syria -->

    <owl:NamedIndividual rdf:about="http://semanticbible.org/ns/2006/NTNames#Syria">
        <rdfs:label xml:lang="en">Syria</rdfs:label>
    </owl:NamedIndividual>
    


    <!-- http://semanticbible.org/ns/2006/NTNames#Syrian -->

    <owl:NamedIndividual rdf:about="http://semanticbible.org/ns/2006/NTNames#Syrian">
        <rdfs:label xml:lang="en">Syrian</rdfs:label>
        <rdfs:comment xml:lang="en">Of the country of Syria.</rdfs:comment>
    </owl:NamedIndividual>
    


    <!-- http://semanticbible.org/ns/2006/NTNames#Syrophoenician -->

    <owl:NamedIndividual rdf:about="http://semanticbible.org/ns/2006/NTNames#Syrophoenician">
        <rdfs:label xml:lang="en">Syrophoenician</rdfs:label>
        <rdfs:comment xml:lang="en">Likely synonymous with Canaanite, and referring to those from the region of Syria and Phoenicia, and therefore a subgroup of Greek Gentiles.</rdfs:comment>
    </owl:NamedIndividual>
    


    <!-- http://semanticbible.org/ns/2006/NTNames#Syrtis -->

    <owl:NamedIndividual rdf:about="http://semanticbible.org/ns/2006/NTNames#Syrtis">
        <rdfs:label xml:lang="en">Syrtis</rdfs:label>
    </owl:NamedIndividual>
    


    <!-- http://semanticbible.org/ns/2006/NTNames#Tabitha -->

    <owl:NamedIndividual rdf:about="http://semanticbible.org/ns/2006/NTNames#Tabitha">
        <rdfs:label xml:lang="en">Dorcas</rdfs:label>
        <rdfs:label xml:lang="en">Tabitha</rdfs:label>
        <rdfs:comment xml:lang="en">The Aramaic name Tabitha corresponds to the Greek form Dorcas. She probably also knew Simon the Tanner. </rdfs:comment>
    </owl:NamedIndividual>
    


    <!-- http://semanticbible.org/ns/2006/NTNames#Tamar -->

    <owl:NamedIndividual rdf:about="http://semanticbible.org/ns/2006/NTNames#Tamar">
        <rdfs:label xml:lang="en">Tamar</rdfs:label>
    </owl:NamedIndividual>
    


    <!-- http://semanticbible.org/ns/2006/NTNames#Tarsus -->

    <owl:NamedIndividual rdf:about="http://semanticbible.org/ns/2006/NTNames#Tarsus">
        <rdfs:label xml:lang="en">Tarsus</rdfs:label>
    </owl:NamedIndividual>
    


    <!-- http://semanticbible.org/ns/2006/NTNames#TarsusGeodata -->

    <owl:NamedIndividual rdf:about="http://semanticbible.org/ns/2006/NTNames#TarsusGeodata">
        <rdfs:label xml:lang="en">geodata for Tarsus</rdfs:label>
    </owl:NamedIndividual>
    


    <!-- http://semanticbible.org/ns/2006/NTNames#Taverns -->

    <owl:NamedIndividual rdf:about="http://semanticbible.org/ns/2006/NTNames#Taverns">
        <rdfs:label xml:lang="en">Taverns</rdfs:label>
    </owl:NamedIndividual>
    


    <!-- http://semanticbible.org/ns/2006/NTNames#Terah -->

    <owl:NamedIndividual rdf:about="http://semanticbible.org/ns/2006/NTNames#Terah">
        <rdfs:label xml:lang="en">Terah</rdfs:label>
    </owl:NamedIndividual>
    


    <!-- http://semanticbible.org/ns/2006/NTNames#Tertius -->

    <owl:NamedIndividual rdf:about="http://semanticbible.org/ns/2006/NTNames#Tertius">
        <rdfs:label xml:lang="en">Tertius</rdfs:label>
        <rdfs:comment rdf:datatype="http://www.w3.org/2001/XMLSchema#string">His residence in Corinth follows from the inference that Paul resided there when he wrote the letter to the Roman church.  </rdfs:comment>
        <description rdf:datatype="http://www.w3.org/2001/XMLSchema#string">the scribe of Paul&#39;s letter to the Roman church</description>
    </owl:NamedIndividual>
    


    <!-- http://semanticbible.org/ns/2006/NTNames#Tertullus -->

    <owl:NamedIndividual rdf:about="http://semanticbible.org/ns/2006/NTNames#Tertullus">
        <rdfs:label xml:lang="en">Tertullus</rdfs:label>
        <rdfs:comment xml:lang="en">Speaking on behalf of the Sanhedrin does not imply Tertullus was Jewish: more likely (but not certain), he was a Roman, hired for his familiarity with Roman law. But the account describes him as traveling from Jerusalem with the others.</rdfs:comment>
    </owl:NamedIndividual>
    


    <!-- http://semanticbible.org/ns/2006/NTNames#Thaddaeus -->

    <owl:NamedIndividual rdf:about="http://semanticbible.org/ns/2006/NTNames#Thaddaeus">
        <rdf:type rdf:resource="http://semanticbible.org/ns/2006/NTNames#Man"/>
        <rdfs:label xml:lang="en">Thaddaeus</rdfs:label>
    </owl:NamedIndividual>
    


    <!-- http://semanticbible.org/ns/2006/NTNames#Theophilus -->

    <owl:NamedIndividual rdf:about="http://semanticbible.org/ns/2006/NTNames#Theophilus">
        <rdfs:label xml:lang="en">Theophilus</rdfs:label>
    </owl:NamedIndividual>
    


    <!-- http://semanticbible.org/ns/2006/NTNames#Thessalonians -->

    <owl:NamedIndividual rdf:about="http://semanticbible.org/ns/2006/NTNames#Thessalonians">
        <rdf:type rdf:resource="http://semanticbible.org/ns/2006/NTNames#ResidenceGroup"/>
        <rdfs:label xml:lang="en">Thessalonians</rdfs:label>
    </owl:NamedIndividual>
    


    <!-- http://semanticbible.org/ns/2006/NTNames#Thessalonica -->

    <owl:NamedIndividual rdf:about="http://semanticbible.org/ns/2006/NTNames#Thessalonica">
        <rdfs:label xml:lang="en">Thessalonica</rdfs:label>
    </owl:NamedIndividual>
    


    <!-- http://semanticbible.org/ns/2006/NTNames#ThessalonicaGeodata -->

    <owl:NamedIndividual rdf:about="http://semanticbible.org/ns/2006/NTNames#ThessalonicaGeodata">
        <rdfs:label xml:lang="en">geodata for Thessalonica</rdfs:label>
    </owl:NamedIndividual>
    


    <!-- http://semanticbible.org/ns/2006/NTNames#Theudas -->

    <owl:NamedIndividual rdf:about="http://semanticbible.org/ns/2006/NTNames#Theudas">
        <rdfs:label xml:lang="en">Theudas</rdfs:label>
    </owl:NamedIndividual>
    


    <!-- http://semanticbible.org/ns/2006/NTNames#Thomas -->

    <owl:NamedIndividual rdf:about="http://semanticbible.org/ns/2006/NTNames#Thomas">
        <rdfs:label xml:lang="en">Thomas</rdfs:label>
    </owl:NamedIndividual>
    


    <!-- http://semanticbible.org/ns/2006/NTNames#Thyatira -->

    <owl:NamedIndividual rdf:about="http://semanticbible.org/ns/2006/NTNames#Thyatira">
        <rdfs:label xml:lang="en">Thyatira</rdfs:label>
    </owl:NamedIndividual>
    


    <!-- http://semanticbible.org/ns/2006/NTNames#ThyatiraGeodata -->

    <owl:NamedIndividual rdf:about="http://semanticbible.org/ns/2006/NTNames#ThyatiraGeodata">
        <rdfs:label xml:lang="en">geodata for Thyatira</rdfs:label>
        <altitude rdf:datatype="http://www.w3.org/2001/XMLSchema#int">0</altitude>
    </owl:NamedIndividual>
    


    <!-- http://semanticbible.org/ns/2006/NTNames#Tiberias -->

    <owl:NamedIndividual rdf:about="http://semanticbible.org/ns/2006/NTNames#Tiberias">
        <rdfs:label xml:lang="en">Tiberias</rdfs:label>
        <rdfs:comment xml:lang="en">Tiberias was built by Herod Antipas, the tetrarch of Galilee, as his capital. </rdfs:comment>
    </owl:NamedIndividual>
    


    <!-- http://semanticbible.org/ns/2006/NTNames#TiberiasGeodata -->

    <owl:NamedIndividual rdf:about="http://semanticbible.org/ns/2006/NTNames#TiberiasGeodata">
        <rdfs:label xml:lang="en">geodata for Tiberias</rdfs:label>
    </owl:NamedIndividual>
    


    <!-- http://semanticbible.org/ns/2006/NTNames#TiberiusCaesar -->

    <owl:NamedIndividual rdf:about="http://semanticbible.org/ns/2006/NTNames#TiberiusCaesar">
        <rdfs:label xml:lang="en">Tiberius Caesar</rdfs:label>
        <rdfs:comment xml:lang="en">Caesar is used as a name for several different individuals in the New Testament. This is the Caesar referred to by Jesus. </rdfs:comment>
    </owl:NamedIndividual>
    


    <!-- http://semanticbible.org/ns/2006/NTNames#Timaeus -->

    <owl:NamedIndividual rdf:about="http://semanticbible.org/ns/2006/NTNames#Timaeus">
        <rdfs:label xml:lang="en">Timaeus</rdfs:label>
    </owl:NamedIndividual>
    


    <!-- http://semanticbible.org/ns/2006/NTNames#Timon -->

    <owl:NamedIndividual rdf:about="http://semanticbible.org/ns/2006/NTNames#Timon">
        <rdfs:label xml:lang="en">Timon</rdfs:label>
    </owl:NamedIndividual>
    


    <!-- http://semanticbible.org/ns/2006/NTNames#Timothy -->

    <owl:NamedIndividual rdf:about="http://semanticbible.org/ns/2006/NTNames#Timothy">
        <rdfs:label xml:lang="en">Timothy</rdfs:label>
        <rdfs:comment xml:lang="en">Timothy&#39;s residence in Corinth follows from the close of Paul&#39;s letter to the Romans, assumed to have been written from Corinth. </rdfs:comment>
        <collaboratesWith rdf:resource="http://semanticbible.org/ns/2006/NTNames#GaiusOfDerbe"/>
        <knows rdf:resource="http://semanticbible.org/ns/2006/NTNames#Jason"/>
    </owl:NamedIndividual>
    


    <!-- http://semanticbible.org/ns/2006/NTNames#Titius -->

    <owl:NamedIndividual rdf:about="http://semanticbible.org/ns/2006/NTNames#Titius">
        <rdfs:label xml:lang="en">Titius</rdfs:label>
    </owl:NamedIndividual>
    


    <!-- http://semanticbible.org/ns/2006/NTNames#Titus -->

    <owl:NamedIndividual rdf:about="http://semanticbible.org/ns/2006/NTNames#Titus">
        <rdfs:label xml:lang="en">Titus</rdfs:label>
    </owl:NamedIndividual>
    


    <!-- http://semanticbible.org/ns/2006/NTNames#Trachonitis -->

    <owl:NamedIndividual rdf:about="http://semanticbible.org/ns/2006/NTNames#Trachonitis">
        <rdfs:label xml:lang="en">Trachonitis</rdfs:label>
    </owl:NamedIndividual>
    


    <!-- http://semanticbible.org/ns/2006/NTNames#TribeOfAsher -->

    <owl:NamedIndividual rdf:about="http://semanticbible.org/ns/2006/NTNames#TribeOfAsher">
        <rdf:type rdf:resource="http://semanticbible.org/ns/2006/NTNames#Tribe"/>
        <rdfs:label xml:lang="en">tribe of Asher</rdfs:label>
    </owl:NamedIndividual>
    


    <!-- http://semanticbible.org/ns/2006/NTNames#TribeOfBenjamin -->

    <owl:NamedIndividual rdf:about="http://semanticbible.org/ns/2006/NTNames#TribeOfBenjamin">
        <rdfs:label xml:lang="en">tribe of Benjamin</rdfs:label>
    </owl:NamedIndividual>
    


    <!-- http://semanticbible.org/ns/2006/NTNames#TribeOfGad -->

    <owl:NamedIndividual rdf:about="http://semanticbible.org/ns/2006/NTNames#TribeOfGad">
        <rdfs:label xml:lang="en">tribe of Gad</rdfs:label>
    </owl:NamedIndividual>
    


    <!-- http://semanticbible.org/ns/2006/NTNames#TribeOfIssachar -->

    <owl:NamedIndividual rdf:about="http://semanticbible.org/ns/2006/NTNames#TribeOfIssachar">
        <rdf:type rdf:resource="http://semanticbible.org/ns/2006/NTNames#Tribe"/>
        <rdfs:label xml:lang="en">tribe of Issachar</rdfs:label>
    </owl:NamedIndividual>
    


    <!-- http://semanticbible.org/ns/2006/NTNames#TribeOfJoseph -->

    <owl:NamedIndividual rdf:about="http://semanticbible.org/ns/2006/NTNames#TribeOfJoseph">
        <rdfs:label xml:lang="en">tribe of Joseph</rdfs:label>
    </owl:NamedIndividual>
    


    <!-- http://semanticbible.org/ns/2006/NTNames#TribeOfJudah -->

    <owl:NamedIndividual rdf:about="http://semanticbible.org/ns/2006/NTNames#TribeOfJudah">
        <rdfs:label xml:lang="en">tribe of Judah</rdfs:label>
    </owl:NamedIndividual>
    


    <!-- http://semanticbible.org/ns/2006/NTNames#TribeOfLevi -->

    <owl:NamedIndividual rdf:about="http://semanticbible.org/ns/2006/NTNames#TribeOfLevi">
        <rdfs:label xml:lang="en">tribe of Levi</rdfs:label>
    </owl:NamedIndividual>
    


    <!-- http://semanticbible.org/ns/2006/NTNames#TribeOfManasseh -->

    <owl:NamedIndividual rdf:about="http://semanticbible.org/ns/2006/NTNames#TribeOfManasseh">
        <rdfs:label xml:lang="en">tribe of Manasseh</rdfs:label>
    </owl:NamedIndividual>
    


    <!-- http://semanticbible.org/ns/2006/NTNames#TribeOfNaphtali -->

    <owl:NamedIndividual rdf:about="http://semanticbible.org/ns/2006/NTNames#TribeOfNaphtali">
        <rdfs:label xml:lang="en">Naphtali</rdfs:label>
        <rdfs:label xml:lang="en">tribe of Naphtali</rdfs:label>
    </owl:NamedIndividual>
    


    <!-- http://semanticbible.org/ns/2006/NTNames#TribeOfReuben -->

    <owl:NamedIndividual rdf:about="http://semanticbible.org/ns/2006/NTNames#TribeOfReuben">
        <rdfs:label xml:lang="en">tribe of Reuben</rdfs:label>
    </owl:NamedIndividual>
    


    <!-- http://semanticbible.org/ns/2006/NTNames#TribeOfSimeon -->

    <owl:NamedIndividual rdf:about="http://semanticbible.org/ns/2006/NTNames#TribeOfSimeon">
        <rdfs:label xml:lang="en">tribe of Simeon</rdfs:label>
    </owl:NamedIndividual>
    


    <!-- http://semanticbible.org/ns/2006/NTNames#TribeOfZebulun -->

    <owl:NamedIndividual rdf:about="http://semanticbible.org/ns/2006/NTNames#TribeOfZebulun">
        <rdf:type rdf:resource="http://semanticbible.org/ns/2006/NTNames#Tribe"/>
        <rdfs:label xml:lang="en">Zebulun</rdfs:label>
        <rdfs:label xml:lang="en">tribe of Zebulun</rdfs:label>
    </owl:NamedIndividual>
    


    <!-- http://semanticbible.org/ns/2006/NTNames#Troas -->

    <owl:NamedIndividual rdf:about="http://semanticbible.org/ns/2006/NTNames#Troas">
        <rdfs:label xml:lang="en">Troas</rdfs:label>
        <visitedPlaceOf rdf:resource="http://semanticbible.org/ns/2006/NTNames#GaiusOfDerbe"/>
    </owl:NamedIndividual>
    


    <!-- http://semanticbible.org/ns/2006/NTNames#TroasGeodata -->

    <owl:NamedIndividual rdf:about="http://semanticbible.org/ns/2006/NTNames#TroasGeodata">
        <rdfs:label xml:lang="en">geodata for Troas</rdfs:label>
        <longitude rdf:datatype="http://www.w3.org/2001/XMLSchema#double">26.08148842388431</longitude>
        <latitude rdf:datatype="http://www.w3.org/2001/XMLSchema#double">39.50181513585497</latitude>
    </owl:NamedIndividual>
    


    <!-- http://semanticbible.org/ns/2006/NTNames#Trophimus -->

    <owl:NamedIndividual rdf:about="http://semanticbible.org/ns/2006/NTNames#Trophimus">
        <rdf:type rdf:resource="http://semanticbible.org/ns/2006/NTNames#Man"/>
        <rdfs:label xml:lang="en">Trophimus</rdfs:label>
    </owl:NamedIndividual>
    


    <!-- http://semanticbible.org/ns/2006/NTNames#Tryphaena -->

    <owl:NamedIndividual rdf:about="http://semanticbible.org/ns/2006/NTNames#Tryphaena">
        <rdfs:label xml:lang="en">Tryphaena</rdfs:label>
    </owl:NamedIndividual>
    


    <!-- http://semanticbible.org/ns/2006/NTNames#Tryphosa -->

    <owl:NamedIndividual rdf:about="http://semanticbible.org/ns/2006/NTNames#Tryphosa">
        <rdfs:label xml:lang="en">Tryphosa</rdfs:label>
        <residentPlace rdf:resource="http://semanticbible.org/ns/2006/NTNames#Rome"/>
    </owl:NamedIndividual>
    


    <!-- http://semanticbible.org/ns/2006/NTNames#Tychicus -->

    <owl:NamedIndividual rdf:about="http://semanticbible.org/ns/2006/NTNames#Tychicus">
        <rdfs:label xml:lang="en">Tychicus</rdfs:label>
        <collaboratesWith rdf:resource="http://semanticbible.org/ns/2006/NTNames#Aristarchus"/>
    </owl:NamedIndividual>
    


    <!-- http://semanticbible.org/ns/2006/NTNames#Tyrannus -->

    <owl:NamedIndividual rdf:about="http://semanticbible.org/ns/2006/NTNames#Tyrannus">
        <rdfs:label xml:lang="en">Tyrannus</rdfs:label>
    </owl:NamedIndividual>
    


    <!-- http://semanticbible.org/ns/2006/NTNames#Tyre -->

    <owl:NamedIndividual rdf:about="http://semanticbible.org/ns/2006/NTNames#Tyre">
        <rdfs:label xml:lang="en">Tyre</rdfs:label>
        <subregionOf rdf:resource="http://semanticbible.org/ns/2006/NTNames#Phoenicia"/>
    </owl:NamedIndividual>
    


    <!-- http://semanticbible.org/ns/2006/NTNames#TyreGeodata -->

    <owl:NamedIndividual rdf:about="http://semanticbible.org/ns/2006/NTNames#TyreGeodata">
        <rdf:type rdf:resource="http://semanticbible.org/ns/2006/NTNames#GeographicLocation"/>
        <rdfs:label xml:lang="en">geodata for Tyre</rdfs:label>
    </owl:NamedIndividual>
    


    <!-- http://semanticbible.org/ns/2006/NTNames#Urbanus -->

    <owl:NamedIndividual rdf:about="http://semanticbible.org/ns/2006/NTNames#Urbanus">
        <rdfs:label xml:lang="en">Urbanus</rdfs:label>
    </owl:NamedIndividual>
    


    <!-- http://semanticbible.org/ns/2006/NTNames#Uriah -->

    <owl:NamedIndividual rdf:about="http://semanticbible.org/ns/2006/NTNames#Uriah">
        <rdfs:label xml:lang="en">Uriah</rdfs:label>
        <hasOnlyGenealogyMention rdf:datatype="http://www.w3.org/2001/XMLSchema#boolean">true</hasOnlyGenealogyMention>
        <rdfs:comment xml:lang="en">From OT sources, Uriah was a Hittite and a soldier in David&#39;s army (therefore having both collaboratesWith and hasEnemy relationships with David). </rdfs:comment>
    </owl:NamedIndividual>
    


    <!-- http://semanticbible.org/ns/2006/NTNames#Uzziah -->

    <owl:NamedIndividual rdf:about="http://semanticbible.org/ns/2006/NTNames#Uzziah">
        <rdfs:label xml:lang="en">Uzziah</rdfs:label>
        <rdfs:comment rdf:datatype="http://www.w3.org/2001/XMLSchema#string">His occupation as King comes from Old Testament sources. </rdfs:comment>
        <ethnicity rdf:resource="http://semanticbible.org/ns/2006/NTNames#Jewish"/>
    </owl:NamedIndividual>
    


    <!-- http://semanticbible.org/ns/2006/NTNames#Zacchaeus -->

    <owl:NamedIndividual rdf:about="http://semanticbible.org/ns/2006/NTNames#Zacchaeus">
        <rdfs:label xml:lang="en">Zacchaeus</rdfs:label>
    </owl:NamedIndividual>
    


    <!-- http://semanticbible.org/ns/2006/NTNames#Zadok -->

    <owl:NamedIndividual rdf:about="http://semanticbible.org/ns/2006/NTNames#Zadok">
        <rdfs:label xml:lang="en">Zadok</rdfs:label>
    </owl:NamedIndividual>
    


    <!-- http://semanticbible.org/ns/2006/NTNames#Zarephath -->

    <owl:NamedIndividual rdf:about="http://semanticbible.org/ns/2006/NTNames#Zarephath">
        <rdfs:label xml:lang="en">Zarephath</rdfs:label>
        <rdfs:comment xml:lang="en">Jesus recounts the story of Elijah being sent to a widow of Zarephath as an example of God blessing those outside the nation of Israel.</rdfs:comment>
    </owl:NamedIndividual>
    


    <!-- http://semanticbible.org/ns/2006/NTNames#Zealot -->

    <owl:NamedIndividual rdf:about="http://semanticbible.org/ns/2006/NTNames#Zealot">
        <rdfs:label xml:lang="en">Zealot</rdfs:label>
    </owl:NamedIndividual>
    


    <!-- http://semanticbible.org/ns/2006/NTNames#Zebedee -->

    <owl:NamedIndividual rdf:about="http://semanticbible.org/ns/2006/NTNames#Zebedee">
        <rdfs:label xml:lang="en">Zebedee</rdfs:label>
        <parentOf rdf:resource="http://semanticbible.org/ns/2006/NTNames#JohnSonOfZebedee"/>
    </owl:NamedIndividual>
    


    <!-- http://semanticbible.org/ns/2006/NTNames#Zebulun -->

    <owl:NamedIndividual rdf:about="http://semanticbible.org/ns/2006/NTNames#Zebulun">
        <rdfs:label xml:lang="en">Zebulun</rdfs:label>
    </owl:NamedIndividual>
    


    <!-- http://semanticbible.org/ns/2006/NTNames#Zechariah -->

    <owl:NamedIndividual rdf:about="http://semanticbible.org/ns/2006/NTNames#Zechariah">
        <rdfs:label xml:lang="en">Zechariah</rdfs:label>
    </owl:NamedIndividual>
    


    <!-- http://semanticbible.org/ns/2006/NTNames#ZechariahSonOfBarachiah -->

    <owl:NamedIndividual rdf:about="http://semanticbible.org/ns/2006/NTNames#ZechariahSonOfBarachiah">
        <rdfs:label xml:lang="en">Zechariah</rdfs:label>
    </owl:NamedIndividual>
    


    <!-- http://semanticbible.org/ns/2006/NTNames#Zenas -->

    <owl:NamedIndividual rdf:about="http://semanticbible.org/ns/2006/NTNames#Zenas">
        <rdfs:label xml:lang="en">Zenas</rdfs:label>
    </owl:NamedIndividual>
    


    <!-- http://semanticbible.org/ns/2006/NTNames#Zerah -->

    <owl:NamedIndividual rdf:about="http://semanticbible.org/ns/2006/NTNames#Zerah">
        <rdfs:label xml:lang="en">Zerah</rdfs:label>
    </owl:NamedIndividual>
    


    <!-- http://semanticbible.org/ns/2006/NTNames#Zerubbabel -->

    <owl:NamedIndividual rdf:about="http://semanticbible.org/ns/2006/NTNames#Zerubbabel">
        <rdfs:label xml:lang="en">Zerubbabel</rdfs:label>
    </owl:NamedIndividual>
    


    <!-- http://semanticbible.org/ns/2006/NTNames#Zeus -->

    <owl:NamedIndividual rdf:about="http://semanticbible.org/ns/2006/NTNames#Zeus">
        <rdfs:label xml:lang="en">Zeus</rdfs:label>
    </owl:NamedIndividual>
    


    <!-- http://semanticbible.org/ns/2006/NTNames#Zion -->

    <owl:NamedIndividual rdf:about="http://semanticbible.org/ns/2006/NTNames#Zion">
        <rdfs:label xml:lang="en">Zion</rdfs:label>
    </owl:NamedIndividual>
    


    <!-- 
    ///////////////////////////////////////////////////////////////////////////////////////
    //
    // General axioms
    //
    ///////////////////////////////////////////////////////////////////////////////////////
     -->

    <rdf:Description>
        <rdf:type rdf:resource="http://www.w3.org/2002/07/owl#AllDifferent"/>
        <owl:distinctMembers rdf:parseType="Collection">
            <rdf:Description rdf:about="http://semanticbible.org/ns/2006/NTNames#Galilean"/>
            <rdf:Description rdf:about="http://semanticbible.org/ns/2006/NTNames#Samaritan"/>
        </owl:distinctMembers>
    </rdf:Description>
    <owl:Restriction>
        <owl:disjointWith>
            <owl:Restriction>
                <owl:onProperty rdf:resource="http://semanticbible.org/ns/2006/NTNames#hasAntagonist"/>
                <owl:someValuesFrom rdf:resource="http://www.w3.org/2002/07/owl#Thing"/>
            </owl:Restriction>
        </owl:disjointWith>
        <owl:onProperty rdf:resource="http://semanticbible.org/ns/2006/NTNames#collaboratesWith"/>
        <owl:someValuesFrom rdf:resource="http://www.w3.org/2002/07/owl#Thing"/>
    </owl:Restriction>
    <owl:Restriction>
        <owl:disjointWith>
            <owl:Restriction>
                <owl:onProperty rdf:resource="http://semanticbible.org/ns/2006/NTNames#hasEnemy"/>
                <owl:someValuesFrom rdf:resource="http://www.w3.org/2002/07/owl#Thing"/>
            </owl:Restriction>
        </owl:disjointWith>
        <owl:onProperty rdf:resource="http://semanticbible.org/ns/2006/NTNames#antagonistOf"/>
        <owl:someValuesFrom rdf:resource="http://www.w3.org/2002/07/owl#Thing"/>
    </owl:Restriction>
    <owl:Restriction>
        <owl:disjointWith>
            <owl:Restriction>
                <owl:onProperty rdf:resource="http://semanticbible.org/ns/2006/NTNames#subregionOf"/>
                <owl:someValuesFrom rdf:resource="http://www.w3.org/2002/07/owl#Thing"/>
            </owl:Restriction>
        </owl:disjointWith>
        <owl:disjointWith>
            <owl:Restriction>
                <owl:disjointWith>
                    <owl:Restriction>
                        <owl:onProperty rdf:resource="http://semanticbible.org/ns/2006/NTNames#subregionOf"/>
                        <owl:someValuesFrom rdf:resource="http://www.w3.org/2002/07/owl#Thing"/>
                    </owl:Restriction>
                </owl:disjointWith>
                <owl:onProperty rdf:resource="http://semanticbible.org/ns/2006/NTNames#subregion"/>
                <owl:someValuesFrom rdf:resource="http://www.w3.org/2002/07/owl#Thing"/>
            </owl:Restriction>
        </owl:disjointWith>
        <owl:disjointWith>
            <owl:Restriction>
                <owl:disjointWith>
                    <owl:Restriction>
                        <owl:onProperty rdf:resource="http://semanticbible.org/ns/2006/NTNames#subregionOf"/>
                        <owl:someValuesFrom rdf:resource="http://www.w3.org/2002/07/owl#Thing"/>
                    </owl:Restriction>
                </owl:disjointWith>
                <owl:disjointWith>
                    <owl:Restriction>
                        <owl:disjointWith>
                            <owl:Restriction>
                                <owl:onProperty rdf:resource="http://semanticbible.org/ns/2006/NTNames#subregionOf"/>
                                <owl:someValuesFrom rdf:resource="http://www.w3.org/2002/07/owl#Thing"/>
                            </owl:Restriction>
                        </owl:disjointWith>
                        <owl:onProperty rdf:resource="http://semanticbible.org/ns/2006/NTNames#subregion"/>
                        <owl:someValuesFrom rdf:resource="http://www.w3.org/2002/07/owl#Thing"/>
                    </owl:Restriction>
                </owl:disjointWith>
                <owl:disjointWith>
                    <owl:Restriction>
                        <owl:onProperty rdf:resource="http://semanticbible.org/ns/2006/NTNames#residentPlaceOf"/>
                        <owl:someValuesFrom rdf:resource="http://www.w3.org/2002/07/owl#Thing"/>
                    </owl:Restriction>
                </owl:disjointWith>
                <owl:onProperty rdf:resource="http://semanticbible.org/ns/2006/NTNames#nativePlaceOf"/>
                <owl:someValuesFrom rdf:resource="http://www.w3.org/2002/07/owl#Thing"/>
            </owl:Restriction>
        </owl:disjointWith>
        <owl:onProperty rdf:resource="http://semanticbible.org/ns/2006/NTNames#location"/>
        <owl:someValuesFrom rdf:resource="http://www.w3.org/2002/07/owl#Thing"/>
    </owl:Restriction>
    <owl:Restriction>
        <owl:disjointWith>
            <owl:Restriction>
                <owl:onProperty rdf:resource="http://semanticbible.org/ns/2006/NTNames#siblingOf"/>
                <owl:someValuesFrom rdf:resource="http://www.w3.org/2002/07/owl#Thing"/>
            </owl:Restriction>
        </owl:disjointWith>
        <owl:onProperty rdf:resource="http://semanticbible.org/ns/2006/NTNames#parentOf"/>
        <owl:someValuesFrom rdf:resource="http://www.w3.org/2002/07/owl#Thing"/>
    </owl:Restriction>
    <owl:Restriction>
        <owl:disjointWith>
            <owl:Restriction>
                <owl:onProperty rdf:resource="http://semanticbible.org/ns/2006/NTNames#visitedPlace"/>
                <owl:someValuesFrom rdf:resource="http://www.w3.org/2002/07/owl#Thing"/>
            </owl:Restriction>
        </owl:disjointWith>
        <owl:onProperty rdf:resource="http://semanticbible.org/ns/2006/NTNames#religiousBelief"/>
        <owl:someValuesFrom rdf:resource="http://www.w3.org/2002/07/owl#Thing"/>
    </owl:Restriction>
    <owl:Restriction>
        <owl:disjointWith>
            <owl:Restriction>
                <owl:onProperty rdf:resource="http://semanticbible.org/ns/2006/NTNames#residentPlace"/>
                <owl:someValuesFrom rdf:resource="http://www.w3.org/2002/07/owl#Thing"/>
            </owl:Restriction>
        </owl:disjointWith>
        <owl:disjointWith>
            <owl:Restriction>
                <owl:onProperty rdf:resource="http://semanticbible.org/ns/2006/NTNames#hasAntagonist"/>
                <owl:someValuesFrom rdf:resource="http://www.w3.org/2002/07/owl#Thing"/>
            </owl:Restriction>
        </owl:disjointWith>
        <owl:disjointWith>
            <owl:Restriction>
                <owl:disjointWith>
                    <owl:Restriction>
                        <owl:onProperty rdf:resource="http://semanticbible.org/ns/2006/NTNames#residentPlace"/>
                        <owl:someValuesFrom rdf:resource="http://www.w3.org/2002/07/owl#Thing"/>
                    </owl:Restriction>
                </owl:disjointWith>
                <owl:onProperty rdf:resource="http://semanticbible.org/ns/2006/NTNames#nativePlace"/>
                <owl:someValuesFrom rdf:resource="http://www.w3.org/2002/07/owl#Thing"/>
            </owl:Restriction>
        </owl:disjointWith>
        <owl:onProperty rdf:resource="http://semanticbible.org/ns/2006/NTNames#enemyOf"/>
        <owl:someValuesFrom rdf:resource="http://www.w3.org/2002/07/owl#Thing"/>
    </owl:Restriction>
</rdf:RDF>



<!-- Generated by the OWL API (version 3.2.4.1806) http://owlapi.sourceforge.net -->

